@prefix : <http://www.semanticweb.org/ghiot/ontologies/2023/11/meaw/> .
@prefix owl: <http://www.w3.org/2002/07/owl#> .
@prefix rdf: <http://www.w3.org/1999/02/22-rdf-syntax-ns#> .
@prefix xml: <http://www.w3.org/XML/1998/namespace> .
@prefix xsd: <http://www.w3.org/2001/XMLSchema#> .
@prefix meaw: <http://www.semanticweb.org/ghiot/ontologies/2023/11/meaw#> .
@prefix rdfs: <http://www.w3.org/2000/01/rdf-schema#> .
@base <http://www.semanticweb.org/ghiot/ontologies/2023/11/meaw/> .

<http://www.semanticweb.org/ghiot/ontologies/2023/11/meaw> rdf:type owl:Ontology ;
                                                            rdfs:comment "First modelet of the Multimodal Emotio Annotation Ontology. Developed within my thesis research in collaboration with the netherlands Institute for Sound and Vision." .

#################################################################
#    Object Properties
#################################################################

###  http://www.semanticweb.org/ghiot/ontologies/2023/11/meaw#addresses
meaw:addresses rdf:type owl:ObjectProperty ;
               owl:inverseOf :isAddressedIn .


###  http://www.semanticweb.org/ghiot/ontologies/2023/11/meaw#hasSpeaker
meaw:hasSpeaker rdf:type owl:ObjectProperty ;
                owl:inverseOf :isSpeakerIn .


###  http://www.semanticweb.org/ghiot/ontologies/2023/11/meaw/broadcastedBy
:broadcastedBy rdf:type owl:ObjectProperty ;
               rdfs:domain :TalkShowSituation ;
               rdfs:range :Broadcaster .


###  http://www.semanticweb.org/ghiot/ontologies/2023/11/meaw/expressedIn
:expressedIn rdf:type owl:ObjectProperty ;
             rdfs:domain :Emotion ;
             rdfs:range :EmotionRelation .


###  http://www.semanticweb.org/ghiot/ontologies/2023/11/meaw/expressesEmotion
:expressesEmotion rdf:type owl:ObjectProperty ;
                  rdfs:domain :EmotionRelation ;
                  rdfs:range :Emotion .


###  http://www.semanticweb.org/ghiot/ontologies/2023/11/meaw/hasConversationalContext
:hasConversationalContext rdf:type owl:ObjectProperty ;
                          rdfs:domain :ConversationalRole ;
                          rdfs:range :TalkShowSituation .


###  http://www.semanticweb.org/ghiot/ontologies/2023/11/meaw/hasFrameContext
:hasFrameContext rdf:type owl:ObjectProperty ;
                 rdfs:domain :EmotionRelation ;
                 rdfs:range :ConversationalFrame .


###  http://www.semanticweb.org/ghiot/ontologies/2023/11/meaw/hasGender
:hasGender rdf:type owl:ObjectProperty ;
           rdfs:domain :Person ;
           rdfs:range :Gender .


###  http://www.semanticweb.org/ghiot/ontologies/2023/11/meaw/hasInScope
:hasInScope rdf:type owl:ObjectProperty ;
            rdfs:domain :TalkShowSituation ;
            rdfs:range :EmotionRelation .


###  http://www.semanticweb.org/ghiot/ontologies/2023/11/meaw/hasRole
:hasRole rdf:type owl:ObjectProperty ;
         rdfs:domain :ConversationalRole ;
         rdfs:range :Role .


###  http://www.semanticweb.org/ghiot/ontologies/2023/11/meaw/hasRoleInConversation
:hasRoleInConversation rdf:type owl:ObjectProperty ;
                       rdfs:domain :Agent ;
                       rdfs:range :ConversationalRole .


###  http://www.semanticweb.org/ghiot/ontologies/2023/11/meaw/includes
:includes rdf:type owl:ObjectProperty ;
          owl:inverseOf :isIncludedIn ;
          rdfs:domain :BasicEmotion ;
          rdfs:range :EmotionState .


###  http://www.semanticweb.org/ghiot/ontologies/2023/11/meaw/isAddressedIn
:isAddressedIn rdf:type owl:ObjectProperty ;
               rdfs:domain :Agent ;
               rdfs:range :EmotionRelation .


###  http://www.semanticweb.org/ghiot/ontologies/2023/11/meaw/isIncludedIn
:isIncludedIn rdf:type owl:ObjectProperty .


###  http://www.semanticweb.org/ghiot/ontologies/2023/11/meaw/isSpeakerIn
:isSpeakerIn rdf:type owl:ObjectProperty ;
             rdfs:domain :Agent ;
             rdfs:range :EmotionRelation .


#################################################################
#    Data properties
#################################################################

###  http://www.semanticweb.org/ghiot/ontologies/2023/11/meaw#hasText
meaw:hasText rdf:type owl:DatatypeProperty ;
             rdfs:domain :EmotionRelation ;
             rdfs:range xsd:string ;
             rdfs:comment "the ASR transcript of the text of the utterance." .


###  http://www.semanticweb.org/ghiot/ontologies/2023/11/meaw/hasDate
:hasDate rdf:type owl:DatatypeProperty ;
         rdfs:domain :TalkShowSituation ;
         rdfs:range xsd:string .


###  http://www.semanticweb.org/ghiot/ontologies/2023/11/meaw/hasDescription
:hasDescription rdf:type owl:DatatypeProperty ;
                rdfs:domain :TalkShowSituation ;
                rdfs:range xsd:string .


###  http://www.semanticweb.org/ghiot/ontologies/2023/11/meaw/hasEnd
:hasEnd rdf:type owl:DatatypeProperty ;
        rdfs:range xsd:string .


###  http://www.semanticweb.org/ghiot/ontologies/2023/11/meaw/hasFileTitle
:hasFileTitle rdf:type owl:DatatypeProperty ;
              rdfs:domain :TalkShowSituation ;
              rdfs:range xsd:string .


###  http://www.semanticweb.org/ghiot/ontologies/2023/11/meaw/hasIdentifier
:hasIdentifier rdf:type owl:DatatypeProperty ;
               rdfs:domain :TalkShowSituation ;
               rdfs:range xsd:string .


###  http://www.semanticweb.org/ghiot/ontologies/2023/11/meaw/hasNameSource
:hasNameSource rdf:type owl:DatatypeProperty ;
               rdfs:domain :NamedPerson ;
               rdfs:range xsd:string ;
               rdfs:comment "The source where the name of the speaker comes from, either the audio of the video, the overlaid captions or the annotator’s recognition." .


###  http://www.semanticweb.org/ghiot/ontologies/2023/11/meaw/hasStart
:hasStart rdf:type owl:DatatypeProperty ;
          rdfs:range xsd:string .


###  http://www.semanticweb.org/ghiot/ontologies/2023/11/meaw/hasSupposedAge
:hasSupposedAge rdf:type owl:DatatypeProperty ;
                rdfs:domain :Person ;
                rdfs:range xsd:int .


###  http://www.semanticweb.org/ghiot/ontologies/2023/11/meaw/hasTitle
:hasTitle rdf:type owl:DatatypeProperty ;
          rdfs:domain :TalkShowSituation ;
          rdfs:range xsd:string .


###  http://www.semanticweb.org/ghiot/ontologies/2023/11/meaw/isAbout
:isAbout rdf:type owl:DatatypeProperty ;
         rdfs:domain :TalkShowSituation ;
         rdfs:range xsd:string .


#################################################################
#    Classes
#################################################################

###  http://www.semanticweb.org/ghiot/ontologies/2023/11/meaw/Agent
:Agent rdf:type owl:Class ;
       rdfs:comment """The Agent is the person talking the most in an utterance. Given the automatic subdivision of a talk show video, there might at times be more than one people talking in the same utterance. In these cases, the person that is occupying the most speaking time should be identified as speaker. If two or more people are occupying the same amount of time, the person expressing more clearly some emotional content should be the identified speaker. 
The speaker can be named, either by the host or by overlaid captions. If the annotator recognizes someone who is unnamed, they can integrate the name of the person. In either case, the provenance of the name must be provided.""" .


###  http://www.semanticweb.org/ghiot/ontologies/2023/11/meaw/BasicEmotion
:BasicEmotion rdf:type owl:Class ;
              rdfs:subClassOf :Emotion ;
              owl:disjointWith :EmotionState ;
              rdfs:comment "An Ekman basic emotion, plus neutrality." .


###  http://www.semanticweb.org/ghiot/ontologies/2023/11/meaw/Broadcaster
:Broadcaster rdf:type owl:Class ;
             rdfs:comment "The name of the broadcaster that aired the talk show." .


###  http://www.semanticweb.org/ghiot/ontologies/2023/11/meaw/ConversationalFrame
:ConversationalFrame rdf:type owl:Class ;
                     rdfs:comment "Considering talk shows as a predefined setting where there are specific conversational conventions, roles and patterns (in other words, a “genre” as defined by van Leeuwen: “Genres link the text with a special context and regulate the adequate selection of semiotic means dependent on that context.” A conversational frame is the identified conversational block that defines the utterance." .


###  http://www.semanticweb.org/ghiot/ontologies/2023/11/meaw/ConversationalRole
:ConversationalRole rdf:type owl:Class ;
                    rdfs:comment "The Class that connects a Role covered by a person to the Talk Show in which the person had that role." .


###  http://www.semanticweb.org/ghiot/ontologies/2023/11/meaw/Emotion
:Emotion rdf:type owl:Class ;
         rdfs:comment "Represents the emotion identified and annotated in a multimodal utterance by an annotator. A taxonomy of emotions is given, where each of the five Ekman basic emotions include a variety of emotional states, as defined by http://atlasofemotions.org/" .


###  http://www.semanticweb.org/ghiot/ontologies/2023/11/meaw/EmotionRelation
:EmotionRelation rdf:type owl:Class ;
                 rdfs:subClassOf [ owl:intersectionOf ( [ rdf:type owl:Restriction ;
                                                          owl:onProperty :expressesEmotion ;
                                                          owl:qualifiedCardinality "1"^^xsd:nonNegativeInteger ;
                                                          owl:onClass :BasicEmotion
                                                        ]
                                                        [ rdf:type owl:Restriction ;
                                                          owl:onProperty :expressesEmotion ;
                                                          owl:maxQualifiedCardinality "2"^^xsd:nonNegativeInteger ;
                                                          owl:onClass :EmotionState
                                                        ]
                                                      ) ;
                                   rdf:type owl:Class
                                 ] ,
                                 [ rdf:type owl:Restriction ;
                                   owl:onProperty :hasStart ;
                                   owl:minQualifiedCardinality "1"^^xsd:nonNegativeInteger ;
                                   owl:onDataRange xsd:string
                                 ] ;
                 rdfs:comment "An emotion Relation, represents the utterance as the smallest sub clip of a talk show video, hence bringing together the three modalities of video and verbal expression (audio and text in the form of Automatic Speech transcript ASR). It is a subclass of tis:TimeIndexedSituation, defined as a Situation (a class to represent things that have something in common) with a specified time interval. It is also defined by a unique identifier." .


###  http://www.semanticweb.org/ghiot/ontologies/2023/11/meaw/EmotionState
:EmotionState rdf:type owl:Class ;
              rdfs:subClassOf :Emotion ;
              rdfs:comment "A fine grained emotion that can be considered an emotional state belonging to one of Ekman's basic emotion." .


###  http://www.semanticweb.org/ghiot/ontologies/2023/11/meaw/Gender
:Gender rdf:type owl:Class ;
        rdfs:comment "The gender, as recognized by the annotator, of the agent who's speaking in the utterance and that expresses the emotion." .


###  http://www.semanticweb.org/ghiot/ontologies/2023/11/meaw/Group
:Group rdf:type owl:Class ;
       rdfs:subClassOf :Agent ;
       owl:disjointWith :Person ;
       rdfs:comment "A collective agent, to represent the studio audience or utterances where multiple speakers are talking over each other." .


###  http://www.semanticweb.org/ghiot/ontologies/2023/11/meaw/NamedPerson
:NamedPerson rdf:type owl:Class ;
             rdfs:subClassOf :Person ,
                             [ rdf:type owl:Restriction ;
                               owl:onProperty :hasNameSource ;
                               owl:someValuesFrom [ rdf:type rdfs:Datatype ;
                                                    owl:oneOf [ rdf:type rdf:List ;
                                                                rdf:first "annotator" ;
                                                                rdf:rest [ rdf:type rdf:List ;
                                                                           rdf:first "audio" ;
                                                                           rdf:rest [ rdf:type rdf:List ;
                                                                                      rdf:first "captions" ;
                                                                                      rdf:rest rdf:nil
                                                                                    ]
                                                                         ]
                                                              ]
                                                  ]
                             ] ;
             rdfs:comment "A single speaker who is also recognized and named." .


###  http://www.semanticweb.org/ghiot/ontologies/2023/11/meaw/Person
:Person rdf:type owl:Class ;
        rdfs:subClassOf :Agent ;
        rdfs:comment "A single speaker." .


###  http://www.semanticweb.org/ghiot/ontologies/2023/11/meaw/Role
:Role rdf:type owl:Class ;
      rdfs:comment "Represents the roles that are identifyed in a Talk Show conversation as a non spontaneous conversation genre." .


###  http://www.semanticweb.org/ghiot/ontologies/2023/11/meaw/TalkShowSituation
:TalkShowSituation rdf:type owl:Class ;
                   rdfs:subClassOf [ rdf:type owl:Restriction ;
                                     owl:onProperty :hasInScope ;
                                     owl:someValuesFrom :EmotionRelation
                                   ] ,
                                   [ rdf:type owl:Restriction ;
                                     owl:onProperty :hasFileTitle ;
                                     owl:qualifiedCardinality "1"^^xsd:nonNegativeInteger ;
                                     owl:onDataRange xsd:string
                                   ] ,
                                   [ rdf:type owl:Restriction ;
                                     owl:onProperty :hasIdentifier ;
                                     owl:qualifiedCardinality "1"^^xsd:nonNegativeInteger ;
                                     owl:onDataRange xsd:string
                                   ] ;
                   rdfs:comment "It represents a video of a talk show, or an extract from it, retrieved from Sound and Vision archive through the media suite. It is defined by a file titlr, a unique identifier, a date, a broadcaster name, a description (if present in the archive metadata) and subjectterms from the archive GTAA that identify the topic of the video. If the talk show situation is an extract from the whole video, these metadata refer to the whole video rather than to the subsection of it, for they are automatically retrieved from the item’s metadata provided by Sound and Vision." .


#################################################################
#    Individuals
#################################################################

###  http://www.semanticweb.org/ghiot/ontologies/2023/11/meaw#2101608040029452931_guest
<http://www.semanticweb.org/ghiot/ontologies/2023/11/meaw#2101608040029452931_guest> rdf:type owl:NamedIndividual ,
                                                                                              :ConversationalRole ;
                                                                                     :hasConversationalContext :welles_nietes ;
                                                                                     :hasRole :guest ;
                                                                                     rdfs:comment "The role of guest in the TalkShowSituation Welles Nietes: WELLES NIETES - WELLES NIETES;Mag je op televisie zeggen wat je denkt?" .


###  http://www.semanticweb.org/ghiot/ontologies/2023/11/meaw#2101608040029452931_host
<http://www.semanticweb.org/ghiot/ontologies/2023/11/meaw#2101608040029452931_host> rdf:type owl:NamedIndividual ,
                                                                                             :ConversationalRole ;
                                                                                    :hasConversationalContext :welles_nietes ;
                                                                                    :hasRole :host ;
                                                                                    rdfs:comment "The role of host in the TalkShowSituation Welles Nietes: WELLES NIETES - WELLES NIETES;Mag je op televisie zeggen wat je denkt?" .


###  http://www.semanticweb.org/ghiot/ontologies/2023/11/meaw#2101608040029452931_studio_audience
<http://www.semanticweb.org/ghiot/ontologies/2023/11/meaw#2101608040029452931_studio_audience> rdf:type owl:NamedIndividual ,
                                                                                                        :ConversationalRole ;
                                                                                               :hasConversationalContext :welles_nietes ;
                                                                                               :hasRole :studio_audience ;
                                                                                               rdfs:comment "The role of studio audience in the TalkShowSituation Welles Nietes: WELLES NIETES - WELLES NIETES;Mag je op televisie zeggen wat je denkt?" .


###  http://www.semanticweb.org/ghiot/ontologies/2023/11/meaw#40_neutrality
<http://www.semanticweb.org/ghiot/ontologies/2023/11/meaw#40_neutrality> rdf:type owl:NamedIndividual ,
                                                                                  :EmotionRelation ;
                                                                         :expressesEmotion :neutrality ;
                                                                         :hasFrameContext :introducing_topic ;
                                                                         meaw:hasText "In de zaal zijn nogal wat mensen die zeggen tegen ons wij zijn af en toe best gekwetst door wat er op de televisie getoond wordt u knikt ja u knikt." ;
                                                                         :hasStart "394" ;
                                                                         rdfs:comment "EmotionRelation, the individual naming convention is the sequence number of the utterance + the annotated emotion." .


###  http://www.semanticweb.org/ghiot/ontologies/2023/11/meaw#41_sadness
<http://www.semanticweb.org/ghiot/ontologies/2023/11/meaw#41_sadness> rdf:type owl:NamedIndividual ,
                                                                               :EmotionRelation ;
                                                                      :expressesEmotion :sadness ;
                                                                      :hasFrameContext :presenting_opinion ;
                                                                      meaw:hasText "Na jaren gekwetst door de laatste uitzending van adelheid roosen over de transseksuele ik vond dat het in het belachelijke getrokken werd en ik denk dus dat er een heleboel mensen daardoor gekwetst zijn want werd in het seksuele vlak getrokken en dat vond ik dus niet goed." ;
                                                                      :hasEnd "" ;
                                                                      :hasStart "405" .


###  http://www.semanticweb.org/ghiot/ontologies/2023/11/meaw#45_neutrality
<http://www.semanticweb.org/ghiot/ontologies/2023/11/meaw#45_neutrality> rdf:type owl:NamedIndividual ,
                                                                                  :EmotionRelation ;
                                                                         :hasFrameContext :giving_talking_space ;
                                                                         meaw:hasText "Nou ze adelheid u zegt het is kwetsend aan het zit bij ons in de studio we hebben van veel mensen gehoord dat een nacht zo kwetsend is die manier hÃ¨ die je bij jou in de uitzending was mevrouw mevrouw." ;
                                                                         :hasEnd "" ;
                                                                         :hasStart "454" .


###  http://www.semanticweb.org/ghiot/ontologies/2023/11/meaw#46_fear
<http://www.semanticweb.org/ghiot/ontologies/2023/11/meaw#46_fear> rdf:type owl:NamedIndividual ,
                                                                            :EmotionRelation ;
                                                                   :expressesEmotion :fear ,
                                                                                     :nervousness ;
                                                                   :hasFrameContext :saying_something_wrong ;
                                                                   meaw:hasText "Vrouw en wat ik nu zeg maar zo snel zou dus want dit nou dit voorbeeld aanhalen." ;
                                                                   :hasStart "469" .


###  http://www.semanticweb.org/ghiot/ontologies/2023/11/meaw#57_disgust
<http://www.semanticweb.org/ghiot/ontologies/2023/11/meaw#57_disgust> rdf:type owl:NamedIndividual ,
                                                                               :EmotionRelation ;
                                                                      :expressesEmotion :aversion ,
                                                                                        :disgust ;
                                                                      :hasFrameContext :presenting_opinion ;
                                                                      meaw:hasText "Ja ik woon vragen je hoorde zoveel kan je geen programma onderhand meer beginnen of moet homoseksuelen als transseksueel aan te pas komt zo over gewone mensen praten." ;
                                                                      :hasEnd "" ;
                                                                      :hasStart "612" .


###  http://www.semanticweb.org/ghiot/ontologies/2023/11/meaw#58_anger
<http://www.semanticweb.org/ghiot/ontologies/2023/11/meaw#58_anger> rdf:type owl:NamedIndividual ,
                                                                             :EmotionRelation ;
                                                                    :expressesEmotion :anger ,
                                                                                      :argumentativeness ;
                                                                    :hasFrameContext :disagreeing_by_interrupting ;
                                                                    meaw:hasText "Dat zijn." ;
                                                                    :hasStart "624" .


###  http://www.semanticweb.org/ghiot/ontologies/2023/11/meaw/abhorrence
:abhorrence rdf:type owl:NamedIndividual ,
                     :EmotionState ;
            rdfs:comment "A mixture of intense disgust and hatred." .


###  http://www.semanticweb.org/ghiot/ontologies/2023/11/meaw/adelheid_roosen
:adelheid_roosen rdf:type owl:NamedIndividual ,
                          :NamedPerson ;
                 :hasGender :female ;
                 :hasRoleInConversation <http://www.semanticweb.org/ghiot/ontologies/2023/11/meaw#2101608040029452931_guest> ;
                 :isAddressedIn <http://www.semanticweb.org/ghiot/ontologies/2023/11/meaw#45_neutrality> ,
                                <http://www.semanticweb.org/ghiot/ontologies/2023/11/meaw#46_fear> ;
                 :isSpeakerIn <http://www.semanticweb.org/ghiot/ontologies/2023/11/meaw#58_anger> ;
                 :hasNameSource "captions" ;
                 :hasSupposedAge "33"^^xsd:int .


###  http://www.semanticweb.org/ghiot/ontologies/2023/11/meaw/agreeing
:agreeing rdf:type owl:NamedIndividual ,
                   :ConversationalFrame ;
          rdfs:comment "A Conversational Frame where the speaker recalls a personal experience or another type of subjective argument to support the validity of their perspective on the topic of conversation." .


###  http://www.semanticweb.org/ghiot/ontologies/2023/11/meaw/amusement
:amusement rdf:type owl:NamedIndividual ,
                    :EmotionState ;
           rdfs:comment "Light, playful feelings of enjoyment and good humor." .


###  http://www.semanticweb.org/ghiot/ontologies/2023/11/meaw/anger
:anger rdf:type owl:NamedIndividual ,
                :BasicEmotion ;
       :includes :annoyance ,
                 :argumentativeness ,
                 :bitterness ,
                 :exasperation ,
                 :frustration ,
                 :fury ,
                 :vengefulness ;
       rdfs:comment "We feel anger when we are mentally or physically blocked. Anger varies in strength and frequency in our lives. (description from http://atlasofemotions.org/)" .


###  http://www.semanticweb.org/ghiot/ontologies/2023/11/meaw/anguish
:anguish rdf:type owl:NamedIndividual ,
                  :EmotionState ;
         rdfs:comment "Intense sadness or suffering." .


###  http://www.semanticweb.org/ghiot/ontologies/2023/11/meaw/annoyance
:annoyance rdf:type owl:NamedIndividual ,
                    :EmotionState ;
           rdfs:comment "Very mild anger caused by a nuisance or inconvenience." .


###  http://www.semanticweb.org/ghiot/ontologies/2023/11/meaw/anonymous
:anonymous rdf:type owl:NamedIndividual ,
                    :Person ;
           :hasGender :female ;
           :hasRoleInConversation <http://www.semanticweb.org/ghiot/ontologies/2023/11/meaw#2101608040029452931_studio_audience> ;
           :isSpeakerIn <http://www.semanticweb.org/ghiot/ontologies/2023/11/meaw#41_sadness> ;
           :hasSupposedAge "50"^^xsd:int .


###  http://www.semanticweb.org/ghiot/ontologies/2023/11/meaw/anonymous1
:anonymous1 rdf:type owl:NamedIndividual ,
                     :Person ;
            :hasGender :male ;
            :hasRoleInConversation <http://www.semanticweb.org/ghiot/ontologies/2023/11/meaw#2101608040029452931_studio_audience> ;
            :isAddressedIn <http://www.semanticweb.org/ghiot/ontologies/2023/11/meaw#58_anger> ;
            :isSpeakerIn <http://www.semanticweb.org/ghiot/ontologies/2023/11/meaw#57_disgust> ;
            :hasSupposedAge "60"^^xsd:int .


###  http://www.semanticweb.org/ghiot/ontologies/2023/11/meaw/anxiety
:anxiety rdf:type owl:NamedIndividual ,
                  :EmotionState ;
         rdfs:comment "Fear of an anticipated or actual threat and uncertainty about one's ability to cope with it." .


###  http://www.semanticweb.org/ghiot/ontologies/2023/11/meaw/argumentativeness
:argumentativeness rdf:type owl:NamedIndividual ,
                            :EmotionState ;
                   rdfs:comment "A tendency to engage in disagreements." .


###  http://www.semanticweb.org/ghiot/ontologies/2023/11/meaw/argumenting_with_facts
:argumenting_with_facts rdf:type owl:NamedIndividual ,
                                 :ConversationalFrame ;
                        rdfs:comment "A Conversational Frames where the speaker expresses objective facts or reports on events to support the validity of their perspective on the topic of conversation." .


###  http://www.semanticweb.org/ghiot/ontologies/2023/11/meaw/argumenting_with_personal_experience
:argumenting_with_personal_experience rdf:type owl:NamedIndividual ,
                                               :ConversationalFrame ;
                                      rdfs:comment "A Conversational Frame where the speaker recalls a personal experience or another type of subjective argument to support the validity of their perspective on the topic of conversation." .


###  http://www.semanticweb.org/ghiot/ontologies/2023/11/meaw/asking_for_argumentation
:asking_for_argumentation rdf:type owl:NamedIndividual ,
                                   :ConversationalFrame ;
                          rdfs:comment "A Conversational Frame where a person participating to the talk show expressly asks another person to argument and furtherly explain their perspective on the topic." .


###  http://www.semanticweb.org/ghiot/ontologies/2023/11/meaw/aversion
:aversion rdf:type owl:NamedIndividual ,
                   :EmotionState ;
          rdfs:comment "An impulse to avoid something disgusting." .


###  http://www.semanticweb.org/ghiot/ontologies/2023/11/meaw/bitterness
:bitterness rdf:type owl:NamedIndividual ,
                     :EmotionState ;
            rdfs:comment "Anger after unfair treatment." .


###  http://www.semanticweb.org/ghiot/ontologies/2023/11/meaw/clarifying_concept
:clarifying_concept rdf:type owl:NamedIndividual ,
                             :ConversationalFrame ;
                    rdfs:comment "A Conversational Frame where the speaker is not expressing their own perspective but clarifying a concept, adding information, or explaining unknown terms to make them clear for everyone taking part in the conversation." .


###  http://www.semanticweb.org/ghiot/ontologies/2023/11/meaw/compassion
:compassion rdf:type owl:NamedIndividual ,
                     :EmotionState ;
            rdfs:comment "Enjoyment of helping to relieve another person's suffering." .


###  http://www.semanticweb.org/ghiot/ontologies/2023/11/meaw/despair
:despair rdf:type owl:NamedIndividual ,
                  :EmotionState ;
         rdfs:comment "The loss of hope that a bad situation will improve or change." .


###  http://www.semanticweb.org/ghiot/ontologies/2023/11/meaw/desperation
:desperation rdf:type owl:NamedIndividual ,
                      :EmotionState ;
             rdfs:comment "A response to the inability to reduce danger." .


###  http://www.semanticweb.org/ghiot/ontologies/2023/11/meaw/disagreeing_by_interrupting
:disagreeing_by_interrupting rdf:type owl:NamedIndividual ,
                                      :ConversationalFrame ;
                             rdfs:comment "A conversational frame where a speaker interrupts another speaker without the host mediating the change, to disagree or contradict the previous speaker." .


###  http://www.semanticweb.org/ghiot/ontologies/2023/11/meaw/disagreeing_with_facts
:disagreeing_with_facts rdf:type owl:NamedIndividual ,
                                 :ConversationalFrame ;
                        rdfs:comment "A Conversational Frame where a speaker is given speaking space by the host, and they outline facts or events related to the topic that have the goal of proving other speaker’s arguments wrong." .


###  http://www.semanticweb.org/ghiot/ontologies/2023/11/meaw/disagreeing_with_opinion
:disagreeing_with_opinion rdf:type owl:NamedIndividual ,
                                   :ConversationalFrame ;
                          rdfs:comment "A Conversational Frame where a speaker is given speaking space by the host, and they express a perspective on the topic that disagrees with the one of the previous speaker." .


###  http://www.semanticweb.org/ghiot/ontologies/2023/11/meaw/disappointment
:disappointment rdf:type owl:NamedIndividual ,
                         :EmotionState ;
                rdfs:comment "A feeling that expectations are not being met." .


###  http://www.semanticweb.org/ghiot/ontologies/2023/11/meaw/discouragement
:discouragement rdf:type owl:NamedIndividual ,
                         :EmotionState ;
                rdfs:comment "A response to repeated failures to accomplish something: the belief that it can't be done." .


###  http://www.semanticweb.org/ghiot/ontologies/2023/11/meaw/disgust
:disgust rdf:type owl:NamedIndividual ,
                  :BasicEmotion ;
         :includes :abhorrence ,
                   :aversion ,
                   :dislike ,
                   :distaste ,
                   :loathing ,
                   :repugnance ,
                   :revulsion ;
         rdfs:comment "Feeling disgusted by what is toxic helps us to avoid being poisoned, physically or socially (description from http://atlasofemotions.org/)." .


###  http://www.semanticweb.org/ghiot/ontologies/2023/11/meaw/dislike
:dislike rdf:type owl:NamedIndividual ,
                  :EmotionState ;
         rdfs:comment "A preference against something." .


###  http://www.semanticweb.org/ghiot/ontologies/2023/11/meaw/distaste
:distaste rdf:type owl:NamedIndividual ,
                   :EmotionState ;
          rdfs:comment "Reaction to a bad taste, smell, thing or idea. Can be literal or metaphorical." .


###  http://www.semanticweb.org/ghiot/ontologies/2023/11/meaw/distraughtness
:distraughtness rdf:type owl:NamedIndividual ,
                         :EmotionState ;
                rdfs:comment "Sadness that makes it hard to think clearly." .


###  http://www.semanticweb.org/ghiot/ontologies/2023/11/meaw/dread
:dread rdf:type owl:NamedIndividual ,
                :EmotionState ;
       rdfs:comment "Anticipation of severe danger." .


###  http://www.semanticweb.org/ghiot/ontologies/2023/11/meaw/ecstasy
:ecstasy rdf:type owl:NamedIndividual ,
                  :EmotionState ;
         rdfs:comment "Rapturous delight. A state of very great happiness, nearly overwhelming." .


###  http://www.semanticweb.org/ghiot/ontologies/2023/11/meaw/enjoyment
:enjoyment rdf:type owl:NamedIndividual ,
                    :BasicEmotion ;
           :includes :amusement ,
                     :compassion ,
                     :ecstasy ,
                     :fiero ,
                     :naches ,
                     :peace ,
                     :pride ,
                     :rejoicing ,
                     :relief ,
                     :schadenfreude ,
                     :sensory_pleasure ,
                     :wonder ;
           rdfs:comment "We feel enjoyment when we experience novelty or comfort. Enjoyment varies in strength and frequency in our lives (description from http://atlasofemotions.org/)." .


###  http://www.semanticweb.org/ghiot/ontologies/2023/11/meaw/exasperation
:exasperation rdf:type owl:NamedIndividual ,
                       :EmotionState ;
              rdfs:comment "Anger caused by a repeated or strong nuisance." .


###  http://www.semanticweb.org/ghiot/ontologies/2023/11/meaw/excitement
:excitement rdf:type owl:NamedIndividual ,
                     :EmotionState ;
            rdfs:comment "A powerful enthusiasm." .


###  http://www.semanticweb.org/ghiot/ontologies/2023/11/meaw/fear
:fear rdf:type owl:NamedIndividual ,
               :BasicEmotion ;
      :includes :anxiety ,
                :desperation ,
                :dread ,
                :horror ,
                :nervousness ,
                :panic ,
                :terror ,
                :trepidation ;
      rdfs:comment "Our fear of danger lets us anticipate threats to our safety (description from http://atlasofemotions.org/)." .


###  http://www.semanticweb.org/ghiot/ontologies/2023/11/meaw/female
:female rdf:type owl:NamedIndividual ,
                 :Gender .


###  http://www.semanticweb.org/ghiot/ontologies/2023/11/meaw/fiero
:fiero rdf:type owl:NamedIndividual ,
                :EmotionState ;
       rdfs:comment "Enjoyment of meeting a difficult challenge (an Italian word)." .


###  http://www.semanticweb.org/ghiot/ontologies/2023/11/meaw/frustration
:frustration rdf:type owl:NamedIndividual ,
                      :EmotionState ;
             rdfs:comment "A response to repeated failures to overcome an obstacle." .


###  http://www.semanticweb.org/ghiot/ontologies/2023/11/meaw/fury
:fury rdf:type owl:NamedIndividual ,
               :EmotionState ;
      rdfs:comment "Uncontrolled and often violent anger." .


###  http://www.semanticweb.org/ghiot/ontologies/2023/11/meaw/giving_talking_space
:giving_talking_space rdf:type owl:NamedIndividual ,
                               :ConversationalFrame ;
                      rdfs:comment "A conversational frame where the host intervenes to change the speaker, mediating from what the last speaker said to what another speaker has to say." .


###  http://www.semanticweb.org/ghiot/ontologies/2023/11/meaw/giving_talking_space_with_question
:giving_talking_space_with_question rdf:type owl:NamedIndividual ,
                                             :ConversationalFrame ;
                                    rdfs:comment "A conversational frame where the host intervenes to change the speaker, mediating from what the last speaker said to what another speaker has to say, by directly asking them a question such as “what do you think about this?”." .


###  http://www.semanticweb.org/ghiot/ontologies/2023/11/meaw/grief
:grief rdf:type owl:NamedIndividual ,
                :EmotionState ;
       rdfs:comment "Sadness over a deep loss." .


###  http://www.semanticweb.org/ghiot/ontologies/2023/11/meaw/guest
:guest rdf:type owl:NamedIndividual ,
                :Role .


###  http://www.semanticweb.org/ghiot/ontologies/2023/11/meaw/helplessness
:helplessness rdf:type owl:NamedIndividual ,
                       :EmotionState ;
              rdfs:comment "The realization that one cannot make a situation better or easier." .


###  http://www.semanticweb.org/ghiot/ontologies/2023/11/meaw/hopelessness
:hopelessness rdf:type owl:NamedIndividual ,
                       :EmotionState ;
              rdfs:comment "The belief that nothing good will happen." .


###  http://www.semanticweb.org/ghiot/ontologies/2023/11/meaw/horror
:horror rdf:type owl:NamedIndividual ,
                 :EmotionState ;
        rdfs:comment "A mixture of fear, disgust, and shock." .


###  http://www.semanticweb.org/ghiot/ontologies/2023/11/meaw/host
:host rdf:type owl:NamedIndividual ,
               :Role .


###  http://www.semanticweb.org/ghiot/ontologies/2023/11/meaw/introducing_topic
:introducing_topic rdf:type owl:NamedIndividual ,
                            :ConversationalFrame ;
                   rdfs:comment "A conversational frame where the hosts introduce a topic of conversation, usually giving some information about the why is something worth discussing, the context of the topic and identifying some divisive or problematic aspect of the issue that participants in the talk show must share their perspective on. It is usually the frame that begins the talk show or a talk show section or it can be a frame present in the middle of the conversation to shift the topic of the discussion." .


###  http://www.semanticweb.org/ghiot/ontologies/2023/11/meaw/legien_kromkamp
:legien_kromkamp rdf:type owl:NamedIndividual ,
                          :NamedPerson ;
                 :hasGender :female ;
                 :hasRoleInConversation <http://www.semanticweb.org/ghiot/ontologies/2023/11/meaw#2101608040029452931_host> ;
                 :isSpeakerIn <http://www.semanticweb.org/ghiot/ontologies/2023/11/meaw#40_neutrality> ,
                              <http://www.semanticweb.org/ghiot/ontologies/2023/11/meaw#45_neutrality> ,
                              <http://www.semanticweb.org/ghiot/ontologies/2023/11/meaw#46_fear> ;
                 :hasNameSource "annotator" ;
                 :hasSupposedAge "40"^^xsd:int .


###  http://www.semanticweb.org/ghiot/ontologies/2023/11/meaw/loathing
:loathing rdf:type owl:NamedIndividual ,
                   :EmotionState ;
          rdfs:comment "Intense disgust focused on a person. Intense disgust focused on oneself is called self-loathing." .


###  http://www.semanticweb.org/ghiot/ontologies/2023/11/meaw/male
:male rdf:type owl:NamedIndividual ,
               :Gender .


###  http://www.semanticweb.org/ghiot/ontologies/2023/11/meaw/misery
:misery rdf:type owl:NamedIndividual ,
                 :EmotionState ;
        rdfs:comment "Strong suffering or unhappiness." .


###  http://www.semanticweb.org/ghiot/ontologies/2023/11/meaw/naches
:naches rdf:type owl:NamedIndividual ,
                 :EmotionState ;
        rdfs:comment "Joyful pride in the accomplishments of one's children or mentees (a Yiddish word)." .


###  http://www.semanticweb.org/ghiot/ontologies/2023/11/meaw/ncrv
:ncrv rdf:type owl:NamedIndividual ,
               :Broadcaster ;
      :broadcastedBy :ncrv .


###  http://www.semanticweb.org/ghiot/ontologies/2023/11/meaw/nervousness
:nervousness rdf:type owl:NamedIndividual ,
                      :EmotionState ;
             rdfs:comment "Uncertainty as to whether there is a danger." .


###  http://www.semanticweb.org/ghiot/ontologies/2023/11/meaw/neutrality
:neutrality rdf:type owl:NamedIndividual ,
                     :BasicEmotion ;
            :hasEnd "" ;
            :hasStart "394" ;
            rdfs:comment "No emotion is present." .


###  http://www.semanticweb.org/ghiot/ontologies/2023/11/meaw/panic
:panic rdf:type owl:NamedIndividual ,
                :EmotionState ;
       rdfs:comment "Sudden uncontrollable fear." .


###  http://www.semanticweb.org/ghiot/ontologies/2023/11/meaw/peace
:peace rdf:type owl:NamedIndividual ,
                :EmotionState ;
       rdfs:comment "An experience of ease and contentment." .


###  http://www.semanticweb.org/ghiot/ontologies/2023/11/meaw/presenting_opinion
:presenting_opinion rdf:type owl:NamedIndividual ,
                             :ConversationalFrame ;
                    rdfs:comment "A Conversational Frame where a speaker expresses their opinion on a topic, without necessarily disagreeing with other speakers, but in a neutral way." .


###  http://www.semanticweb.org/ghiot/ontologies/2023/11/meaw/pride
:pride rdf:type owl:NamedIndividual ,
                :EmotionState ;
       rdfs:comment "Deep pleasure and satisfaction derived from one's own achievements or the achievements of an associate." .


###  http://www.semanticweb.org/ghiot/ontologies/2023/11/meaw/rejoicing
:rejoicing rdf:type owl:NamedIndividual ,
                    :EmotionState ;
           rdfs:comment "A warm, uplifting feeling that people experience when they see acts of human goodness, kindness and compassion. Also called elevation." .


###  http://www.semanticweb.org/ghiot/ontologies/2023/11/meaw/relief
:relief rdf:type owl:NamedIndividual ,
                 :EmotionState ;
        rdfs:comment "When something expected to be unpleasant, especially the threat of harm, is avoided or comes to an end." .


###  http://www.semanticweb.org/ghiot/ontologies/2023/11/meaw/repugnance
:repugnance rdf:type owl:NamedIndividual ,
                     :EmotionState ;
            rdfs:comment "Strong distaste for something, often a concept or idea." .


###  http://www.semanticweb.org/ghiot/ontologies/2023/11/meaw/resignation
:resignation rdf:type owl:NamedIndividual ,
                      :EmotionState ;
             rdfs:comment "The belief that nothing can be done." .


###  http://www.semanticweb.org/ghiot/ontologies/2023/11/meaw/revulsion
:revulsion rdf:type owl:NamedIndividual ,
                    :EmotionState ;
           rdfs:comment "A mixture of disgust and loathing." .


###  http://www.semanticweb.org/ghiot/ontologies/2023/11/meaw/sadness
:sadness rdf:type owl:NamedIndividual ,
                  :BasicEmotion ;
         :includes :anguish ,
                   :despair ,
                   :disappointment ,
                   :discouragement ,
                   :distraughtness ,
                   :grief ,
                   :helplessness ,
                   :misery ,
                   :resignation ,
                   :sorrow ;
         rdfs:comment "Sadness is a response to loss, and feeling sad allows us to take a timeout and show others that we need support (description from http://atlasofemotions.org/)." .


###  http://www.semanticweb.org/ghiot/ontologies/2023/11/meaw/saying_something_wrong
:saying_something_wrong rdf:type owl:NamedIndividual ,
                                 :ConversationalFrame .


###  http://www.semanticweb.org/ghiot/ontologies/2023/11/meaw/schadenfreude
:schadenfreude rdf:type owl:NamedIndividual ,
                        :EmotionState ;
               rdfs:comment "Enjoyment of the misfortunes of another person, usually a rival." .


###  http://www.semanticweb.org/ghiot/ontologies/2023/11/meaw/sensory_pleasure
:sensory_pleasure rdf:type owl:NamedIndividual ,
                           :EmotionState ;
                  rdfs:comment "Enjoyment derived through one of the five physical senses: sight, sound, touch, taste and smell." .


###  http://www.semanticweb.org/ghiot/ontologies/2023/11/meaw/sorrow
:sorrow rdf:type owl:NamedIndividual ,
                 :EmotionState ;
        rdfs:comment "A feeling of distress and sadness, often caused by a loss." .


###  http://www.semanticweb.org/ghiot/ontologies/2023/11/meaw/studio_audience
:studio_audience rdf:type owl:NamedIndividual ,
                          :Group ,
                          :Role ;
                 rdfs:comment "Represents all the people sitting in the studio during the talk show, as a characteristic of the talk show genre, they usually are ordinary people that can intervene alongside invited guests. The studio audience can have collective reactions to the discourse taking place, such as clapping, cheereing, booing and so on. It might happen that an utterance has no individual speaker but shows in fact, a chaotic collective display of emotion by the studio audience. In these cases, the studio audience is considered as the speaker of the utterance." .


###  http://www.semanticweb.org/ghiot/ontologies/2023/11/meaw/surprise
:surprise rdf:type owl:NamedIndividual ,
                   :BasicEmotion .


###  http://www.semanticweb.org/ghiot/ontologies/2023/11/meaw/terror
:terror rdf:type owl:NamedIndividual ,
                 :EmotionState ;
        rdfs:comment "Intense, overpowering fear." .


###  http://www.semanticweb.org/ghiot/ontologies/2023/11/meaw/trepidation
:trepidation rdf:type owl:NamedIndividual ,
                      :EmotionState ;
             rdfs:comment "Anticipation of the possibility of danger." .


###  http://www.semanticweb.org/ghiot/ontologies/2023/11/meaw/unknown
:unknown rdf:type owl:NamedIndividual ,
                  :Gender .


###  http://www.semanticweb.org/ghiot/ontologies/2023/11/meaw/vengefulness
:vengefulness rdf:type owl:NamedIndividual ,
                       :EmotionState ;
              rdfs:comment "Desire to retaliate after one is hurt." .


###  http://www.semanticweb.org/ghiot/ontologies/2023/11/meaw/welles_nietes
:welles_nietes rdf:type owl:NamedIndividual ,
                        :TalkShowSituation ;
               :broadcastedBy :ncrv ;
               :hasInScope <http://www.semanticweb.org/ghiot/ontologies/2023/11/meaw#40_neutrality> ,
                           <http://www.semanticweb.org/ghiot/ontologies/2023/11/meaw#41_sadness> ,
                           <http://www.semanticweb.org/ghiot/ontologies/2023/11/meaw#45_neutrality> ,
                           <http://www.semanticweb.org/ghiot/ontologies/2023/11/meaw#46_fear> ,
                           <http://www.semanticweb.org/ghiot/ontologies/2023/11/meaw#57_disgust> ,
                           <http://www.semanticweb.org/ghiot/ontologies/2023/11/meaw#58_anger> ;
               :hasDate "1988-03-19" ;
               :hasDescription "Discussie over de stelling: 'Mag je op televisie zeggen wat je denkt?'. Discussiedeelnemers: voor- en tegenstanders in het publiek, onder wie Adelheid Roosen, Paul de Leeuw, mr. A. Duijser, algemeen directeur NCRV en vijf panelleden. De discussie wordt geleid door Legien Kromkamp." ,
                               "Laatste 'Welles nietes' van het seizoen. Dit keer gaat het om gekwetst worden door iets op de televisie. Actrice Adelheid Roosen, bekend van 'De nacht', en acteur Paul de Leeuw bevinden zich te midden van een merendeels conservatief publiek. Confrontaties kunnen niet uitblijven. Adelheid Roosen vat de discussie sportief op. Ze biedt haar opponenten een waterpistool aan waarmee ze haar mogen natspuiten. Een vrouw gaat in op dit aanbod." ,
                               "Pittige maatschappelijke discussies onder leiding van Legien Kromkamp over een bepaalde stelling. Voor- en tegenstanders zetten hun argumenten uiteen en proberen zo de mening van de vijf vaste panelleden te beïnvloeden. Allerlei vraagstukken komen aan bod. Van drugsproblematiek, armoede of voetbalgeweld tot het milieu en amusement op televisie. Aan het einde van de aflevering wordt de stelling voor de volgende uitzending bekendgemaakt. Kijkers kunnen hierop reageren en enkelen worden uitgenodigd om in de studio deel te nemen aan de discussie. Het programma is te zien geweest van 1985 tot en met 1990. Felle reacties De NCRV krijgt veel brieven op de uitzendingen. Sommige onderwerpen roepen tegengestelde reacties op bij de achterban. Maar ook het taalgebruik leidt tot een stroom aan reacties. In een discussie wordt nogal eens gevloekt of grove taal geuit, voor menig kijker reden genoeg om in de pen te klimmen." ,
                               "Tweewekelijks praatprogramma waarin gediscussieerd wordt over een stelling, waarna de panelleden zich voor of tegen de stelling uitspreken." ;
               :hasFileTitle "WELLESNIETES_-HRE0000551A" ;
               :hasIdentifier "2101608040029452931" ;
               :hasTitle "WELLES NIETES - WELLES NIETES;Mag je op televisie zeggen wat je denkt?" ;
               :isAbout "televisie, vrijheid van meningsuiting" .


###  http://www.semanticweb.org/ghiot/ontologies/2023/11/meaw/wonder
:wonder rdf:type owl:NamedIndividual ,
                 :EmotionState ;
        rdfs:comment "An experience of something that is very surprising, beautiful, amazing or hard to believe." .


###  Generated by the OWL API (version 4.5.26.2023-07-17T20:34:13Z) https://github.com/owlcs/owlapi
