@prefix : <https://raw.githubusercontent.com/MaddaGh/DataProcessing_EmoAnnotation/main/meaw.ttl#> .
@prefix owl: <http://www.w3.org/2002/07/owl#> .
@prefix rdf: <http://www.w3.org/1999/02/22-rdf-syntax-ns#> .
@prefix xml: <http://www.w3.org/XML/1998/namespace> .
@prefix xsd: <http://www.w3.org/2001/XMLSchema#> .
@prefix rdfs: <http://www.w3.org/2000/01/rdf-schema#> .
@base <https://raw.githubusercontent.com/MaddaGh/DataProcessing_EmoAnnotation/main/meaw.ttl> .

<https://raw.githubusercontent.com/MaddaGh/DataProcessing_EmoAnnotation/main/meaw.ttl> rdf:type owl:Ontology ;
                                                                                        rdfs:comment "First modelet of the Multimodal Emotio Annotation Ontology. Developed within my thesis research in collaboration with the netherlands Institute for Sound and Vision." .

#################################################################
#    Annotation properties
#################################################################

###  http://swrl.stanford.edu/ontologies/3.3/swrla.owl#isRuleEnabled
<http://swrl.stanford.edu/ontologies/3.3/swrla.owl#isRuleEnabled> rdf:type owl:AnnotationProperty .


#################################################################
#    Object Properties
#################################################################

###  https://raw.githubusercontent.com/MaddaGh/DataProcessing_EmoAnnotation/main/meaw.ttl#broadcastedBy
:broadcastedBy rdf:type owl:ObjectProperty ;
               rdfs:domain :TalkShow ;
               rdfs:range :Broadcaster .


###  https://raw.githubusercontent.com/MaddaGh/DataProcessing_EmoAnnotation/main/meaw.ttl#emotion
:emotion rdf:type owl:ObjectProperty ;
         owl:inverseOf :expressedIn ;
         rdfs:domain :EmotionAnnotation ;
         rdfs:range :Emotion .


###  https://raw.githubusercontent.com/MaddaGh/DataProcessing_EmoAnnotation/main/meaw.ttl#experiencer
:experiencer rdf:type owl:ObjectProperty ;
             owl:inverseOf :isExperiencerIn ;
             rdfs:domain :EmotionAnnotation ;
             rdfs:range :Agent .


###  https://raw.githubusercontent.com/MaddaGh/DataProcessing_EmoAnnotation/main/meaw.ttl#expressedIn
:expressedIn rdf:type owl:ObjectProperty ;
             rdfs:domain :Emotion ;
             rdfs:range :EmotionAnnotation .


###  https://raw.githubusercontent.com/MaddaGh/DataProcessing_EmoAnnotation/main/meaw.ttl#follows
:follows rdf:type owl:ObjectProperty ;
         owl:inverseOf :precedes ;
         rdfs:domain :Frame ;
         rdfs:range :Frame .


###  https://raw.githubusercontent.com/MaddaGh/DataProcessing_EmoAnnotation/main/meaw.ttl#framedBy
:framedBy rdf:type owl:ObjectProperty ;
          owl:inverseOf :frames ;
          rdfs:domain :EmotionAnnotation ;
          rdfs:range :Frame .


###  https://raw.githubusercontent.com/MaddaGh/DataProcessing_EmoAnnotation/main/meaw.ttl#frames
:frames rdf:type owl:ObjectProperty ;
        rdfs:domain :Frame ;
        rdfs:range :EmotionAnnotation .


###  https://raw.githubusercontent.com/MaddaGh/DataProcessing_EmoAnnotation/main/meaw.ttl#hasAngle
:hasAngle rdf:type owl:ObjectProperty ;
          rdfs:subPropertyOf :hasFramingTechnique ;
          rdfs:domain :Frame ;
          rdfs:range :CameraAngle .


###  https://raw.githubusercontent.com/MaddaGh/DataProcessing_EmoAnnotation/main/meaw.ttl#hasAuralComposition
:hasAuralComposition rdf:type owl:ObjectProperty ;
                     rdfs:domain :Frame ;
                     rdfs:range :AuralComposition .


###  https://raw.githubusercontent.com/MaddaGh/DataProcessing_EmoAnnotation/main/meaw.ttl#hasAuralTrigger
:hasAuralTrigger rdf:type owl:ObjectProperty ;
                 rdfs:subPropertyOf :hasTrigger ,
                                    [ owl:inverseOf :triggers
                                    ] ;
                 rdfs:domain :EmotionAnnotation ;
                 rdfs:range :AuralTrigger .


###  https://raw.githubusercontent.com/MaddaGh/DataProcessing_EmoAnnotation/main/meaw.ttl#hasCameraFramingInterpretation
:hasCameraFramingInterpretation rdf:type owl:ObjectProperty ;
                                owl:inverseOf :isframingInterpretationOf ;
                                rdfs:domain :EmotionAnnotation ;
                                rdfs:range :CameraFramingInterpretation .


###  https://raw.githubusercontent.com/MaddaGh/DataProcessing_EmoAnnotation/main/meaw.ttl#hasConversationalContext
:hasConversationalContext rdf:type owl:ObjectProperty ;
                          rdfs:domain :ConversationalRolePlay ;
                          rdfs:range :TalkShow .


###  https://raw.githubusercontent.com/MaddaGh/DataProcessing_EmoAnnotation/main/meaw.ttl#hasConversationalRolePlay
:hasConversationalRolePlay rdf:type owl:ObjectProperty ;
                           owl:inverseOf :isRolePlayOf ;
                           rdfs:domain :Agent ;
                           rdfs:range :ConversationalRolePlay .


###  https://raw.githubusercontent.com/MaddaGh/DataProcessing_EmoAnnotation/main/meaw.ttl#hasFrameContext
:hasFrameContext rdf:type owl:ObjectProperty ;
                 rdfs:domain :EmotionAnnotation ;
                 rdfs:range :ConversationalFrame .


###  https://raw.githubusercontent.com/MaddaGh/DataProcessing_EmoAnnotation/main/meaw.ttl#hasFramingTechnique
:hasFramingTechnique rdf:type owl:ObjectProperty ;
                     rdfs:domain :Frame ;
                     rdfs:range :FramingTechnique .


###  https://raw.githubusercontent.com/MaddaGh/DataProcessing_EmoAnnotation/main/meaw.ttl#hasGender
:hasGender rdf:type owl:ObjectProperty ;
           rdfs:domain :Person ;
           rdfs:range :Gender .


###  https://raw.githubusercontent.com/MaddaGh/DataProcessing_EmoAnnotation/main/meaw.ttl#hasInScope
:hasInScope rdf:type owl:ObjectProperty ;
            owl:inverseOf :isInScopeOf ;
            rdfs:domain :TalkShow ;
            rdfs:range :EmotionAnnotation .


###  https://raw.githubusercontent.com/MaddaGh/DataProcessing_EmoAnnotation/main/meaw.ttl#hasMovement
:hasMovement rdf:type owl:ObjectProperty ;
             rdfs:subPropertyOf :hasFramingTechnique ;
             rdfs:domain :Frame ;
             rdfs:range :CameraMovement .


###  https://raw.githubusercontent.com/MaddaGh/DataProcessing_EmoAnnotation/main/meaw.ttl#hasRole
:hasRole rdf:type owl:ObjectProperty ;
         rdfs:domain :ConversationalRolePlay ;
         rdfs:range :Role .


###  https://raw.githubusercontent.com/MaddaGh/DataProcessing_EmoAnnotation/main/meaw.ttl#hasShotType
:hasShotType rdf:type owl:ObjectProperty ;
             rdfs:subPropertyOf :hasFramingTechnique ;
             rdfs:domain :Frame ;
             rdfs:range :ShotType .


###  https://raw.githubusercontent.com/MaddaGh/DataProcessing_EmoAnnotation/main/meaw.ttl#hasTrigger
:hasTrigger rdf:type owl:ObjectProperty ;
            owl:inverseOf :triggers ;
            rdfs:domain :EmotionAnnotation ;
            rdfs:range :Trigger .


###  https://raw.githubusercontent.com/MaddaGh/DataProcessing_EmoAnnotation/main/meaw.ttl#hasVerbalTrigger
:hasVerbalTrigger rdf:type owl:ObjectProperty ;
                  rdfs:subPropertyOf :hasTrigger ,
                                     [ owl:inverseOf :triggers
                                     ] ;
                  rdfs:domain :EmotionAnnotation ;
                  rdfs:range :VerbalTrigger .


###  https://raw.githubusercontent.com/MaddaGh/DataProcessing_EmoAnnotation/main/meaw.ttl#hasVisualTrigger
:hasVisualTrigger rdf:type owl:ObjectProperty ;
                  rdfs:subPropertyOf :hasTrigger ,
                                     [ owl:inverseOf :triggers
                                     ] ;
                  rdfs:domain :EmotionAnnotation ;
                  rdfs:range :VisualTrigger .


###  https://raw.githubusercontent.com/MaddaGh/DataProcessing_EmoAnnotation/main/meaw.ttl#includes
:includes rdf:type owl:ObjectProperty ;
          owl:inverseOf :isIncludedIn ;
          rdfs:domain :BasicEmotion ;
          rdfs:range :EmotionState .


###  https://raw.githubusercontent.com/MaddaGh/DataProcessing_EmoAnnotation/main/meaw.ttl#involves
:involves rdf:type owl:ObjectProperty ;
          owl:inverseOf :participatesIn .


###  https://raw.githubusercontent.com/MaddaGh/DataProcessing_EmoAnnotation/main/meaw.ttl#isExperiencerIn
:isExperiencerIn rdf:type owl:ObjectProperty ;
                 rdfs:domain :Agent ;
                 rdfs:range :EmotionAnnotation .


###  https://raw.githubusercontent.com/MaddaGh/DataProcessing_EmoAnnotation/main/meaw.ttl#isInScopeOf
:isInScopeOf rdf:type owl:ObjectProperty .


###  https://raw.githubusercontent.com/MaddaGh/DataProcessing_EmoAnnotation/main/meaw.ttl#isIncludedIn
:isIncludedIn rdf:type owl:ObjectProperty ;
              rdfs:domain :EmotionState ;
              rdfs:range :BasicEmotion .


###  https://raw.githubusercontent.com/MaddaGh/DataProcessing_EmoAnnotation/main/meaw.ttl#isRolePlayOf
:isRolePlayOf rdf:type owl:ObjectProperty .


###  https://raw.githubusercontent.com/MaddaGh/DataProcessing_EmoAnnotation/main/meaw.ttl#isShownIn
:isShownIn rdf:type owl:ObjectProperty ;
           owl:inverseOf :shows ;
           rdfs:domain :HumanVisualContent ;
           rdfs:range :Frame .


###  https://raw.githubusercontent.com/MaddaGh/DataProcessing_EmoAnnotation/main/meaw.ttl#isframingInterpretationOf
:isframingInterpretationOf rdf:type owl:ObjectProperty ;
                           rdfs:domain :CameraFramingInterpretation ;
                           rdfs:range :EmotionAnnotation .


###  https://raw.githubusercontent.com/MaddaGh/DataProcessing_EmoAnnotation/main/meaw.ttl#participatesIn
:participatesIn rdf:type owl:ObjectProperty ;
                owl:propertyChainAxiom ( :participatesIn
                                       ) .


###  https://raw.githubusercontent.com/MaddaGh/DataProcessing_EmoAnnotation/main/meaw.ttl#precedes
:precedes rdf:type owl:ObjectProperty ;
          rdfs:domain :Frame ;
          rdfs:range :Frame .


###  https://raw.githubusercontent.com/MaddaGh/DataProcessing_EmoAnnotation/main/meaw.ttl#shows
:shows rdf:type owl:ObjectProperty ;
       rdfs:domain :Frame ;
       rdfs:range :HumanVisualContent .


###  https://raw.githubusercontent.com/MaddaGh/DataProcessing_EmoAnnotation/main/meaw.ttl#showsExpression
:showsExpression rdf:type owl:ObjectProperty ;
                 rdfs:subPropertyOf :shows ,
                                    [ owl:inverseOf :isShownIn
                                    ] ;
                 rdfs:domain :Frame ;
                 rdfs:range :FacialMovement .


###  https://raw.githubusercontent.com/MaddaGh/DataProcessing_EmoAnnotation/main/meaw.ttl#showsEyes
:showsEyes rdf:type owl:ObjectProperty ;
           rdfs:subPropertyOf :shows ,
                              [ owl:inverseOf :isShownIn
                              ] ;
           rdfs:domain :Frame ;
           rdfs:range :EyeMovement .


###  https://raw.githubusercontent.com/MaddaGh/DataProcessing_EmoAnnotation/main/meaw.ttl#showsHandGesture
:showsHandGesture rdf:type owl:ObjectProperty ;
                  rdfs:subPropertyOf :shows ,
                                     [ owl:inverseOf :isShownIn
                                     ] ;
                  rdfs:domain :Frame ;
                  rdfs:range :Gesture ,
                             :HandGesture .


###  https://raw.githubusercontent.com/MaddaGh/DataProcessing_EmoAnnotation/main/meaw.ttl#showsHeadGesture
:showsHeadGesture rdf:type owl:ObjectProperty ;
                  rdfs:subPropertyOf :shows ,
                                     [ owl:inverseOf :isShownIn
                                     ] ;
                  rdfs:domain :Frame ;
                  rdfs:range :HeadGesture .


###  https://raw.githubusercontent.com/MaddaGh/DataProcessing_EmoAnnotation/main/meaw.ttl#showsMovement
:showsMovement rdf:type owl:ObjectProperty ;
               rdfs:subPropertyOf :shows ,
                                  [ owl:inverseOf :isShownIn
                                  ] ;
               rdfs:domain :Frame ;
               rdfs:range :Kinetic .


###  https://raw.githubusercontent.com/MaddaGh/DataProcessing_EmoAnnotation/main/meaw.ttl#triggers
:triggers rdf:type owl:ObjectProperty .


#################################################################
#    Data properties
#################################################################

###  https://raw.githubusercontent.com/MaddaGh/DataProcessing_EmoAnnotation/main/meaw.ttl#hasDate
:hasDate rdf:type owl:DatatypeProperty ,
                  owl:FunctionalProperty ;
         rdfs:domain :TalkShow ;
         rdfs:range xsd:string .


###  https://raw.githubusercontent.com/MaddaGh/DataProcessing_EmoAnnotation/main/meaw.ttl#hasDescription
:hasDescription rdf:type owl:DatatypeProperty ;
                rdfs:domain :TalkShow ;
                rdfs:range xsd:string .


###  https://raw.githubusercontent.com/MaddaGh/DataProcessing_EmoAnnotation/main/meaw.ttl#hasEnd
:hasEnd rdf:type owl:DatatypeProperty ,
                 owl:FunctionalProperty ;
        rdfs:domain :EmotionAnnotation ;
        rdfs:range xsd:string .


###  https://raw.githubusercontent.com/MaddaGh/DataProcessing_EmoAnnotation/main/meaw.ttl#hasFileName
:hasFileName rdf:type owl:DatatypeProperty ,
                      owl:FunctionalProperty ;
             rdfs:domain :TalkShow ;
             rdfs:range xsd:string .


###  https://raw.githubusercontent.com/MaddaGh/DataProcessing_EmoAnnotation/main/meaw.ttl#hasIdentifier
:hasIdentifier rdf:type owl:DatatypeProperty ,
                        owl:FunctionalProperty ;
               rdfs:domain :TalkShow ;
               rdfs:range xsd:string .


###  https://raw.githubusercontent.com/MaddaGh/DataProcessing_EmoAnnotation/main/meaw.ttl#hasNameSource
:hasNameSource rdf:type owl:DatatypeProperty ;
               rdfs:domain :NamedPerson ;
               rdfs:range xsd:string ;
               rdfs:comment "The source where the name of the speaker comes from, either the audio of the video, the overlaid captions or the annotator’s recognition." .


###  https://raw.githubusercontent.com/MaddaGh/DataProcessing_EmoAnnotation/main/meaw.ttl#hasStart
:hasStart rdf:type owl:DatatypeProperty ,
                   owl:FunctionalProperty ;
          rdfs:domain :EmotionAnnotation ;
          rdfs:range xsd:string .


###  https://raw.githubusercontent.com/MaddaGh/DataProcessing_EmoAnnotation/main/meaw.ttl#hasText
:hasText rdf:type owl:DatatypeProperty ;
         rdfs:domain :EmotionAnnotation ;
         rdfs:range xsd:string ;
         rdfs:comment "the ASR transcript of the text of the utterance." .


###  https://raw.githubusercontent.com/MaddaGh/DataProcessing_EmoAnnotation/main/meaw.ttl#hasTimecode
:hasTimecode rdf:type owl:DatatypeProperty ;
             rdfs:domain :HumanVisualContent ;
             rdfs:range xsd:string .


###  https://raw.githubusercontent.com/MaddaGh/DataProcessing_EmoAnnotation/main/meaw.ttl#hasTitle
:hasTitle rdf:type owl:DatatypeProperty ;
          rdfs:domain :TalkShow ;
          rdfs:range xsd:string .


###  https://raw.githubusercontent.com/MaddaGh/DataProcessing_EmoAnnotation/main/meaw.ttl#isAbout
:isAbout rdf:type owl:DatatypeProperty ;
         rdfs:domain :TalkShow ;
         rdfs:range xsd:string .


#################################################################
#    Classes
#################################################################

###  https://raw.githubusercontent.com/MaddaGh/DataProcessing_EmoAnnotation/main/meaw.ttl#Agent
:Agent rdf:type owl:Class ;
       rdfs:comment """The Agent can be either a person, in the intuitive meaning of the term, or a group of people. At least an agent needs to be recognized as participating in a talk show and also to be the speaker in an Emotion Annotation for this one to exist. This is because, logically, an emotion expression exists only if it is expressed by an agent. 
Given the automatic subdivision into utterances of a video, which is based on ASR segmentation of speech, there might be more than one person talking in the same utterance and more people can express an emotion in the same utterance. Nonetheless, it is crucial to respect the unique connection between 1 agent expressing 1 emotion.   
The speaker can be named, either by the host or by overlaid captions. If the annotator recognizes someone who is unnamed, they can integrate the name of the person. In either case, the provenance of the name must be provided by mean of the data property hasNameSource.""" .


###  https://raw.githubusercontent.com/MaddaGh/DataProcessing_EmoAnnotation/main/meaw.ttl#AppraisedEmotionAnnotation
:AppraisedEmotionAnnotation rdf:type owl:Class ;
                            rdfs:subClassOf :EmotionAnnotation ,
                                            [ rdf:type owl:Restriction ;
                                              owl:onProperty :hasTrigger ;
                                              owl:allValuesFrom :VerbalTrigger
                                            ] ;
                            owl:disjointWith :ExperiencedEmotionAnnotation ;
                            rdfs:comment "An emotion that is not experienced personally by the speaker but is appraised in a third person. The speaker reports that somebody else’s experiences an emotion. It can only be triggered by a verbal trigger." .


###  https://raw.githubusercontent.com/MaddaGh/DataProcessing_EmoAnnotation/main/meaw.ttl#AuralComposition
:AuralComposition rdf:type owl:Class ;
                  rdfs:comment """Describes the way the audio composes with the video of the utterance. For example:
-The speaker is clearly framed and so the audio is aligned with what the viewer sees
-The speaker is framed but not clearly, as it is, for example, in the background of a long shot, or in positions where the viewer cannot clearly identify who’s speaking
-The audio is a voiceover and the video frames something else, such as the listener or the studio
-The audio is muddled, as two or more people are talking over each other. In this case regardless of who’s speaking, it is difficult to identify a unique relation between speaker and audio as well as understanding what people are saying.""" .


###  https://raw.githubusercontent.com/MaddaGh/DataProcessing_EmoAnnotation/main/meaw.ttl#AuralTrigger
:AuralTrigger rdf:type owl:Class ;
              rdfs:subClassOf :Trigger ;
              owl:disjointWith :VerbalTrigger ,
                               :VisualTrigger ;
              rdfs:comment "A trigger that is observed in the audio, some characteristics in the way a person speak that can hint at the person’s emotion (such as tense articulation, startling, a laughter etc)." .


###  https://raw.githubusercontent.com/MaddaGh/DataProcessing_EmoAnnotation/main/meaw.ttl#BasicEmotion
:BasicEmotion rdf:type owl:Class ;
              rdfs:subClassOf :Emotion ;
              owl:disjointWith :EmotionState ;
              rdfs:comment "An Ekman basic emotion: anger, disgust, enjoyment, fear, sadness, surprise. Defined in www.atlasofemotions.org." .


###  https://raw.githubusercontent.com/MaddaGh/DataProcessing_EmoAnnotation/main/meaw.ttl#Broadcaster
:Broadcaster rdf:type owl:Class ;
             rdfs:comment "The class representing the broadcaster that aired the talk show." .


###  https://raw.githubusercontent.com/MaddaGh/DataProcessing_EmoAnnotation/main/meaw.ttl#CameraAngle
:CameraAngle rdf:type owl:Class ;
             rdfs:subClassOf :FramingTechnique ;
             rdfs:comment "Camera angle in cinema refers to the specific position of the camera in relation to the subject, influencing the viewer's perspective and emotional engagement." .


###  https://raw.githubusercontent.com/MaddaGh/DataProcessing_EmoAnnotation/main/meaw.ttl#CameraFramingInterpretation
:CameraFramingInterpretation rdf:type owl:Class ;
                             rdfs:comment "It’s the perspective conveyed by the way the talk show is filmed (on the basis of Tan, 2009). This information is based on the assumptions that the syntax of the visual modality influences the perception and understanding of meanings and emotional aspects. A Visual framing is considered at an utterance level: each emotion relation is framed visually in a unique way." .


###  https://raw.githubusercontent.com/MaddaGh/DataProcessing_EmoAnnotation/main/meaw.ttl#CameraMovement
:CameraMovement rdf:type owl:Class ;
                rdfs:subClassOf :FramingTechnique ;
                rdfs:comment "The physical displacement of the camera during filming, contributing to the visual storytelling and emotional impact of a scene (ex. tilt, pan, zoom...)." .


###  https://raw.githubusercontent.com/MaddaGh/DataProcessing_EmoAnnotation/main/meaw.ttl#ConversationalFrame
:ConversationalFrame rdf:type owl:Class ;
                     rdfs:comment "Considering talk shows as a predefined setting where there are specific conversational conventions, roles and patterns (in other words, a “genre” as defined by van Leeuwen: “Genres link the text with a special context and regulate the adequate selection of semiotic means dependent on that context.” A conversational frame is the identified conversational block in which the emotion is expressed." .


###  https://raw.githubusercontent.com/MaddaGh/DataProcessing_EmoAnnotation/main/meaw.ttl#ConversationalRolePlay
:ConversationalRolePlay rdf:type owl:Class ;
                        rdfs:comment "The Class that connects a Role covered by a person to the Talk Show in which the person had that role. The naming convention for instances of this class is: id of the archival item + type of role, ex: 2101608040029452931_guest." .


###  https://raw.githubusercontent.com/MaddaGh/DataProcessing_EmoAnnotation/main/meaw.ttl#Emotion
:Emotion rdf:type owl:Class ;
         rdfs:comment "Represents the emotion identified and annotated in a multimodal utterance by an annotator. A taxonomy of emotions is given, where each of the five Ekman basic emotions include a variety of emotional states, as defined by http://atlasofemotions.org/" .


###  https://raw.githubusercontent.com/MaddaGh/DataProcessing_EmoAnnotation/main/meaw.ttl#EmotionAnnotation
:EmotionAnnotation rdf:type owl:Class ;
                   rdfs:subClassOf [ owl:intersectionOf ( [ rdf:type owl:Restriction ;
                                                            owl:onProperty :emotion ;
                                                            owl:minQualifiedCardinality "1"^^xsd:nonNegativeInteger ;
                                                            owl:onClass :BasicEmotion
                                                          ]
                                                          [ rdf:type owl:Restriction ;
                                                            owl:onProperty :emotion ;
                                                            owl:maxQualifiedCardinality "2"^^xsd:nonNegativeInteger ;
                                                            owl:onClass :EmotionState
                                                          ]
                                                        ) ;
                                     rdf:type owl:Class
                                   ] ,
                                   [ rdf:type owl:Restriction ;
                                     owl:onProperty :emotion ;
                                     owl:someValuesFrom :Emotion
                                   ] ,
                                   [ rdf:type owl:Restriction ;
                                     owl:onProperty :hasTrigger ;
                                     owl:someValuesFrom :Trigger
                                   ] ,
                                   [ rdf:type owl:Restriction ;
                                     owl:onProperty :framedBy ;
                                     owl:minQualifiedCardinality "1"^^xsd:nonNegativeInteger ;
                                     owl:onClass :Frame
                                   ] ,
                                   [ rdf:type owl:Restriction ;
                                     owl:onProperty :experiencer ;
                                     owl:qualifiedCardinality "1"^^xsd:nonNegativeInteger ;
                                     owl:onClass :Agent
                                   ] ,
                                   [ rdf:type owl:Restriction ;
                                     owl:onProperty :hasEnd ;
                                     owl:qualifiedCardinality "1"^^xsd:nonNegativeInteger ;
                                     owl:onDataRange xsd:string
                                   ] ,
                                   [ rdf:type owl:Restriction ;
                                     owl:onProperty :hasStart ;
                                     owl:qualifiedCardinality "1"^^xsd:nonNegativeInteger ;
                                     owl:onDataRange xsd:string
                                   ] ;
                   rdfs:comment """The n-ary relation class that represents the expression of an emotion in an utterance. It is time indexed, since the utterance is the smallest sub-clip of a talk show video, defined by start and end timecodes, where an emotion, expressed by three modalities (audio, video, and text in the form of Automatic Speech Recognition transcript), needs to be annotated. It is a subclass of dul:Situation and it is also defined by a unique identifier.
The naming convention for instances of this class is: id of the archival item + numeric reference to the talk show segment + sequence number. The mp4 files of the utterances are named in the same way, ex: 2101608050034534331_9_175.""" .


###  https://raw.githubusercontent.com/MaddaGh/DataProcessing_EmoAnnotation/main/meaw.ttl#EmotionState
:EmotionState rdf:type owl:Class ;
              rdfs:subClassOf :Emotion ;
              rdfs:comment """A fine-grained emotion that can be considered an emotional state belonging to one of Ekman's basic emotion, as defined in www.atlasofemotions.org 
They are organized according to intensity level.""" .


###  https://raw.githubusercontent.com/MaddaGh/DataProcessing_EmoAnnotation/main/meaw.ttl#ExperiencedEmotionAnnotation
:ExperiencedEmotionAnnotation rdf:type owl:Class ;
                              rdfs:subClassOf :EmotionAnnotation ;
                              rdfs:comment "An emotion that is experienced by the speaker personally." .


###  https://raw.githubusercontent.com/MaddaGh/DataProcessing_EmoAnnotation/main/meaw.ttl#EyeMovement
:EyeMovement rdf:type owl:Class ;
             rdfs:subClassOf :FacialMovement .


###  https://raw.githubusercontent.com/MaddaGh/DataProcessing_EmoAnnotation/main/meaw.ttl#FacialMovement
:FacialMovement rdf:type owl:Class ;
                rdfs:subClassOf :HumanVisualContent ;
                rdfs:comment "The facial expressions on the basis of Ekman and Friesen's Facial Action Coding System (FACS). This class encompasses a series of facial movements that one can interpret as emotional triggers. It is to be noted that, even though in Ekman and Friesen's study facial expressions are related to emotional expressions, in the present study, this univoque relation is overlooked, and facial movements are only collected as a vocabulary for annotation. When the annotator identifies an emotion they can freely indicate the facial movement they recognise as visual trigger of the emotion." .


###  https://raw.githubusercontent.com/MaddaGh/DataProcessing_EmoAnnotation/main/meaw.ttl#Frame
:Frame rdf:type owl:Class ;
       rdfs:comment "The single frame that films the utterance. The overall visual framing of an emotion relation is a sequence of frames." .


###  https://raw.githubusercontent.com/MaddaGh/DataProcessing_EmoAnnotation/main/meaw.ttl#FramingTechnique
:FramingTechnique rdf:type owl:Class ;
                  rdfs:comment "The technical “grammatical” aspects with which one can describe a frame. These are three main aspects taken from cinema theory: camera angle (the positioning of the camera with respect to the content that is filmed), camera movement and type of shot." .


###  https://raw.githubusercontent.com/MaddaGh/DataProcessing_EmoAnnotation/main/meaw.ttl#FutureEmotionAnnotation
:FutureEmotionAnnotation rdf:type owl:Class ;
                         rdfs:subClassOf :EmotionAnnotation ,
                                         [ rdf:type owl:Restriction ;
                                           owl:onProperty :hasTrigger ;
                                           owl:allValuesFrom :VerbalTrigger
                                         ] ;
                         owl:disjointWith :PastEmotionAnnotation ,
                                          :PresentEmotionAnnotation ;
                         rdfs:comment "An emotion expressed conditionally, as a state that will occur in the future. For instance: “if you do this, it will hurt me”. It can only be triggered by a verbal trigger." .


###  https://raw.githubusercontent.com/MaddaGh/DataProcessing_EmoAnnotation/main/meaw.ttl#Gender
:Gender rdf:type owl:Class ;
        rdfs:comment "The gender, as recognized by the annotator, of the agent who's speaking in the utterance and that expresses the emotion." .


###  https://raw.githubusercontent.com/MaddaGh/DataProcessing_EmoAnnotation/main/meaw.ttl#Gesture
:Gesture rdf:type owl:Class ;
         rdfs:subClassOf :HumanVisualContent ;
         rdfs:comment "Head and hand gestures. Vocabularies are taken respectively from FACS and https://www.indiabix.com/body-language/hand-to-face-gestures/, they can be expanded." .


###  https://raw.githubusercontent.com/MaddaGh/DataProcessing_EmoAnnotation/main/meaw.ttl#Group
:Group rdf:type owl:Class ;
       rdfs:subClassOf :Agent ;
       owl:disjointWith :NamedPerson ,
                        :Person ;
       rdfs:comment "A collective agent, to represent the studio audience or the agent in utterances where multiple speakers are talking over each other." .


###  https://raw.githubusercontent.com/MaddaGh/DataProcessing_EmoAnnotation/main/meaw.ttl#HandGesture
:HandGesture rdf:type owl:Class ;
             rdfs:subClassOf :Gesture .


###  https://raw.githubusercontent.com/MaddaGh/DataProcessing_EmoAnnotation/main/meaw.ttl#HeadGesture
:HeadGesture rdf:type owl:Class ;
             rdfs:subClassOf :Gesture .


###  https://raw.githubusercontent.com/MaddaGh/DataProcessing_EmoAnnotation/main/meaw.ttl#HumanVisualContent
:HumanVisualContent rdf:type owl:Class ;
                    rdfs:comment "The type of visual content related to human aspects, such as gestures, movements and facial expressions. These are the visual modality features that concur to convey emotional meanings. Therefore, individuals of this class may also be visual triggers. It answers the question \"who and what is shown in the video?\"." .


###  https://raw.githubusercontent.com/MaddaGh/DataProcessing_EmoAnnotation/main/meaw.ttl#Kinetic
:Kinetic rdf:type owl:Class ;
         rdfs:subClassOf :HumanVisualContent ;
         rdfs:comment "Kinetics represent whole body movements, such as standing up or walking or turning towards someone. No precise vocabulary is defined; hence they can be described by the annotator as preferred." .


###  https://raw.githubusercontent.com/MaddaGh/DataProcessing_EmoAnnotation/main/meaw.ttl#NamedPerson
:NamedPerson rdf:type owl:Class ;
             rdfs:subClassOf :Person ,
                             [ rdf:type owl:Restriction ;
                               owl:onProperty :hasNameSource ;
                               owl:someValuesFrom [ rdf:type rdfs:Datatype ;
                                                    owl:oneOf [ rdf:type rdf:List ;
                                                                rdf:first "annotator" ;
                                                                rdf:rest [ rdf:type rdf:List ;
                                                                           rdf:first "audio" ;
                                                                           rdf:rest [ rdf:type rdf:List ;
                                                                                      rdf:first "captions" ;
                                                                                      rdf:rest rdf:nil
                                                                                    ]
                                                                         ]
                                                              ]
                                                  ]
                             ] ;
             rdfs:comment "A person who is recognized and named." .


###  https://raw.githubusercontent.com/MaddaGh/DataProcessing_EmoAnnotation/main/meaw.ttl#PastEmotionAnnotation
:PastEmotionAnnotation rdf:type owl:Class ;
                       rdfs:subClassOf :EmotionAnnotation ,
                                       [ rdf:type owl:Restriction ;
                                         owl:onProperty :hasTrigger ;
                                         owl:allValuesFrom :VerbalTrigger
                                       ] ;
                       owl:disjointWith :PresentEmotionAnnotation ;
                       rdfs:comment "An emotion that is recalled from the past. For instance: “I was worried”. It can only be triggered by a verbal trigger." .


###  https://raw.githubusercontent.com/MaddaGh/DataProcessing_EmoAnnotation/main/meaw.ttl#Person
:Person rdf:type owl:Class ;
        rdfs:subClassOf :Agent ,
                        [ rdf:type owl:Restriction ;
                          owl:onProperty :hasConversationalRolePlay ;
                          owl:someValuesFrom :ConversationalRolePlay
                        ] ,
                        [ rdf:type owl:Restriction ;
                          owl:onProperty :hasGender ;
                          owl:someValuesFrom :Gender
                        ] ;
        rdfs:comment "An Agent that is a single person in the intuitive meaning of the term." .


###  https://raw.githubusercontent.com/MaddaGh/DataProcessing_EmoAnnotation/main/meaw.ttl#PresentEmotionAnnotation
:PresentEmotionAnnotation rdf:type owl:Class ;
                          rdfs:subClassOf :EmotionAnnotation ;
                          rdfs:comment "An emotion that occurs in the present, while the speaker pronounces the utterance." .


###  https://raw.githubusercontent.com/MaddaGh/DataProcessing_EmoAnnotation/main/meaw.ttl#Role
:Role rdf:type owl:Class ;
      rdfs:comment "Represents the roles that are identifyed in a Talk Show conversation as a semi-scripted television genre." .


###  https://raw.githubusercontent.com/MaddaGh/DataProcessing_EmoAnnotation/main/meaw.ttl#ShotType
:ShotType rdf:type owl:Class ;
          rdfs:subClassOf :FramingTechnique ;
          rdfs:comment "Refers to the framing and composition of an individual shot, influencing the visual storytelling and communication of emotions or information within a scene." .


###  https://raw.githubusercontent.com/MaddaGh/DataProcessing_EmoAnnotation/main/meaw.ttl#TalkShow
:TalkShow rdf:type owl:Class ;
          rdfs:subClassOf [ rdf:type owl:Restriction ;
                            owl:onProperty :broadcastedBy ;
                            owl:someValuesFrom :Broadcaster
                          ] ,
                          [ rdf:type owl:Restriction ;
                            owl:onProperty :hasInScope ;
                            owl:someValuesFrom :EmotionAnnotation
                          ] ,
                          [ rdf:type owl:Restriction ;
                            owl:onProperty :involves ;
                            owl:minQualifiedCardinality "2"^^xsd:nonNegativeInteger ;
                            owl:onClass :Person
                          ] ,
                          [ rdf:type owl:Restriction ;
                            owl:onProperty :hasDate ;
                            owl:qualifiedCardinality "1"^^xsd:nonNegativeInteger ;
                            owl:onDataRange xsd:string
                          ] ,
                          [ rdf:type owl:Restriction ;
                            owl:onProperty :hasFileName ;
                            owl:qualifiedCardinality "1"^^xsd:nonNegativeInteger ;
                            owl:onDataRange xsd:string
                          ] ,
                          [ rdf:type owl:Restriction ;
                            owl:onProperty :hasIdentifier ;
                            owl:qualifiedCardinality "1"^^xsd:nonNegativeInteger ;
                            owl:onDataRange xsd:string
                          ] ;
          rdfs:comment """The n-ary relation class to represent statements defining a talk show as a dul:Situation: a video of a talk show, or an extract from it, retrieved from Sound and Vision archive through the media suite. It is defined by a file title, a unique identifier, a date, a broadcaster name, a description (if present in the archive metadata) and a topic labelled by subject terms from the archive GTAA that identify the topic of the video. If the talk show situation is an extract from the whole video, these metadata refer to the whole video rather than to the subsection of it, for they are automatically retrieved from the item’s metadata provided by Sound and Vision.
The naming convention for instances of this class is: id of the archival item + numeric reference. The mp4 files of the talk shows are named in the same way, ex: 2101608050034534331_9.""" .


###  https://raw.githubusercontent.com/MaddaGh/DataProcessing_EmoAnnotation/main/meaw.ttl#Trigger
:Trigger rdf:type owl:Class ;
         rdfs:comment """A precisely identifiable part in one or more than one modality (text, audio, video) where the annotator can recognise the expression of the emotion. Ex: a frowning facial expression in the video; the text “I am hurt” in the text; a louder pitch and tense articulation in the audio. 
It should be noticed that:
1.	For an Emotion to be identified at least 1 trigger needs to be identified.
2.	Triggers have no emotional meaning on their own but assume one in the context of the utterance (ex. a smile can be a happy smile but also a smile of embarrassment or pride)""" .


###  https://raw.githubusercontent.com/MaddaGh/DataProcessing_EmoAnnotation/main/meaw.ttl#VerbalTrigger
:VerbalTrigger rdf:type owl:Class ;
               rdfs:subClassOf :Trigger ;
               owl:disjointWith :VisualTrigger ;
               rdfs:comment "A trigger that is observed in what is said, a word or a sentence." .


###  https://raw.githubusercontent.com/MaddaGh/DataProcessing_EmoAnnotation/main/meaw.ttl#VisualTrigger
:VisualTrigger rdf:type owl:Class ;
               rdfs:subClassOf :Trigger ;
               rdfs:comment "A trigger that is observed in the video." .


#################################################################
#    Individuals
#################################################################

###  https://raw.githubusercontent.com/MaddaGh/DataProcessing_EmoAnnotation/main/meaw.ttl#abhorrence
:abhorrence rdf:type owl:NamedIndividual ,
                     :Emotion ,
                     :EmotionState ;
            :isIncludedIn :disgust ;
            rdfs:comment "A mixture of intense disgust and hatred." .


###  https://raw.githubusercontent.com/MaddaGh/DataProcessing_EmoAnnotation/main/meaw.ttl#adelheid_roosen
:adelheid_roosen rdf:type owl:NamedIndividual ,
                          :Agent ,
                          :NamedPerson ,
                          :Person ;
                 :hasConversationalRolePlay <https://raw.githubusercontent.com/MaddaGh/DataProcessing_EmoAnnotation/main/meaw.ttl#2101608040029452931_guest> ;
                 :hasGender :female ;
                 :isExperiencerIn <https://raw.githubusercontent.com/MaddaGh/DataProcessing_EmoAnnotation/main/meaw.ttl#50_anger> ,
                                  <https://raw.githubusercontent.com/MaddaGh/DataProcessing_EmoAnnotation/main/meaw.ttl#51_anger> ,
                                  <https://raw.githubusercontent.com/MaddaGh/DataProcessing_EmoAnnotation/main/meaw.ttl#58_anger> ;
                 :hasNameSource "captions" .


###  https://raw.githubusercontent.com/MaddaGh/DataProcessing_EmoAnnotation/main/meaw.ttl#agreeing
:agreeing rdf:type owl:NamedIndividual ,
                   :ConversationalFrame ;
          rdfs:comment "A Conversational Frame where the speaker recalls a personal experience or another type of subjective argument to support the validity of their perspective on the topic of conversation." .


###  https://raw.githubusercontent.com/MaddaGh/DataProcessing_EmoAnnotation/main/meaw.ttl#aligned
:aligned rdf:type owl:NamedIndividual ,
                  :AuralComposition .


###  https://raw.githubusercontent.com/MaddaGh/DataProcessing_EmoAnnotation/main/meaw.ttl#amusement
:amusement rdf:type owl:NamedIndividual ,
                    :Emotion ,
                    :EmotionState ;
           :isIncludedIn :enjoyment ;
           rdfs:comment "Light, playful feelings of enjoyment and good humor." .


###  https://raw.githubusercontent.com/MaddaGh/DataProcessing_EmoAnnotation/main/meaw.ttl#anger
:anger rdf:type owl:NamedIndividual ,
                :BasicEmotion ,
                :Emotion ;
       :expressedIn <https://raw.githubusercontent.com/MaddaGh/DataProcessing_EmoAnnotation/main/meaw.ttl#58_anger> ;
       :includes :annoyance ,
                 :argumentativeness ,
                 :bitterness ,
                 :exasperation ,
                 :frustration ,
                 :fury ,
                 :vengefulness ;
       rdfs:comment "We feel anger when we are mentally or physically blocked. Anger varies in strength and frequency in our lives. (description from http://atlasofemotions.org/)" .


###  https://raw.githubusercontent.com/MaddaGh/DataProcessing_EmoAnnotation/main/meaw.ttl#anguish
:anguish rdf:type owl:NamedIndividual ,
                  :Emotion ,
                  :EmotionState ;
         :isIncludedIn :sadness ;
         rdfs:comment "Intense sadness or suffering." .


###  https://raw.githubusercontent.com/MaddaGh/DataProcessing_EmoAnnotation/main/meaw.ttl#annoyance
:annoyance rdf:type owl:NamedIndividual ,
                    :Emotion ,
                    :EmotionState ;
           :expressedIn <https://raw.githubusercontent.com/MaddaGh/DataProcessing_EmoAnnotation/main/meaw.ttl#43_anger> ;
           :isIncludedIn :anger ;
           rdfs:comment "Very mild anger caused by a nuisance or inconvenience." .


###  https://raw.githubusercontent.com/MaddaGh/DataProcessing_EmoAnnotation/main/meaw.ttl#anonymous
:anonymous rdf:type owl:NamedIndividual ,
                    :Agent ,
                    :Person ;
           :hasConversationalRolePlay <https://raw.githubusercontent.com/MaddaGh/DataProcessing_EmoAnnotation/main/meaw.ttl#2101608040029452931_studio_audience> ;
           :hasGender :female ;
           :isExperiencerIn <https://raw.githubusercontent.com/MaddaGh/DataProcessing_EmoAnnotation/main/meaw.ttl#41_sadness> ,
                            <https://raw.githubusercontent.com/MaddaGh/DataProcessing_EmoAnnotation/main/meaw.ttl#43_fear> .


###  https://raw.githubusercontent.com/MaddaGh/DataProcessing_EmoAnnotation/main/meaw.ttl#anonymous1
:anonymous1 rdf:type owl:NamedIndividual ,
                     :Agent ,
                     :Person ;
            :hasConversationalRolePlay <https://raw.githubusercontent.com/MaddaGh/DataProcessing_EmoAnnotation/main/meaw.ttl#2101608040029452931_studio_audience> ;
            :hasGender :male ;
            :isExperiencerIn <https://raw.githubusercontent.com/MaddaGh/DataProcessing_EmoAnnotation/main/meaw.ttl#57_disgust> .


###  https://raw.githubusercontent.com/MaddaGh/DataProcessing_EmoAnnotation/main/meaw.ttl#anxiety
:anxiety rdf:type owl:NamedIndividual ,
                  :Emotion ,
                  :EmotionState ;
         :isIncludedIn :fear ;
         rdfs:comment "Fear of an anticipated or actual threat and uncertainty about one's ability to cope with it." .


###  https://raw.githubusercontent.com/MaddaGh/DataProcessing_EmoAnnotation/main/meaw.ttl#argumentativeness
:argumentativeness rdf:type owl:NamedIndividual ,
                            :Emotion ,
                            :EmotionState ;
                   :expressedIn <https://raw.githubusercontent.com/MaddaGh/DataProcessing_EmoAnnotation/main/meaw.ttl#55_anger> ,
                                <https://raw.githubusercontent.com/MaddaGh/DataProcessing_EmoAnnotation/main/meaw.ttl#58_anger> ;
                   :isIncludedIn :anger ;
                   rdfs:comment "A tendency to engage in disagreements." .


###  https://raw.githubusercontent.com/MaddaGh/DataProcessing_EmoAnnotation/main/meaw.ttl#argumenting_with_facts
:argumenting_with_facts rdf:type owl:NamedIndividual ,
                                 :ConversationalFrame ;
                        rdfs:comment "A Conversational Frames where the speaker expresses objective facts or reports on events to support the validity of their perspective on the topic of conversation." .


###  https://raw.githubusercontent.com/MaddaGh/DataProcessing_EmoAnnotation/main/meaw.ttl#argumenting_with_personal_experience
:argumenting_with_personal_experience rdf:type owl:NamedIndividual ,
                                               :ConversationalFrame ;
                                      rdfs:comment "A Conversational Frame where the speaker recalls a personal experience or another type of subjective argument to support the validity of their perspective on the topic of conversation." .


###  https://raw.githubusercontent.com/MaddaGh/DataProcessing_EmoAnnotation/main/meaw.ttl#asking_for_argumentation
:asking_for_argumentation rdf:type owl:NamedIndividual ,
                                   :ConversationalFrame ;
                          rdfs:comment "A Conversational Frame where a person participating to the talk show expressly asks another person to argument and furtherly explain their perspective on the topic." .


###  https://raw.githubusercontent.com/MaddaGh/DataProcessing_EmoAnnotation/main/meaw.ttl#aversion
:aversion rdf:type owl:NamedIndividual ,
                   :Emotion ,
                   :EmotionState ;
          :expressedIn <https://raw.githubusercontent.com/MaddaGh/DataProcessing_EmoAnnotation/main/meaw.ttl#57_disgust> ;
          :isIncludedIn :disgust ;
          rdfs:comment "An impulse to avoid something disgusting." .


###  https://raw.githubusercontent.com/MaddaGh/DataProcessing_EmoAnnotation/main/meaw.ttl#bitterness
:bitterness rdf:type owl:NamedIndividual ,
                     :Emotion ,
                     :EmotionState ;
            :isIncludedIn :anger ;
            rdfs:comment "Anger after unfair treatment." .


###  https://raw.githubusercontent.com/MaddaGh/DataProcessing_EmoAnnotation/main/meaw.ttl#clarifying_concept
:clarifying_concept rdf:type owl:NamedIndividual ,
                             :ConversationalFrame ;
                    rdfs:comment "A Conversational Frame where the speaker is not expressing their own perspective but clarifying a concept, adding information, or explaining unknown terms to make them clear for everyone taking part in the conversation." .


###  https://raw.githubusercontent.com/MaddaGh/DataProcessing_EmoAnnotation/main/meaw.ttl#close_up
:close_up rdf:type owl:NamedIndividual ,
                   :FramingTechnique ,
                   :ShotType ;
          rdfs:comment "Close-Up (CU): Isolates a specific part of the subject, often the face, to convey emotions, reactions, or details in a more intimate way." .


###  https://raw.githubusercontent.com/MaddaGh/DataProcessing_EmoAnnotation/main/meaw.ttl#compassion
:compassion rdf:type owl:NamedIndividual ,
                     :Emotion ,
                     :EmotionState ;
            :isIncludedIn :enjoyment ;
            rdfs:comment "Enjoyment of helping to relieve another person's suffering." .


###  https://raw.githubusercontent.com/MaddaGh/DataProcessing_EmoAnnotation/main/meaw.ttl#conflict
:conflict rdf:type owl:NamedIndividual ,
                   :CameraFramingInterpretation ;
          :isframingInterpretationOf <https://raw.githubusercontent.com/MaddaGh/DataProcessing_EmoAnnotation/main/meaw.ttl#51_anger> ,
                                     <https://raw.githubusercontent.com/MaddaGh/DataProcessing_EmoAnnotation/main/meaw.ttl#55_anger> .


###  https://raw.githubusercontent.com/MaddaGh/DataProcessing_EmoAnnotation/main/meaw.ttl#contextualizing
:contextualizing rdf:type owl:NamedIndividual ,
                          :CameraFramingInterpretation ;
                 :isframingInterpretationOf <https://raw.githubusercontent.com/MaddaGh/DataProcessing_EmoAnnotation/main/meaw.ttl#40_neutrality> ,
                                            <https://raw.githubusercontent.com/MaddaGh/DataProcessing_EmoAnnotation/main/meaw.ttl#46_fear> ,
                                            <https://raw.githubusercontent.com/MaddaGh/DataProcessing_EmoAnnotation/main/meaw.ttl#58_anger> .


###  https://raw.githubusercontent.com/MaddaGh/DataProcessing_EmoAnnotation/main/meaw.ttl#couple
:couple rdf:type owl:NamedIndividual ,
                 :Agent ,
                 :Group ;
        :isExperiencerIn <https://raw.githubusercontent.com/MaddaGh/DataProcessing_EmoAnnotation/main/meaw.ttl#55_anger> .


###  https://raw.githubusercontent.com/MaddaGh/DataProcessing_EmoAnnotation/main/meaw.ttl#cover_mouth
:cover_mouth rdf:type owl:NamedIndividual ,
                      :Gesture ,
                      :HandGesture ,
                      :HumanVisualContent ,
                      :Trigger ,
                      :VisualTrigger ;
             :isShownIn <https://raw.githubusercontent.com/MaddaGh/DataProcessing_EmoAnnotation/main/meaw.ttl#46_2> ;
             :triggers <https://raw.githubusercontent.com/MaddaGh/DataProcessing_EmoAnnotation/main/meaw.ttl#46_fear> .


###  https://raw.githubusercontent.com/MaddaGh/DataProcessing_EmoAnnotation/main/meaw.ttl#cross_eye
:cross_eye rdf:type owl:NamedIndividual ,
                    :EyeMovement ,
                    :FacialMovement ,
                    :HumanVisualContent .


###  https://raw.githubusercontent.com/MaddaGh/DataProcessing_EmoAnnotation/main/meaw.ttl#depress_lip_corner
:depress_lip_corner rdf:type owl:NamedIndividual ,
                             :FacialMovement ,
                             :HumanVisualContent .


###  https://raw.githubusercontent.com/MaddaGh/DataProcessing_EmoAnnotation/main/meaw.ttl#depress_lower_lip
:depress_lower_lip rdf:type owl:NamedIndividual ,
                            :FacialMovement ,
                            :HumanVisualContent .


###  https://raw.githubusercontent.com/MaddaGh/DataProcessing_EmoAnnotation/main/meaw.ttl#despair
:despair rdf:type owl:NamedIndividual ,
                  :Emotion ,
                  :EmotionState ;
         :isIncludedIn :sadness ;
         rdfs:comment "The loss of hope that a bad situation will improve or change." .


###  https://raw.githubusercontent.com/MaddaGh/DataProcessing_EmoAnnotation/main/meaw.ttl#desperation
:desperation rdf:type owl:NamedIndividual ,
                      :Emotion ,
                      :EmotionState ;
             :isIncludedIn :fear ;
             rdfs:comment "A response to the inability to reduce danger." .


###  https://raw.githubusercontent.com/MaddaGh/DataProcessing_EmoAnnotation/main/meaw.ttl#detachement
:detachement rdf:type owl:NamedIndividual ,
                      :CameraFramingInterpretation .


###  https://raw.githubusercontent.com/MaddaGh/DataProcessing_EmoAnnotation/main/meaw.ttl#detail
:detail rdf:type owl:NamedIndividual ,
                 :FramingTechnique ,
                 :ShotType ;
        rdfs:comment "Detail Shot (DS): A shot that focuses on a small, specific element within the scene, highlighting details that are crucial to the narrative or conveying specific information." .


###  https://raw.githubusercontent.com/MaddaGh/DataProcessing_EmoAnnotation/main/meaw.ttl#dialogue
:dialogue rdf:type owl:NamedIndividual ,
                   :AuralComposition .


###  https://raw.githubusercontent.com/MaddaGh/DataProcessing_EmoAnnotation/main/meaw.ttl#disagreeing_by_interrupting
:disagreeing_by_interrupting rdf:type owl:NamedIndividual ,
                                      :ConversationalFrame ;
                             rdfs:comment "A conversational frame where a speaker interrupts another speaker without the host mediating the change, to disagree or contradict the previous speaker." .


###  https://raw.githubusercontent.com/MaddaGh/DataProcessing_EmoAnnotation/main/meaw.ttl#disagreeing_with_facts
:disagreeing_with_facts rdf:type owl:NamedIndividual ,
                                 :ConversationalFrame ;
                        rdfs:comment "A Conversational Frame where a speaker is given speaking space by the host, and they outline facts or events related to the topic that have the goal of proving other speaker’s arguments wrong." .


###  https://raw.githubusercontent.com/MaddaGh/DataProcessing_EmoAnnotation/main/meaw.ttl#disagreeing_with_opinion
:disagreeing_with_opinion rdf:type owl:NamedIndividual ,
                                   :ConversationalFrame ;
                          rdfs:comment "A Conversational Frame where a speaker is given speaking space by the host, and they express a perspective on the topic that disagrees with the one of the previous speaker." .


###  https://raw.githubusercontent.com/MaddaGh/DataProcessing_EmoAnnotation/main/meaw.ttl#disappointment
:disappointment rdf:type owl:NamedIndividual ,
                         :Emotion ,
                         :EmotionState ;
                :isIncludedIn :sadness ;
                rdfs:comment "A feeling that expectations are not being met." .


###  https://raw.githubusercontent.com/MaddaGh/DataProcessing_EmoAnnotation/main/meaw.ttl#discouragement
:discouragement rdf:type owl:NamedIndividual ,
                         :Emotion ,
                         :EmotionState ;
                :isIncludedIn :sadness ;
                rdfs:comment "A response to repeated failures to accomplish something: the belief that it can't be done." .


###  https://raw.githubusercontent.com/MaddaGh/DataProcessing_EmoAnnotation/main/meaw.ttl#disgust
:disgust rdf:type owl:NamedIndividual ,
                  :BasicEmotion ,
                  :Emotion ;
         :expressedIn <https://raw.githubusercontent.com/MaddaGh/DataProcessing_EmoAnnotation/main/meaw.ttl#57_disgust> ;
         :includes :abhorrence ,
                   :aversion ,
                   :dislike ,
                   :distaste ,
                   :loathing ,
                   :repugnance ,
                   :revulsion ;
         rdfs:comment "Feeling disgusted by what is toxic helps us to avoid being poisoned, physically or socially (description from http://atlasofemotions.org/)." .


###  https://raw.githubusercontent.com/MaddaGh/DataProcessing_EmoAnnotation/main/meaw.ttl#dislike
:dislike rdf:type owl:NamedIndividual ,
                  :Emotion ,
                  :EmotionState ;
         :isIncludedIn :disgust ;
         rdfs:comment "A preference against something." .


###  https://raw.githubusercontent.com/MaddaGh/DataProcessing_EmoAnnotation/main/meaw.ttl#distaste
:distaste rdf:type owl:NamedIndividual ,
                   :Emotion ,
                   :EmotionState ;
          :isIncludedIn :disgust ;
          rdfs:comment "Reaction to a bad taste, smell, thing or idea. Can be literal or metaphorical." .


###  https://raw.githubusercontent.com/MaddaGh/DataProcessing_EmoAnnotation/main/meaw.ttl#distraughtness
:distraughtness rdf:type owl:NamedIndividual ,
                         :Emotion ,
                         :EmotionState ;
                :isIncludedIn :sadness ;
                rdfs:comment "Sadness that makes it hard to think clearly." .


###  https://raw.githubusercontent.com/MaddaGh/DataProcessing_EmoAnnotation/main/meaw.ttl#dolly
:dolly rdf:type owl:NamedIndividual ,
                :CameraMovement ,
                :FramingTechnique ;
       rdfs:comment "Dolly Shot: Similar to a tracking shot but involves moving the entire camera rig on a set of wheels or tracks." .


###  https://raw.githubusercontent.com/MaddaGh/DataProcessing_EmoAnnotation/main/meaw.ttl#dread
:dread rdf:type owl:NamedIndividual ,
                :Emotion ,
                :EmotionState ;
       :isIncludedIn :fear ;
       rdfs:comment "Anticipation of severe danger." .


###  https://raw.githubusercontent.com/MaddaGh/DataProcessing_EmoAnnotation/main/meaw.ttl#ecstasy
:ecstasy rdf:type owl:NamedIndividual ,
                  :Emotion ,
                  :EmotionState ;
         :isIncludedIn :enjoyment ;
         rdfs:comment "Rapturous delight. A state of very great happiness, nearly overwhelming." .


###  https://raw.githubusercontent.com/MaddaGh/DataProcessing_EmoAnnotation/main/meaw.ttl#engaging_with
:engaging_with rdf:type owl:NamedIndividual ,
                        :CameraFramingInterpretation ;
               :isframingInterpretationOf <https://raw.githubusercontent.com/MaddaGh/DataProcessing_EmoAnnotation/main/meaw.ttl#41_sadness> ,
                                          <https://raw.githubusercontent.com/MaddaGh/DataProcessing_EmoAnnotation/main/meaw.ttl#45_neutrality> ,
                                          <https://raw.githubusercontent.com/MaddaGh/DataProcessing_EmoAnnotation/main/meaw.ttl#57_disgust> .


###  https://raw.githubusercontent.com/MaddaGh/DataProcessing_EmoAnnotation/main/meaw.ttl#enjoyment
:enjoyment rdf:type owl:NamedIndividual ,
                    :BasicEmotion ,
                    :Emotion ;
           :includes :amusement ,
                     :compassion ,
                     :ecstasy ,
                     :fiero ,
                     :naches ,
                     :peace ,
                     :pride ,
                     :rejoicing ,
                     :relief ,
                     :schadenfreude ,
                     :sensory_pleasure ,
                     :wonder ;
           rdfs:comment "We feel enjoyment when we experience novelty or comfort. Enjoyment varies in strength and frequency in our lives (description from http://atlasofemotions.org/)." .


###  https://raw.githubusercontent.com/MaddaGh/DataProcessing_EmoAnnotation/main/meaw.ttl#exasperation
:exasperation rdf:type owl:NamedIndividual ,
                       :Emotion ,
                       :EmotionState ;
              :isIncludedIn :anger ;
              rdfs:comment "Anger caused by a repeated or strong nuisance." .


###  https://raw.githubusercontent.com/MaddaGh/DataProcessing_EmoAnnotation/main/meaw.ttl#excitement
:excitement rdf:type owl:NamedIndividual ,
                     :Emotion ,
                     :EmotionState ;
            rdfs:comment "A powerful enthusiasm." .


###  https://raw.githubusercontent.com/MaddaGh/DataProcessing_EmoAnnotation/main/meaw.ttl#extreme_close_up
:extreme_close_up rdf:type owl:NamedIndividual ,
                           :FramingTechnique ,
                           :ShotType ;
                  rdfs:comment "Extreme Close-Up (ECU): Zooms in on a very small detail or portion of the subject, emphasizing extreme emotions or important details." .


###  https://raw.githubusercontent.com/MaddaGh/DataProcessing_EmoAnnotation/main/meaw.ttl#extreme_long_shot
:extreme_long_shot rdf:type owl:NamedIndividual ,
                            :FramingTechnique ,
                            :ShotType ;
                   rdfs:comment "Extreme Long Shot (ELS): Captures a vast landscape or environment, often featuring small or distant subjects to establish a location." .


###  https://raw.githubusercontent.com/MaddaGh/DataProcessing_EmoAnnotation/main/meaw.ttl#eyes_closed
:eyes_closed rdf:type owl:NamedIndividual ,
                      :EyeMovement ,
                      :FacialMovement ,
                      :HumanVisualContent .


###  https://raw.githubusercontent.com/MaddaGh/DataProcessing_EmoAnnotation/main/meaw.ttl#eyes_down
:eyes_down rdf:type owl:NamedIndividual ,
                    :EyeMovement ,
                    :FacialMovement ,
                    :HumanVisualContent .


###  https://raw.githubusercontent.com/MaddaGh/DataProcessing_EmoAnnotation/main/meaw.ttl#eyes_turn_left
:eyes_turn_left rdf:type owl:NamedIndividual ,
                         :EyeMovement ,
                         :FacialMovement ,
                         :HumanVisualContent .


###  https://raw.githubusercontent.com/MaddaGh/DataProcessing_EmoAnnotation/main/meaw.ttl#eyes_turn_right
:eyes_turn_right rdf:type owl:NamedIndividual ,
                          :EyeMovement ,
                          :FacialMovement ,
                          :HumanVisualContent .


###  https://raw.githubusercontent.com/MaddaGh/DataProcessing_EmoAnnotation/main/meaw.ttl#eyes_up
:eyes_up rdf:type owl:NamedIndividual ,
                  :EyeMovement ,
                  :FacialMovement ,
                  :HumanVisualContent ;
         :isShownIn <https://raw.githubusercontent.com/MaddaGh/DataProcessing_EmoAnnotation/main/meaw.ttl#43_1> ,
                    <https://raw.githubusercontent.com/MaddaGh/DataProcessing_EmoAnnotation/main/meaw.ttl#50_1> ,
                    <https://raw.githubusercontent.com/MaddaGh/DataProcessing_EmoAnnotation/main/meaw.ttl#51_1> ,
                    <https://raw.githubusercontent.com/MaddaGh/DataProcessing_EmoAnnotation/main/meaw.ttl#55_2> .


###  https://raw.githubusercontent.com/MaddaGh/DataProcessing_EmoAnnotation/main/meaw.ttl#fear
:fear rdf:type owl:NamedIndividual ,
               :BasicEmotion ,
               :Emotion ;
      :expressedIn <https://raw.githubusercontent.com/MaddaGh/DataProcessing_EmoAnnotation/main/meaw.ttl#43_fear> ,
                   <https://raw.githubusercontent.com/MaddaGh/DataProcessing_EmoAnnotation/main/meaw.ttl#46_fear> ;
      :includes :anxiety ,
                :desperation ,
                :dread ,
                :horror ,
                :nervousness ,
                :panic ,
                :terror ;
      rdfs:comment "Our fear of danger lets us anticipate threats to our safety (description from http://atlasofemotions.org/)." .


###  https://raw.githubusercontent.com/MaddaGh/DataProcessing_EmoAnnotation/main/meaw.ttl#female
:female rdf:type owl:NamedIndividual ,
                 :Gender .


###  https://raw.githubusercontent.com/MaddaGh/DataProcessing_EmoAnnotation/main/meaw.ttl#fiero
:fiero rdf:type owl:NamedIndividual ,
                :Emotion ,
                :EmotionState ;
       :isIncludedIn :enjoyment ;
       rdfs:comment "Enjoyment of meeting a difficult challenge (an Italian word)." .


###  https://raw.githubusercontent.com/MaddaGh/DataProcessing_EmoAnnotation/main/meaw.ttl#frowning
:frowning rdf:type owl:NamedIndividual ,
                   :FacialMovement ,
                   :HumanVisualContent ,
                   :Trigger ,
                   :VisualTrigger ;
          owl:sameAs :lower_brow ;
          :isShownIn <https://raw.githubusercontent.com/MaddaGh/DataProcessing_EmoAnnotation/main/meaw.ttl#43_2> ,
                     <https://raw.githubusercontent.com/MaddaGh/DataProcessing_EmoAnnotation/main/meaw.ttl#51_1> ,
                     <https://raw.githubusercontent.com/MaddaGh/DataProcessing_EmoAnnotation/main/meaw.ttl#55_1> ;
          :triggers <https://raw.githubusercontent.com/MaddaGh/DataProcessing_EmoAnnotation/main/meaw.ttl#50_anger> ,
                    <https://raw.githubusercontent.com/MaddaGh/DataProcessing_EmoAnnotation/main/meaw.ttl#51_anger> .


###  https://raw.githubusercontent.com/MaddaGh/DataProcessing_EmoAnnotation/main/meaw.ttl#lower_brow
:lower_brow rdf:type owl:NamedIndividual .


###  https://raw.githubusercontent.com/MaddaGh/DataProcessing_EmoAnnotation/main/meaw.ttl#frustration
:frustration rdf:type owl:NamedIndividual ,
                      :Emotion ,
                      :EmotionState ;
             :expressedIn <https://raw.githubusercontent.com/MaddaGh/DataProcessing_EmoAnnotation/main/meaw.ttl#50_anger> ,
                          <https://raw.githubusercontent.com/MaddaGh/DataProcessing_EmoAnnotation/main/meaw.ttl#51_anger> ;
             :isIncludedIn :anger ;
             rdfs:comment "A response to repeated failures to overcome an obstacle." .


###  https://raw.githubusercontent.com/MaddaGh/DataProcessing_EmoAnnotation/main/meaw.ttl#funnel_lips
:funnel_lips rdf:type owl:NamedIndividual ,
                      :FacialMovement ,
                      :HumanVisualContent .


###  https://raw.githubusercontent.com/MaddaGh/DataProcessing_EmoAnnotation/main/meaw.ttl#fury
:fury rdf:type owl:NamedIndividual ,
               :Emotion ,
               :EmotionState ;
      :isIncludedIn :anger ;
      rdfs:comment "Uncontrolled and often violent anger." .


###  https://raw.githubusercontent.com/MaddaGh/DataProcessing_EmoAnnotation/main/meaw.ttl#gekwetst
:gekwetst rdf:type owl:NamedIndividual ,
                   :Trigger ,
                   :VerbalTrigger ;
          :triggers <https://raw.githubusercontent.com/MaddaGh/DataProcessing_EmoAnnotation/main/meaw.ttl#40_sadness> ,
                    <https://raw.githubusercontent.com/MaddaGh/DataProcessing_EmoAnnotation/main/meaw.ttl#41_sadness> ,
                    <https://raw.githubusercontent.com/MaddaGh/DataProcessing_EmoAnnotation/main/meaw.ttl#51_anger> .


###  https://raw.githubusercontent.com/MaddaGh/DataProcessing_EmoAnnotation/main/meaw.ttl#gesticulation
:gesticulation rdf:type owl:NamedIndividual ,
                        :Gesture ,
                        :HandGesture ,
                        :HumanVisualContent ;
               :isShownIn <https://raw.githubusercontent.com/MaddaGh/DataProcessing_EmoAnnotation/main/meaw.ttl#50_1> ,
                          <https://raw.githubusercontent.com/MaddaGh/DataProcessing_EmoAnnotation/main/meaw.ttl#51_1> ,
                          <https://raw.githubusercontent.com/MaddaGh/DataProcessing_EmoAnnotation/main/meaw.ttl#57_2> .


###  https://raw.githubusercontent.com/MaddaGh/DataProcessing_EmoAnnotation/main/meaw.ttl#giving_talking_space
:giving_talking_space rdf:type owl:NamedIndividual ,
                               :ConversationalFrame ;
                      rdfs:comment "A conversational frame where the host intervenes to change the speaker, mediating from what the last speaker said to what another speaker has to say." .


###  https://raw.githubusercontent.com/MaddaGh/DataProcessing_EmoAnnotation/main/meaw.ttl#giving_talking_space_with_question
:giving_talking_space_with_question rdf:type owl:NamedIndividual ,
                                             :ConversationalFrame ;
                                    rdfs:comment "A conversational frame where the host intervenes to change the speaker, mediating from what the last speaker said to what another speaker has to say, by directly asking them a question such as “what do you think about this?”." .


###  https://raw.githubusercontent.com/MaddaGh/DataProcessing_EmoAnnotation/main/meaw.ttl#grief
:grief rdf:type owl:NamedIndividual ,
                :Emotion ,
                :EmotionState ;
       :isIncludedIn :sadness ;
       rdfs:comment "Sadness over a deep loss." .


###  https://raw.githubusercontent.com/MaddaGh/DataProcessing_EmoAnnotation/main/meaw.ttl#guest
:guest rdf:type owl:NamedIndividual ,
                :Role ;
       rdfs:comment "One or more people, usually named public figures that are invited as guests in the talk show on the premises of their expertise or involvement in the topic of conversation." .


###  https://raw.githubusercontent.com/MaddaGh/DataProcessing_EmoAnnotation/main/meaw.ttl#head_back
:head_back rdf:type owl:NamedIndividual ,
                    :Gesture ,
                    :HeadGesture ,
                    :HumanVisualContent .


###  https://raw.githubusercontent.com/MaddaGh/DataProcessing_EmoAnnotation/main/meaw.ttl#head_down
:head_down rdf:type owl:NamedIndividual ,
                    :Gesture ,
                    :HeadGesture ,
                    :HumanVisualContent ;
           :isShownIn <https://raw.githubusercontent.com/MaddaGh/DataProcessing_EmoAnnotation/main/meaw.ttl#43_2> .


###  https://raw.githubusercontent.com/MaddaGh/DataProcessing_EmoAnnotation/main/meaw.ttl#head_forward
:head_forward rdf:type owl:NamedIndividual ,
                       :Gesture ,
                       :HeadGesture ,
                       :HumanVisualContent .


###  https://raw.githubusercontent.com/MaddaGh/DataProcessing_EmoAnnotation/main/meaw.ttl#head_shake_side_to_side
:head_shake_side_to_side rdf:type owl:NamedIndividual ,
                                  :Gesture ,
                                  :HeadGesture ,
                                  :HumanVisualContent ,
                                  :Trigger ,
                                  :VisualTrigger ;
                         owl:sameAs :headshake ;
                         :isShownIn <https://raw.githubusercontent.com/MaddaGh/DataProcessing_EmoAnnotation/main/meaw.ttl#41_3> ;
                         :triggers <https://raw.githubusercontent.com/MaddaGh/DataProcessing_EmoAnnotation/main/meaw.ttl#57_disgust> .


###  https://raw.githubusercontent.com/MaddaGh/DataProcessing_EmoAnnotation/main/meaw.ttl#headshake
:headshake rdf:type owl:NamedIndividual .


###  https://raw.githubusercontent.com/MaddaGh/DataProcessing_EmoAnnotation/main/meaw.ttl#head_shake_up_and_down
:head_shake_up_and_down rdf:type owl:NamedIndividual ,
                                 :Gesture ,
                                 :HeadGesture ,
                                 :HumanVisualContent ;
                        :isShownIn <https://raw.githubusercontent.com/MaddaGh/DataProcessing_EmoAnnotation/main/meaw.ttl#43_1> ,
                                   <https://raw.githubusercontent.com/MaddaGh/DataProcessing_EmoAnnotation/main/meaw.ttl#45_2> ,
                                   <https://raw.githubusercontent.com/MaddaGh/DataProcessing_EmoAnnotation/main/meaw.ttl#46_2> ,
                                   <https://raw.githubusercontent.com/MaddaGh/DataProcessing_EmoAnnotation/main/meaw.ttl#51_2> ,
                                   <https://raw.githubusercontent.com/MaddaGh/DataProcessing_EmoAnnotation/main/meaw.ttl#55_3> ,
                                   <https://raw.githubusercontent.com/MaddaGh/DataProcessing_EmoAnnotation/main/meaw.ttl#55_4> ,
                                   <https://raw.githubusercontent.com/MaddaGh/DataProcessing_EmoAnnotation/main/meaw.ttl#55_5> .


###  https://raw.githubusercontent.com/MaddaGh/DataProcessing_EmoAnnotation/main/meaw.ttl#head_thrust_forward
:head_thrust_forward rdf:type owl:NamedIndividual ,
                              :Gesture ,
                              :HeadGesture ,
                              :HumanVisualContent .


###  https://raw.githubusercontent.com/MaddaGh/DataProcessing_EmoAnnotation/main/meaw.ttl#head_tilt_left
:head_tilt_left rdf:type owl:NamedIndividual ,
                         :Gesture ,
                         :HeadGesture ,
                         :HumanVisualContent .


###  https://raw.githubusercontent.com/MaddaGh/DataProcessing_EmoAnnotation/main/meaw.ttl#head_tilt_right
:head_tilt_right rdf:type owl:NamedIndividual ,
                          :Gesture ,
                          :HeadGesture ,
                          :HumanVisualContent .


###  https://raw.githubusercontent.com/MaddaGh/DataProcessing_EmoAnnotation/main/meaw.ttl#head_turn_left
:head_turn_left rdf:type owl:NamedIndividual ,
                         :Gesture ,
                         :HeadGesture ,
                         :HumanVisualContent .


###  https://raw.githubusercontent.com/MaddaGh/DataProcessing_EmoAnnotation/main/meaw.ttl#head_turn_right
:head_turn_right rdf:type owl:NamedIndividual ,
                          :Gesture ,
                          :HeadGesture ,
                          :HumanVisualContent .


###  https://raw.githubusercontent.com/MaddaGh/DataProcessing_EmoAnnotation/main/meaw.ttl#head_up
:head_up rdf:type owl:NamedIndividual ,
                  :Gesture ,
                  :HeadGesture ,
                  :HumanVisualContent .


###  https://raw.githubusercontent.com/MaddaGh/DataProcessing_EmoAnnotation/main/meaw.ttl#head_upward_and_side
:head_upward_and_side rdf:type owl:NamedIndividual ,
                               :Gesture ,
                               :HeadGesture ,
                               :HumanVisualContent .


###  https://raw.githubusercontent.com/MaddaGh/DataProcessing_EmoAnnotation/main/meaw.ttl#headshake
:headshake rdf:type owl:NamedIndividual ,
                    :Gesture ,
                    :HeadGesture ,
                    :HumanVisualContent ,
                    :Trigger ,
                    :VisualTrigger ;
           :isShownIn <https://raw.githubusercontent.com/MaddaGh/DataProcessing_EmoAnnotation/main/meaw.ttl#41_3> ;
           :triggers <https://raw.githubusercontent.com/MaddaGh/DataProcessing_EmoAnnotation/main/meaw.ttl#57_disgust> .


###  https://raw.githubusercontent.com/MaddaGh/DataProcessing_EmoAnnotation/main/meaw.ttl#helplessness
:helplessness rdf:type owl:NamedIndividual ,
                       :Emotion ,
                       :EmotionState ;
              :isIncludedIn :sadness ;
              rdfs:comment "The realization that one cannot make a situation better or easier." .


###  https://raw.githubusercontent.com/MaddaGh/DataProcessing_EmoAnnotation/main/meaw.ttl#hopelessness
:hopelessness rdf:type owl:NamedIndividual ,
                       :Emotion ,
                       :EmotionState ;
              rdfs:comment "The belief that nothing good will happen." .


###  https://raw.githubusercontent.com/MaddaGh/DataProcessing_EmoAnnotation/main/meaw.ttl#horizontal_frontal
:horizontal_frontal rdf:type owl:NamedIndividual ,
                             :CameraAngle ,
                             :FramingTechnique .


###  https://raw.githubusercontent.com/MaddaGh/DataProcessing_EmoAnnotation/main/meaw.ttl#horizontal_oblique
:horizontal_oblique rdf:type owl:NamedIndividual ,
                             :CameraAngle ,
                             :FramingTechnique .


###  https://raw.githubusercontent.com/MaddaGh/DataProcessing_EmoAnnotation/main/meaw.ttl#horror
:horror rdf:type owl:NamedIndividual ,
                 :Emotion ,
                 :EmotionState ;
        :isIncludedIn :fear ;
        rdfs:comment "A mixture of fear, disgust, and shock." .


###  https://raw.githubusercontent.com/MaddaGh/DataProcessing_EmoAnnotation/main/meaw.ttl#host
:host rdf:type owl:NamedIndividual ,
               :Role ;
      rdfs:comment "The host of the talk show, which is the person that introduces the topic of discussion and mediates the discussion throughout the talk show." .


###  https://raw.githubusercontent.com/MaddaGh/DataProcessing_EmoAnnotation/main/meaw.ttl#ik_ben_doodzenuwachtig
:ik_ben_doodzenuwachtig rdf:type owl:NamedIndividual ,
                                 :Trigger ,
                                 :VerbalTrigger ;
                        :triggers <https://raw.githubusercontent.com/MaddaGh/DataProcessing_EmoAnnotation/main/meaw.ttl#43_fear> .


###  https://raw.githubusercontent.com/MaddaGh/DataProcessing_EmoAnnotation/main/meaw.ttl#ik_vond_het_heel_vervelend
:ik_vond_het_heel_vervelend rdf:type owl:NamedIndividual ,
                                     :Trigger ,
                                     :VerbalTrigger ;
                            :triggers <https://raw.githubusercontent.com/MaddaGh/DataProcessing_EmoAnnotation/main/meaw.ttl#43_anger> .


###  https://raw.githubusercontent.com/MaddaGh/DataProcessing_EmoAnnotation/main/meaw.ttl#introducing_topic
:introducing_topic rdf:type owl:NamedIndividual ,
                            :ConversationalFrame ;
                   rdfs:comment "A conversational frame where the hosts introduce a topic of conversation, usually giving some information about the why is something worth discussing, the context of the topic and identifying some divisive or problematic aspect of the issue that participants in the talk show must share their perspective on. It is usually the frame that begins the talk show or a talk show section or it can be a frame present in the middle of the conversation to shift the topic of the discussion." .


###  https://raw.githubusercontent.com/MaddaGh/DataProcessing_EmoAnnotation/main/meaw.ttl#involvement
:involvement rdf:type owl:NamedIndividual ,
                      :CameraFramingInterpretation ;
             :isframingInterpretationOf <https://raw.githubusercontent.com/MaddaGh/DataProcessing_EmoAnnotation/main/meaw.ttl#43_fear> ,
                                        <https://raw.githubusercontent.com/MaddaGh/DataProcessing_EmoAnnotation/main/meaw.ttl#50_anger> .


###  https://raw.githubusercontent.com/MaddaGh/DataProcessing_EmoAnnotation/main/meaw.ttl#jaw_drop
:jaw_drop rdf:type owl:NamedIndividual ,
                   :FacialMovement ,
                   :HumanVisualContent .


###  https://raw.githubusercontent.com/MaddaGh/DataProcessing_EmoAnnotation/main/meaw.ttl#laughter
:laughter rdf:type owl:NamedIndividual ,
                   :AuralTrigger ,
                   :Trigger ;
          :triggers <https://raw.githubusercontent.com/MaddaGh/DataProcessing_EmoAnnotation/main/meaw.ttl#46_fear> .


###  https://raw.githubusercontent.com/MaddaGh/DataProcessing_EmoAnnotation/main/meaw.ttl#leaning_towards_interlocutor
:leaning_towards_interlocutor rdf:type owl:NamedIndividual ,
                                       :HumanVisualContent ,
                                       :Kinetic ;
                              :isShownIn <https://raw.githubusercontent.com/MaddaGh/DataProcessing_EmoAnnotation/main/meaw.ttl#57_1> .


###  https://raw.githubusercontent.com/MaddaGh/DataProcessing_EmoAnnotation/main/meaw.ttl#legien_kromkamp
:legien_kromkamp rdf:type owl:NamedIndividual ,
                          :Agent ,
                          :NamedPerson ,
                          :Person ;
                 :hasConversationalRolePlay <https://raw.githubusercontent.com/MaddaGh/DataProcessing_EmoAnnotation/main/meaw.ttl#2101608040029452931_host> ;
                 :hasGender :female ;
                 :isExperiencerIn <https://raw.githubusercontent.com/MaddaGh/DataProcessing_EmoAnnotation/main/meaw.ttl#40_neutrality> ,
                                  <https://raw.githubusercontent.com/MaddaGh/DataProcessing_EmoAnnotation/main/meaw.ttl#45_neutrality> ,
                                  <https://raw.githubusercontent.com/MaddaGh/DataProcessing_EmoAnnotation/main/meaw.ttl#46_fear> ;
                 :hasNameSource "annotator" .


###  https://raw.githubusercontent.com/MaddaGh/DataProcessing_EmoAnnotation/main/meaw.ttl#lips_toward_each_other
:lips_toward_each_other rdf:type owl:NamedIndividual ,
                                 :FacialMovement ,
                                 :HumanVisualContent .


###  https://raw.githubusercontent.com/MaddaGh/DataProcessing_EmoAnnotation/main/meaw.ttl#loathing
:loathing rdf:type owl:NamedIndividual ,
                   :Emotion ,
                   :EmotionState ;
          :isIncludedIn :disgust ;
          rdfs:comment "Intense disgust focused on a person. Intense disgust focused on oneself is called self-loathing." .


###  https://raw.githubusercontent.com/MaddaGh/DataProcessing_EmoAnnotation/main/meaw.ttl#long_shot
:long_shot rdf:type owl:NamedIndividual ,
                    :FramingTechnique ,
                    :ShotType ;
           rdfs:comment "Long Shot (LS): Frames the full body of the subject, showing them in relation to their surroundings." .


###  https://raw.githubusercontent.com/MaddaGh/DataProcessing_EmoAnnotation/main/meaw.ttl#look_forward
:look_forward rdf:type owl:NamedIndividual ,
                       :EyeMovement ,
                       :FacialMovement ,
                       :HumanVisualContent ,
                       :Trigger ,
                       :VisualTrigger ;
              :isShownIn <https://raw.githubusercontent.com/MaddaGh/DataProcessing_EmoAnnotation/main/meaw.ttl#50_1> ,
                         <https://raw.githubusercontent.com/MaddaGh/DataProcessing_EmoAnnotation/main/meaw.ttl#58_1> .


###  https://raw.githubusercontent.com/MaddaGh/DataProcessing_EmoAnnotation/main/meaw.ttl#lower_brow
:lower_brow rdf:type owl:NamedIndividual ,
                     :FacialMovement ,
                     :HumanVisualContent ,
                     :Trigger ,
                     :VisualTrigger ;
            :isShownIn <https://raw.githubusercontent.com/MaddaGh/DataProcessing_EmoAnnotation/main/meaw.ttl#43_2> ,
                       <https://raw.githubusercontent.com/MaddaGh/DataProcessing_EmoAnnotation/main/meaw.ttl#51_1> ,
                       <https://raw.githubusercontent.com/MaddaGh/DataProcessing_EmoAnnotation/main/meaw.ttl#55_1> ;
            :triggers <https://raw.githubusercontent.com/MaddaGh/DataProcessing_EmoAnnotation/main/meaw.ttl#50_anger> ,
                      <https://raw.githubusercontent.com/MaddaGh/DataProcessing_EmoAnnotation/main/meaw.ttl#51_anger> .


###  https://raw.githubusercontent.com/MaddaGh/DataProcessing_EmoAnnotation/main/meaw.ttl#make_eye_contact
:make_eye_contact rdf:type owl:NamedIndividual ,
                           :EyeMovement ,
                           :FacialMovement ,
                           :HumanVisualContent ;
                  :isShownIn <https://raw.githubusercontent.com/MaddaGh/DataProcessing_EmoAnnotation/main/meaw.ttl#41_3> ,
                             <https://raw.githubusercontent.com/MaddaGh/DataProcessing_EmoAnnotation/main/meaw.ttl#45_2> ,
                             <https://raw.githubusercontent.com/MaddaGh/DataProcessing_EmoAnnotation/main/meaw.ttl#46_2> ,
                             <https://raw.githubusercontent.com/MaddaGh/DataProcessing_EmoAnnotation/main/meaw.ttl#46_3> ,
                             <https://raw.githubusercontent.com/MaddaGh/DataProcessing_EmoAnnotation/main/meaw.ttl#55_2> ,
                             <https://raw.githubusercontent.com/MaddaGh/DataProcessing_EmoAnnotation/main/meaw.ttl#55_5> .


###  https://raw.githubusercontent.com/MaddaGh/DataProcessing_EmoAnnotation/main/meaw.ttl#male
:male rdf:type owl:NamedIndividual ,
               :Gender .


###  https://raw.githubusercontent.com/MaddaGh/DataProcessing_EmoAnnotation/main/meaw.ttl#medium_close_up
:medium_close_up rdf:type owl:NamedIndividual ,
                          :FramingTechnique ,
                          :ShotType ;
                 rdfs:comment "Medium Close-Up (MCU): Frames the subject from the chest or shoulders up, focusing on facial expressions and emotional nuances." .


###  https://raw.githubusercontent.com/MaddaGh/DataProcessing_EmoAnnotation/main/meaw.ttl#medium_long_shot
:medium_long_shot rdf:type owl:NamedIndividual ,
                           :FramingTechnique ,
                           :ShotType ;
                  rdfs:comment "Medium Long Shot (MLS): Frames the subject from the knees or hips up, providing more detail than a long shot while still showing some of the surroundings." .


###  https://raw.githubusercontent.com/MaddaGh/DataProcessing_EmoAnnotation/main/meaw.ttl#medium_shot
:medium_shot rdf:type owl:NamedIndividual ,
                      :FramingTechnique ,
                      :ShotType ;
             rdfs:comment "Medium Shot (MS): Frames the subject from the waist up, allowing for a closer view and emphasizing facial expressions and body language." .


###  https://raw.githubusercontent.com/MaddaGh/DataProcessing_EmoAnnotation/main/meaw.ttl#mensen_gekwetst_zijn
:mensen_gekwetst_zijn rdf:type owl:NamedIndividual ,
                               :Trigger ,
                               :VerbalTrigger ;
                      :triggers <https://raw.githubusercontent.com/MaddaGh/DataProcessing_EmoAnnotation/main/meaw.ttl#41_sadness1> .


###  https://raw.githubusercontent.com/MaddaGh/DataProcessing_EmoAnnotation/main/meaw.ttl#misery
:misery rdf:type owl:NamedIndividual ,
                 :Emotion ,
                 :EmotionState ;
        :isIncludedIn :sadness ;
        rdfs:comment "Strong suffering or unhappiness." .


###  https://raw.githubusercontent.com/MaddaGh/DataProcessing_EmoAnnotation/main/meaw.ttl#muddle
:muddle rdf:type owl:NamedIndividual ,
                 :AuralComposition .


###  https://raw.githubusercontent.com/MaddaGh/DataProcessing_EmoAnnotation/main/meaw.ttl#naches
:naches rdf:type owl:NamedIndividual ,
                 :Emotion ,
                 :EmotionState ;
        :isIncludedIn :enjoyment ;
        rdfs:comment "Joyful pride in the accomplishments of one's children or mentees (a Yiddish word)." .


###  https://raw.githubusercontent.com/MaddaGh/DataProcessing_EmoAnnotation/main/meaw.ttl#ncrv
:ncrv rdf:type owl:NamedIndividual ,
               :Broadcaster .


###  https://raw.githubusercontent.com/MaddaGh/DataProcessing_EmoAnnotation/main/meaw.ttl#nervousness
:nervousness rdf:type owl:NamedIndividual ,
                      :Emotion ,
                      :EmotionState ;
             :expressedIn <https://raw.githubusercontent.com/MaddaGh/DataProcessing_EmoAnnotation/main/meaw.ttl#46_fear> ;
             :isIncludedIn :fear ;
             rdfs:comment "Uncertainty as to whether there is a danger." .


###  https://raw.githubusercontent.com/MaddaGh/DataProcessing_EmoAnnotation/main/meaw.ttl#pan_left
:pan_left rdf:type owl:NamedIndividual ,
                   :CameraMovement ,
                   :FramingTechnique ;
          rdfs:comment "Pan: A camera movement where the camera pivots horizontally from a fixed position, scanning the scene from right to left. Panning is often used to follow action or reveal new elements within the frame." .


###  https://raw.githubusercontent.com/MaddaGh/DataProcessing_EmoAnnotation/main/meaw.ttl#pan_right
:pan_right rdf:type owl:NamedIndividual ,
                    :CameraMovement ,
                    :FramingTechnique ;
           rdfs:comment "Pan: A camera movement where the camera pivots horizontally from a fixed position, scanning the scene from left to right. Panning is often used to follow action or reveal new elements within the frame." .


###  https://raw.githubusercontent.com/MaddaGh/DataProcessing_EmoAnnotation/main/meaw.ttl#panic
:panic rdf:type owl:NamedIndividual ,
                :Emotion ,
                :EmotionState ;
       :isIncludedIn :fear ;
       rdfs:comment "Sudden uncontrollable fear." .


###  https://raw.githubusercontent.com/MaddaGh/DataProcessing_EmoAnnotation/main/meaw.ttl#part_lips
:part_lips rdf:type owl:NamedIndividual ,
                    :FacialMovement ,
                    :HumanVisualContent .


###  https://raw.githubusercontent.com/MaddaGh/DataProcessing_EmoAnnotation/main/meaw.ttl#peace
:peace rdf:type owl:NamedIndividual ,
                :Emotion ,
                :EmotionState ;
       :isIncludedIn :enjoyment ;
       rdfs:comment "An experience of ease and contentment." .


###  https://raw.githubusercontent.com/MaddaGh/DataProcessing_EmoAnnotation/main/meaw.ttl#presenting_opinion
:presenting_opinion rdf:type owl:NamedIndividual ,
                             :ConversationalFrame ;
                    rdfs:comment "A Conversational Frame where a speaker expresses their opinion on a topic, without necessarily disagreeing with other speakers, but in a neutral way." .


###  https://raw.githubusercontent.com/MaddaGh/DataProcessing_EmoAnnotation/main/meaw.ttl#press_lips
:press_lips rdf:type owl:NamedIndividual ,
                     :FacialMovement ,
                     :HumanVisualContent .


###  https://raw.githubusercontent.com/MaddaGh/DataProcessing_EmoAnnotation/main/meaw.ttl#pride
:pride rdf:type owl:NamedIndividual ,
                :Emotion ,
                :EmotionState ;
       :isIncludedIn :enjoyment ;
       rdfs:comment "Deep pleasure and satisfaction derived from one's own achievements or the achievements of an associate." .


###  https://raw.githubusercontent.com/MaddaGh/DataProcessing_EmoAnnotation/main/meaw.ttl#pucker_lip
:pucker_lip rdf:type owl:NamedIndividual ,
                     :FacialMovement ,
                     :HumanVisualContent .


###  https://raw.githubusercontent.com/MaddaGh/DataProcessing_EmoAnnotation/main/meaw.ttl#pull_lip_corner
:pull_lip_corner rdf:type owl:NamedIndividual ,
                          :FacialMovement ,
                          :HumanVisualContent .


###  https://raw.githubusercontent.com/MaddaGh/DataProcessing_EmoAnnotation/main/meaw.ttl#quick_bicker
:quick_bicker rdf:type owl:NamedIndividual ,
                       :AuralTrigger ,
                       :Trigger ;
              :triggers <https://raw.githubusercontent.com/MaddaGh/DataProcessing_EmoAnnotation/main/meaw.ttl#55_anger> .


###  https://raw.githubusercontent.com/MaddaGh/DataProcessing_EmoAnnotation/main/meaw.ttl#raise_cheek
:raise_cheek rdf:type owl:NamedIndividual ,
                      :FacialMovement ,
                      :HumanVisualContent .


###  https://raw.githubusercontent.com/MaddaGh/DataProcessing_EmoAnnotation/main/meaw.ttl#raise_chin
:raise_chin rdf:type owl:NamedIndividual ,
                     :FacialMovement ,
                     :HumanVisualContent ;
            :isShownIn <https://raw.githubusercontent.com/MaddaGh/DataProcessing_EmoAnnotation/main/meaw.ttl#58_1> .


###  https://raw.githubusercontent.com/MaddaGh/DataProcessing_EmoAnnotation/main/meaw.ttl#raise_eyebrow
:raise_eyebrow rdf:type owl:NamedIndividual ,
                        :FacialMovement ,
                        :HumanVisualContent ,
                        :Trigger ,
                        :VisualTrigger ;
               owl:sameAs :raise_outer_brow ;
               :isShownIn <https://raw.githubusercontent.com/MaddaGh/DataProcessing_EmoAnnotation/main/meaw.ttl#55_2> ,
                          <https://raw.githubusercontent.com/MaddaGh/DataProcessing_EmoAnnotation/main/meaw.ttl#55_4> ;
               :triggers <https://raw.githubusercontent.com/MaddaGh/DataProcessing_EmoAnnotation/main/meaw.ttl#55_anger> .


###  https://raw.githubusercontent.com/MaddaGh/DataProcessing_EmoAnnotation/main/meaw.ttl#raise_outer_brow
:raise_outer_brow rdf:type owl:NamedIndividual .


###  https://raw.githubusercontent.com/MaddaGh/DataProcessing_EmoAnnotation/main/meaw.ttl#raise_finger
:raise_finger rdf:type owl:NamedIndividual ,
                       :Gesture ,
                       :HandGesture ,
                       :HumanVisualContent ;
              :isShownIn <https://raw.githubusercontent.com/MaddaGh/DataProcessing_EmoAnnotation/main/meaw.ttl#46_3> .


###  https://raw.githubusercontent.com/MaddaGh/DataProcessing_EmoAnnotation/main/meaw.ttl#raise_inner_brow
:raise_inner_brow rdf:type owl:NamedIndividual ,
                           :FacialMovement ,
                           :HumanVisualContent .


###  https://raw.githubusercontent.com/MaddaGh/DataProcessing_EmoAnnotation/main/meaw.ttl#raise_outer_brow
:raise_outer_brow rdf:type owl:NamedIndividual ,
                           :FacialMovement ,
                           :HumanVisualContent ,
                           :Trigger ,
                           :VisualTrigger ;
                  :isShownIn <https://raw.githubusercontent.com/MaddaGh/DataProcessing_EmoAnnotation/main/meaw.ttl#55_2> ,
                             <https://raw.githubusercontent.com/MaddaGh/DataProcessing_EmoAnnotation/main/meaw.ttl#55_4> ;
                  :triggers <https://raw.githubusercontent.com/MaddaGh/DataProcessing_EmoAnnotation/main/meaw.ttl#55_anger> .


###  https://raw.githubusercontent.com/MaddaGh/DataProcessing_EmoAnnotation/main/meaw.ttl#raise_shoulder
:raise_shoulder rdf:type owl:NamedIndividual ,
                         :HumanVisualContent ,
                         :Kinetic ;
                :isShownIn <https://raw.githubusercontent.com/MaddaGh/DataProcessing_EmoAnnotation/main/meaw.ttl#55_1> .


###  https://raw.githubusercontent.com/MaddaGh/DataProcessing_EmoAnnotation/main/meaw.ttl#raise_upper_lid
:raise_upper_lid rdf:type owl:NamedIndividual ,
                          :FacialMovement ,
                          :HumanVisualContent .


###  https://raw.githubusercontent.com/MaddaGh/DataProcessing_EmoAnnotation/main/meaw.ttl#raise_upper_lip
:raise_upper_lip rdf:type owl:NamedIndividual ,
                          :FacialMovement ,
                          :HumanVisualContent .


###  https://raw.githubusercontent.com/MaddaGh/DataProcessing_EmoAnnotation/main/meaw.ttl#rejoicing
:rejoicing rdf:type owl:NamedIndividual ,
                    :Emotion ,
                    :EmotionState ;
           :isIncludedIn :enjoyment ;
           rdfs:comment "A warm, uplifting feeling that people experience when they see acts of human goodness, kindness and compassion. Also called elevation." .


###  https://raw.githubusercontent.com/MaddaGh/DataProcessing_EmoAnnotation/main/meaw.ttl#relief
:relief rdf:type owl:NamedIndividual ,
                 :Emotion ,
                 :EmotionState ;
        :isIncludedIn :enjoyment ;
        rdfs:comment "When something expected to be unpleasant, especially the threat of harm, is avoided or comes to an end." .


###  https://raw.githubusercontent.com/MaddaGh/DataProcessing_EmoAnnotation/main/meaw.ttl#repugnance
:repugnance rdf:type owl:NamedIndividual ,
                     :Emotion ,
                     :EmotionState ;
            :isIncludedIn :disgust ;
            rdfs:comment "Strong distaste for something, often a concept or idea." .


###  https://raw.githubusercontent.com/MaddaGh/DataProcessing_EmoAnnotation/main/meaw.ttl#resignation
:resignation rdf:type owl:NamedIndividual ,
                      :Emotion ,
                      :EmotionState ;
             :isIncludedIn :sadness ;
             rdfs:comment "The belief that nothing can be done." .


###  https://raw.githubusercontent.com/MaddaGh/DataProcessing_EmoAnnotation/main/meaw.ttl#reverse_shot
:reverse_shot rdf:type owl:NamedIndividual ,
                       :CameraAngle ,
                       :FramingTechnique ;
              rdfs:comment "Reverse Shot (RS): A shot that shows the reverse perspective of the preceding shot, typically used in conversation scenes to depict the reactions or responses of the characters." .


###  https://raw.githubusercontent.com/MaddaGh/DataProcessing_EmoAnnotation/main/meaw.ttl#revulsion
:revulsion rdf:type owl:NamedIndividual ,
                    :Emotion ,
                    :EmotionState ;
           :isIncludedIn :disgust ;
           rdfs:comment "A mixture of disgust and loathing." .


###  https://raw.githubusercontent.com/MaddaGh/DataProcessing_EmoAnnotation/main/meaw.ttl#sadness
:sadness rdf:type owl:NamedIndividual ,
                  :BasicEmotion ,
                  :Emotion ;
         :expressedIn <https://raw.githubusercontent.com/MaddaGh/DataProcessing_EmoAnnotation/main/meaw.ttl#41_sadness> ;
         :includes :anguish ,
                   :despair ,
                   :disappointment ,
                   :discouragement ,
                   :distraughtness ,
                   :grief ,
                   :helplessness ,
                   :misery ,
                   :resignation ,
                   :sorrow ;
         rdfs:comment "Sadness is a response to loss, and feeling sad allows us to take a timeout and show others that we need support (description from http://atlasofemotions.org/)." .


###  https://raw.githubusercontent.com/MaddaGh/DataProcessing_EmoAnnotation/main/meaw.ttl#saying_something_wrong
:saying_something_wrong rdf:type owl:NamedIndividual ,
                                 :ConversationalFrame .


###  https://raw.githubusercontent.com/MaddaGh/DataProcessing_EmoAnnotation/main/meaw.ttl#schadenfreude
:schadenfreude rdf:type owl:NamedIndividual ,
                        :Emotion ,
                        :EmotionState ;
               :isIncludedIn :enjoyment ;
               rdfs:comment "Enjoyment of the misfortunes of another person, usually a rival." .


###  https://raw.githubusercontent.com/MaddaGh/DataProcessing_EmoAnnotation/main/meaw.ttl#sensory_pleasure
:sensory_pleasure rdf:type owl:NamedIndividual ,
                           :Emotion ,
                           :EmotionState ;
                  :isIncludedIn :enjoyment ;
                  rdfs:comment "Enjoyment derived through one of the five physical senses: sight, sound, touch, taste and smell." .


###  https://raw.githubusercontent.com/MaddaGh/DataProcessing_EmoAnnotation/main/meaw.ttl#show_tongue
:show_tongue rdf:type owl:NamedIndividual ,
                      :FacialMovement ,
                      :HumanVisualContent .


###  https://raw.githubusercontent.com/MaddaGh/DataProcessing_EmoAnnotation/main/meaw.ttl#smiling
:smiling rdf:type owl:NamedIndividual ,
                  :FacialMovement ,
                  :HumanVisualContent ,
                  :Trigger ,
                  :VisualTrigger ;
         :isShownIn <https://raw.githubusercontent.com/MaddaGh/DataProcessing_EmoAnnotation/main/meaw.ttl#46_1> ,
                    <https://raw.githubusercontent.com/MaddaGh/DataProcessing_EmoAnnotation/main/meaw.ttl#46_2> .


###  https://raw.githubusercontent.com/MaddaGh/DataProcessing_EmoAnnotation/main/meaw.ttl#sorrow
:sorrow rdf:type owl:NamedIndividual ,
                 :Emotion ,
                 :EmotionState ;
        :expressedIn <https://raw.githubusercontent.com/MaddaGh/DataProcessing_EmoAnnotation/main/meaw.ttl#40_sadness> ,
                     <https://raw.githubusercontent.com/MaddaGh/DataProcessing_EmoAnnotation/main/meaw.ttl#41_sadness1> ;
        :isIncludedIn :sadness ;
        rdfs:comment "A feeling of distress and sadness, often caused by a loss." .


###  https://raw.githubusercontent.com/MaddaGh/DataProcessing_EmoAnnotation/main/meaw.ttl#speaker_in_background
:speaker_in_background rdf:type owl:NamedIndividual ,
                                :AuralComposition .


###  https://raw.githubusercontent.com/MaddaGh/DataProcessing_EmoAnnotation/main/meaw.ttl#stationary
:stationary rdf:type owl:NamedIndividual ,
                     :CameraMovement ,
                     :FramingTechnique .


###  https://raw.githubusercontent.com/MaddaGh/DataProcessing_EmoAnnotation/main/meaw.ttl#stressed_syllables
:stressed_syllables rdf:type owl:NamedIndividual ,
                             :AuralTrigger ,
                             :Trigger ;
                    :triggers <https://raw.githubusercontent.com/MaddaGh/DataProcessing_EmoAnnotation/main/meaw.ttl#50_anger> .


###  https://raw.githubusercontent.com/MaddaGh/DataProcessing_EmoAnnotation/main/meaw.ttl#stretch_lip
:stretch_lip rdf:type owl:NamedIndividual ,
                      :FacialMovement ,
                      :HumanVisualContent .


###  https://raw.githubusercontent.com/MaddaGh/DataProcessing_EmoAnnotation/main/meaw.ttl#stretch_mouth
:stretch_mouth rdf:type owl:NamedIndividual ,
                        :FacialMovement ,
                        :HumanVisualContent .


###  https://raw.githubusercontent.com/MaddaGh/DataProcessing_EmoAnnotation/main/meaw.ttl#strong_gesticulation
:strong_gesticulation rdf:type owl:NamedIndividual ,
                               :Gesture ,
                               :HandGesture ,
                               :HumanVisualContent ;
                      :isShownIn <https://raw.githubusercontent.com/MaddaGh/DataProcessing_EmoAnnotation/main/meaw.ttl#51_2> .


###  https://raw.githubusercontent.com/MaddaGh/DataProcessing_EmoAnnotation/main/meaw.ttl#studio_audience
:studio_audience rdf:type owl:NamedIndividual ,
                          :Agent ,
                          :Group ,
                          :Role ;
                 rdfs:comment "A group agent, representing all the people sitting in the studio during the talk show, as a characteristic of the television talk show genre, they usually are common people that can intervene alongside invited guests. The studio audience can have collective reactions to the discourse taking place, such as clapping, cheereing, booing and so on. It might happen that an utterance has no individual speaker but shows in fact, a collective display of emotion by the studio audience. In these cases, the studio audience is considered as the agent expressing the emotion." .


###  https://raw.githubusercontent.com/MaddaGh/DataProcessing_EmoAnnotation/main/meaw.ttl#suck_lip
:suck_lip rdf:type owl:NamedIndividual ,
                   :FacialMovement ,
                   :HumanVisualContent .


###  https://raw.githubusercontent.com/MaddaGh/DataProcessing_EmoAnnotation/main/meaw.ttl#surprise
:surprise rdf:type owl:NamedIndividual ,
                   :BasicEmotion ,
                   :Emotion .


###  https://raw.githubusercontent.com/MaddaGh/DataProcessing_EmoAnnotation/main/meaw.ttl#tense_articulation
:tense_articulation rdf:type owl:NamedIndividual ,
                             :AuralTrigger ,
                             :Trigger ;
                    :triggers <https://raw.githubusercontent.com/MaddaGh/DataProcessing_EmoAnnotation/main/meaw.ttl#51_anger> ,
                              <https://raw.githubusercontent.com/MaddaGh/DataProcessing_EmoAnnotation/main/meaw.ttl#58_anger> .


###  https://raw.githubusercontent.com/MaddaGh/DataProcessing_EmoAnnotation/main/meaw.ttl#terror
:terror rdf:type owl:NamedIndividual ,
                 :Emotion ,
                 :EmotionState ;
        :isIncludedIn :fear ;
        rdfs:comment "Intense, overpowering fear." .


###  https://raw.githubusercontent.com/MaddaGh/DataProcessing_EmoAnnotation/main/meaw.ttl#tighten_lid
:tighten_lid rdf:type owl:NamedIndividual ,
                      :FacialMovement ,
                      :HumanVisualContent .


###  https://raw.githubusercontent.com/MaddaGh/DataProcessing_EmoAnnotation/main/meaw.ttl#tighten_lips
:tighten_lips rdf:type owl:NamedIndividual ,
                       :FacialMovement ,
                       :HumanVisualContent .


###  https://raw.githubusercontent.com/MaddaGh/DataProcessing_EmoAnnotation/main/meaw.ttl#tighten_neck
:tighten_neck rdf:type owl:NamedIndividual ,
                       :FacialMovement ,
                       :HumanVisualContent .


###  https://raw.githubusercontent.com/MaddaGh/DataProcessing_EmoAnnotation/main/meaw.ttl#tilt_down
:tilt_down rdf:type owl:NamedIndividual ,
                    :CameraMovement ,
                    :FramingTechnique ;
           rdfs:comment "Tilt: A camera movement where the camera tilts vertically, pointing downward from a fixed position. Tilting is employed to reveal or emphasize vertical elements in the scene, such as tall buildings or characters." .


###  https://raw.githubusercontent.com/MaddaGh/DataProcessing_EmoAnnotation/main/meaw.ttl#tilt_up
:tilt_up rdf:type owl:NamedIndividual ,
                  :CameraMovement ,
                  :FramingTechnique ;
         rdfs:comment "Tilt: A camera movement where the camera tilts vertically, pointing upward from a fixed position. Tilting is employed to reveal or emphasize vertical elements in the scene, such as tall buildings or characters." .


###  https://raw.githubusercontent.com/MaddaGh/DataProcessing_EmoAnnotation/main/meaw.ttl#tracking_shot
:tracking_shot rdf:type owl:NamedIndividual ,
                        :CameraMovement ,
                        :FramingTechnique ;
               rdfs:comment "Tracking Shot: Involves moving the camera along a predetermined path to follow the action." .


###  https://raw.githubusercontent.com/MaddaGh/DataProcessing_EmoAnnotation/main/meaw.ttl#trepidation
:trepidation rdf:type owl:NamedIndividual ,
                      :Emotion ,
                      :EmotionState ;
             rdfs:comment "Anticipation of the possibility of danger." .


###  https://raw.githubusercontent.com/MaddaGh/DataProcessing_EmoAnnotation/main/meaw.ttl#turning_towards_interlocutor
:turning_towards_interlocutor rdf:type owl:NamedIndividual ,
                                       :HumanVisualContent ,
                                       :Kinetic ;
                              :isShownIn <https://raw.githubusercontent.com/MaddaGh/DataProcessing_EmoAnnotation/main/meaw.ttl#55_1> .


###  https://raw.githubusercontent.com/MaddaGh/DataProcessing_EmoAnnotation/main/meaw.ttl#unknown
:unknown rdf:type owl:NamedIndividual ,
                  :Gender .


###  https://raw.githubusercontent.com/MaddaGh/DataProcessing_EmoAnnotation/main/meaw.ttl#upward_rolling_eye
:upward_rolling_eye rdf:type owl:NamedIndividual ,
                             :EyeMovement ,
                             :FacialMovement ,
                             :HumanVisualContent .


###  https://raw.githubusercontent.com/MaddaGh/DataProcessing_EmoAnnotation/main/meaw.ttl#vengefulness
:vengefulness rdf:type owl:NamedIndividual ,
                       :Emotion ,
                       :EmotionState ;
              :isIncludedIn :anger ;
              rdfs:comment "Desire to retaliate after one is hurt." .


###  https://raw.githubusercontent.com/MaddaGh/DataProcessing_EmoAnnotation/main/meaw.ttl#vertical_high
:vertical_high rdf:type owl:NamedIndividual ,
                        :CameraAngle ,
                        :FramingTechnique .


###  https://raw.githubusercontent.com/MaddaGh/DataProcessing_EmoAnnotation/main/meaw.ttl#vertical_low
:vertical_low rdf:type owl:NamedIndividual ,
                       :CameraAngle ,
                       :FramingTechnique .


###  https://raw.githubusercontent.com/MaddaGh/DataProcessing_EmoAnnotation/main/meaw.ttl#vertical_median
:vertical_median rdf:type owl:NamedIndividual ,
                          :CameraAngle ,
                          :FramingTechnique .


###  https://raw.githubusercontent.com/MaddaGh/DataProcessing_EmoAnnotation/main/meaw.ttl#voiceover
:voiceover rdf:type owl:NamedIndividual ,
                    :AuralComposition .


###  https://raw.githubusercontent.com/MaddaGh/DataProcessing_EmoAnnotation/main/meaw.ttl#walking
:walking rdf:type owl:NamedIndividual ,
                  :HumanVisualContent ,
                  :Kinetic ;
         :isShownIn <https://raw.githubusercontent.com/MaddaGh/DataProcessing_EmoAnnotation/main/meaw.ttl#40_1> ,
                    <https://raw.githubusercontent.com/MaddaGh/DataProcessing_EmoAnnotation/main/meaw.ttl#40_2> ,
                    <https://raw.githubusercontent.com/MaddaGh/DataProcessing_EmoAnnotation/main/meaw.ttl#45_1> ,
                    <https://raw.githubusercontent.com/MaddaGh/DataProcessing_EmoAnnotation/main/meaw.ttl#57_1> .


###  https://raw.githubusercontent.com/MaddaGh/DataProcessing_EmoAnnotation/main/meaw.ttl#welles_nietes
:welles_nietes rdf:type owl:NamedIndividual ,
                        :TalkShow ;
               :broadcastedBy :ncrv ;
               :hasInScope <https://raw.githubusercontent.com/MaddaGh/DataProcessing_EmoAnnotation/main/meaw.ttl#40_neutrality> ,
                           <https://raw.githubusercontent.com/MaddaGh/DataProcessing_EmoAnnotation/main/meaw.ttl#41_sadness> ,
                           <https://raw.githubusercontent.com/MaddaGh/DataProcessing_EmoAnnotation/main/meaw.ttl#43_fear> ,
                           <https://raw.githubusercontent.com/MaddaGh/DataProcessing_EmoAnnotation/main/meaw.ttl#45_neutrality> ,
                           <https://raw.githubusercontent.com/MaddaGh/DataProcessing_EmoAnnotation/main/meaw.ttl#46_fear> ,
                           <https://raw.githubusercontent.com/MaddaGh/DataProcessing_EmoAnnotation/main/meaw.ttl#50_anger> ,
                           <https://raw.githubusercontent.com/MaddaGh/DataProcessing_EmoAnnotation/main/meaw.ttl#51_anger> ,
                           <https://raw.githubusercontent.com/MaddaGh/DataProcessing_EmoAnnotation/main/meaw.ttl#55_anger> ,
                           <https://raw.githubusercontent.com/MaddaGh/DataProcessing_EmoAnnotation/main/meaw.ttl#57_disgust> ,
                           <https://raw.githubusercontent.com/MaddaGh/DataProcessing_EmoAnnotation/main/meaw.ttl#58_anger> ;
               :hasDate "1988-03-19" ;
               :hasDescription "Discussie over de stelling: 'Mag je op televisie zeggen wat je denkt?'. Discussiedeelnemers: voor- en tegenstanders in het publiek, onder wie Adelheid Roosen, Paul de Leeuw, mr. A. Duijser, algemeen directeur NCRV en vijf panelleden. De discussie wordt geleid door Legien Kromkamp." ,
                               "Laatste 'Welles nietes' van het seizoen. Dit keer gaat het om gekwetst worden door iets op de televisie. Actrice Adelheid Roosen, bekend van 'De nacht', en acteur Paul de Leeuw bevinden zich te midden van een merendeels conservatief publiek. Confrontaties kunnen niet uitblijven. Adelheid Roosen vat de discussie sportief op. Ze biedt haar opponenten een waterpistool aan waarmee ze haar mogen natspuiten. Een vrouw gaat in op dit aanbod." ,
                               "Pittige maatschappelijke discussies onder leiding van Legien Kromkamp over een bepaalde stelling. Voor- en tegenstanders zetten hun argumenten uiteen en proberen zo de mening van de vijf vaste panelleden te beïnvloeden. Allerlei vraagstukken komen aan bod. Van drugsproblematiek, armoede of voetbalgeweld tot het milieu en amusement op televisie. Aan het einde van de aflevering wordt de stelling voor de volgende uitzending bekendgemaakt. Kijkers kunnen hierop reageren en enkelen worden uitgenodigd om in de studio deel te nemen aan de discussie. Het programma is te zien geweest van 1985 tot en met 1990. Felle reacties De NCRV krijgt veel brieven op de uitzendingen. Sommige onderwerpen roepen tegengestelde reacties op bij de achterban. Maar ook het taalgebruik leidt tot een stroom aan reacties. In een discussie wordt nogal eens gevloekt of grove taal geuit, voor menig kijker reden genoeg om in de pen te klimmen." ,
                               "Tweewekelijks praatprogramma waarin gediscussieerd wordt over een stelling, waarna de panelleden zich voor of tegen de stelling uitspreken." ;
               :hasFileName "WELLESNIETES_-HRE0000551A" ;
               :hasIdentifier "2101608040029452931" ;
               :hasTitle "WELLES NIETES - WELLES NIETES;Mag je op televisie zeggen wat je denkt?" ;
               :isAbout "televisie, vrijheid van meningsuiting" .


###  https://raw.githubusercontent.com/MaddaGh/DataProcessing_EmoAnnotation/main/meaw.ttl#wonder
:wonder rdf:type owl:NamedIndividual ,
                 :Emotion ,
                 :EmotionState ;
        :isIncludedIn :enjoyment ;
        rdfs:comment "An experience of something that is very surprising, beautiful, amazing or hard to believe." .


###  https://raw.githubusercontent.com/MaddaGh/DataProcessing_EmoAnnotation/main/meaw.ttl#wrink_nose
:wrink_nose rdf:type owl:NamedIndividual ,
                     :FacialMovement ,
                     :HumanVisualContent .


###  https://raw.githubusercontent.com/MaddaGh/DataProcessing_EmoAnnotation/main/meaw.ttl#zoom_in
:zoom_in rdf:type owl:NamedIndividual ,
                  :CameraMovement ,
                  :FramingTechnique ;
         rdfs:comment "Zoom Shot: Adjusts the focal length of the lens to make the subject appear closer, creating a dynamic effect." .


###  https://raw.githubusercontent.com/MaddaGh/DataProcessing_EmoAnnotation/main/meaw.ttl#zoom_out
:zoom_out rdf:type owl:NamedIndividual ,
                   :CameraMovement ,
                   :FramingTechnique ;
          rdfs:comment "Zoom Shot: Adjusts the focal length of the lens to make the subject appear farther away, creating a dynamic effect." .


###  https://raw.githubusercontent.com/MaddaGh/DataProcessing_EmoAnnotation/main/meaw.ttl#2101608040029452931_guest
<https://raw.githubusercontent.com/MaddaGh/DataProcessing_EmoAnnotation/main/meaw.ttl#2101608040029452931_guest> rdf:type owl:NamedIndividual ,
                                                                                                                          :ConversationalRolePlay ;
                                                                                                                 :hasConversationalContext :welles_nietes ;
                                                                                                                 :hasRole :guest ;
                                                                                                                 :isRolePlayOf :adelheid_roosen ;
                                                                                                                 rdfs:comment "The role of guest in the TalkShowSituation Welles Nietes: WELLES NIETES - WELLES NIETES;Mag je op televisie zeggen wat je denkt?" .


###  https://raw.githubusercontent.com/MaddaGh/DataProcessing_EmoAnnotation/main/meaw.ttl#2101608040029452931_host
<https://raw.githubusercontent.com/MaddaGh/DataProcessing_EmoAnnotation/main/meaw.ttl#2101608040029452931_host> rdf:type owl:NamedIndividual ,
                                                                                                                         :ConversationalRolePlay ;
                                                                                                                :hasConversationalContext :welles_nietes ;
                                                                                                                :hasRole :host ;
                                                                                                                :isRolePlayOf :legien_kromkamp ;
                                                                                                                rdfs:comment "The role of host in the TalkShowSituation Welles Nietes: WELLES NIETES - WELLES NIETES;Mag je op televisie zeggen wat je denkt?" .


###  https://raw.githubusercontent.com/MaddaGh/DataProcessing_EmoAnnotation/main/meaw.ttl#2101608040029452931_studio_audience
<https://raw.githubusercontent.com/MaddaGh/DataProcessing_EmoAnnotation/main/meaw.ttl#2101608040029452931_studio_audience> rdf:type owl:NamedIndividual ,
                                                                                                                                    :ConversationalRolePlay ;
                                                                                                                           :hasConversationalContext :welles_nietes ;
                                                                                                                           :hasRole :studio_audience ;
                                                                                                                           :isRolePlayOf :anonymous ,
                                                                                                                                         :anonymous1 ;
                                                                                                                           rdfs:comment "The role of studio audience in the TalkShowSituation Welles Nietes: WELLES NIETES - WELLES NIETES;Mag je op televisie zeggen wat je denkt?" .


###  https://raw.githubusercontent.com/MaddaGh/DataProcessing_EmoAnnotation/main/meaw.ttl#40_1
<https://raw.githubusercontent.com/MaddaGh/DataProcessing_EmoAnnotation/main/meaw.ttl#40_1> rdf:type owl:NamedIndividual ,
                                                                                                     :Frame ;
                                                                                            :frames <https://raw.githubusercontent.com/MaddaGh/DataProcessing_EmoAnnotation/main/meaw.ttl#40_neutrality> ;
                                                                                            :hasAngle :horizontal_oblique ;
                                                                                            :hasAuralComposition :aligned ;
                                                                                            :hasFramingTechnique :horizontal_oblique ,
                                                                                                                 :long_shot ,
                                                                                                                 :stationary ;
                                                                                            :hasMovement :stationary ;
                                                                                            :hasShotType :long_shot ;
                                                                                            :precedes <https://raw.githubusercontent.com/MaddaGh/DataProcessing_EmoAnnotation/main/meaw.ttl#40_2> ;
                                                                                            :shows :walking ;
                                                                                            :showsMovement :walking .


###  https://raw.githubusercontent.com/MaddaGh/DataProcessing_EmoAnnotation/main/meaw.ttl#40_2
<https://raw.githubusercontent.com/MaddaGh/DataProcessing_EmoAnnotation/main/meaw.ttl#40_2> rdf:type owl:NamedIndividual ,
                                                                                                     :Frame ;
                                                                                            :follows <https://raw.githubusercontent.com/MaddaGh/DataProcessing_EmoAnnotation/main/meaw.ttl#40_1> ;
                                                                                            :frames <https://raw.githubusercontent.com/MaddaGh/DataProcessing_EmoAnnotation/main/meaw.ttl#40_neutrality> ;
                                                                                            :hasAngle :horizontal_frontal ;
                                                                                            :hasAuralComposition :aligned ;
                                                                                            :hasFramingTechnique :horizontal_frontal ,
                                                                                                                 :medium_long_shot ,
                                                                                                                 :tracking_shot ;
                                                                                            :hasMovement :tracking_shot ;
                                                                                            :hasShotType :medium_long_shot ;
                                                                                            :shows :walking ;
                                                                                            :showsMovement :walking .


###  https://raw.githubusercontent.com/MaddaGh/DataProcessing_EmoAnnotation/main/meaw.ttl#40_neutrality
<https://raw.githubusercontent.com/MaddaGh/DataProcessing_EmoAnnotation/main/meaw.ttl#40_neutrality> rdf:type owl:NamedIndividual ,
                                                                                                              :EmotionAnnotation ;
                                                                                                     :experiencer :legien_kromkamp ;
                                                                                                     :framedBy <https://raw.githubusercontent.com/MaddaGh/DataProcessing_EmoAnnotation/main/meaw.ttl#40_1> ,
                                                                                                               <https://raw.githubusercontent.com/MaddaGh/DataProcessing_EmoAnnotation/main/meaw.ttl#40_2> ;
                                                                                                     :hasCameraFramingInterpretation :contextualizing ;
                                                                                                     :hasFrameContext :introducing_topic ;
                                                                                                     :isInScopeOf :welles_nietes ;
                                                                                                     :hasStart "394" ;
                                                                                                     :hasText "In de zaal zijn nogal wat mensen die zeggen tegen ons wij zijn af en toe best gekwetst door wat er op de televisie getoond wordt u knikt ja u knikt." ;
                                                                                                     rdfs:comment "EmotionRelation, the individual naming convention is the sequence number of the utterance + the annotated emotion." .


###  https://raw.githubusercontent.com/MaddaGh/DataProcessing_EmoAnnotation/main/meaw.ttl#40_sadness
<https://raw.githubusercontent.com/MaddaGh/DataProcessing_EmoAnnotation/main/meaw.ttl#40_sadness> rdf:type owl:NamedIndividual ,
                                                                                                           :AppraisedEmotionAnnotation ,
                                                                                                           :EmotionAnnotation ,
                                                                                                           :PastEmotionAnnotation ;
                                                                                                  :emotion :sorrow ;
                                                                                                  :hasTrigger :gekwetst ;
                                                                                                  :hasVerbalTrigger :gekwetst ;
                                                                                                  :hasStart "394" ;
                                                                                                  :hasText "In de zaal zijn nogal wat mensen die zeggen tegen ons wij zijn af en toe best gekwetst door wat er op de televisie getoond wordt u knikt ja u knikt." .


###  https://raw.githubusercontent.com/MaddaGh/DataProcessing_EmoAnnotation/main/meaw.ttl#41_1
<https://raw.githubusercontent.com/MaddaGh/DataProcessing_EmoAnnotation/main/meaw.ttl#41_1> rdf:type owl:NamedIndividual ,
                                                                                                     :Frame ;
                                                                                            :frames <https://raw.githubusercontent.com/MaddaGh/DataProcessing_EmoAnnotation/main/meaw.ttl#41_sadness> ;
                                                                                            :hasAngle :horizontal_frontal ;
                                                                                            :hasAuralComposition :speaker_in_background ;
                                                                                            :hasFramingTechnique :horizontal_frontal ,
                                                                                                                 :medium_long_shot ,
                                                                                                                 :tracking_shot ;
                                                                                            :hasMovement :tracking_shot ;
                                                                                            :hasShotType :medium_long_shot ;
                                                                                            :precedes <https://raw.githubusercontent.com/MaddaGh/DataProcessing_EmoAnnotation/main/meaw.ttl#41_2> .


###  https://raw.githubusercontent.com/MaddaGh/DataProcessing_EmoAnnotation/main/meaw.ttl#41_2
<https://raw.githubusercontent.com/MaddaGh/DataProcessing_EmoAnnotation/main/meaw.ttl#41_2> rdf:type owl:NamedIndividual ,
                                                                                                     :Frame ;
                                                                                            :follows <https://raw.githubusercontent.com/MaddaGh/DataProcessing_EmoAnnotation/main/meaw.ttl#41_1> ;
                                                                                            :frames <https://raw.githubusercontent.com/MaddaGh/DataProcessing_EmoAnnotation/main/meaw.ttl#41_sadness> ;
                                                                                            :hasAngle :horizontal_oblique ;
                                                                                            :hasAuralComposition :aligned ;
                                                                                            :hasFramingTechnique :horizontal_oblique ,
                                                                                                                 :medium_shot ,
                                                                                                                 :stationary ;
                                                                                            :hasMovement :stationary ;
                                                                                            :hasShotType :medium_shot .


###  https://raw.githubusercontent.com/MaddaGh/DataProcessing_EmoAnnotation/main/meaw.ttl#41_3
<https://raw.githubusercontent.com/MaddaGh/DataProcessing_EmoAnnotation/main/meaw.ttl#41_3> rdf:type owl:NamedIndividual ,
                                                                                                     :Frame ;
                                                                                            :hasAngle :horizontal_frontal ;
                                                                                            :hasAuralComposition :aligned ;
                                                                                            :hasFramingTechnique :horizontal_frontal ,
                                                                                                                 :medium_close_up ,
                                                                                                                 :stationary ;
                                                                                            :hasMovement :stationary ;
                                                                                            :hasShotType :medium_close_up ;
                                                                                            :shows :head_shake_side_to_side ,
                                                                                                   :headshake ,
                                                                                                   :make_eye_contact ;
                                                                                            :showsEyes :make_eye_contact ;
                                                                                            :showsHeadGesture :head_shake_side_to_side ,
                                                                                                              :headshake .


###  https://raw.githubusercontent.com/MaddaGh/DataProcessing_EmoAnnotation/main/meaw.ttl#41_sadness
<https://raw.githubusercontent.com/MaddaGh/DataProcessing_EmoAnnotation/main/meaw.ttl#41_sadness> rdf:type owl:NamedIndividual ,
                                                                                                           :EmotionAnnotation ,
                                                                                                           :ExperiencedEmotionAnnotation ,
                                                                                                           :PresentEmotionAnnotation ;
                                                                                                  :emotion :sadness ;
                                                                                                  :experiencer :anonymous ;
                                                                                                  :framedBy <https://raw.githubusercontent.com/MaddaGh/DataProcessing_EmoAnnotation/main/meaw.ttl#41_1> ,
                                                                                                            <https://raw.githubusercontent.com/MaddaGh/DataProcessing_EmoAnnotation/main/meaw.ttl#41_2> ;
                                                                                                  :hasCameraFramingInterpretation :engaging_with ;
                                                                                                  :hasFrameContext :presenting_opinion ;
                                                                                                  :hasTrigger :gekwetst ;
                                                                                                  :hasVerbalTrigger :gekwetst ;
                                                                                                  :isInScopeOf :welles_nietes ;
                                                                                                  :hasEnd "" ;
                                                                                                  :hasStart "405" ;
                                                                                                  :hasText "Na jaren gekwetst door de laatste uitzending van adelheid roosen over de transseksuele ik vond dat het in het belachelijke getrokken werd en ik denk dus dat er een heleboel mensen daardoor gekwetst zijn want werd in het seksuele vlak getrokken en dat vond ik dus niet goed." .


###  https://raw.githubusercontent.com/MaddaGh/DataProcessing_EmoAnnotation/main/meaw.ttl#41_sadness1
<https://raw.githubusercontent.com/MaddaGh/DataProcessing_EmoAnnotation/main/meaw.ttl#41_sadness1> rdf:type owl:NamedIndividual ,
                                                                                                            :AppraisedEmotionAnnotation ,
                                                                                                            :EmotionAnnotation ,
                                                                                                            :PastEmotionAnnotation ;
                                                                                                   :emotion :sorrow ;
                                                                                                   :hasTrigger :mensen_gekwetst_zijn ;
                                                                                                   :hasVerbalTrigger :mensen_gekwetst_zijn ;
                                                                                                   :hasStart "405" ;
                                                                                                   :hasText "Na jaren gekwetst door de laatste uitzending van adelheid roosen over de transseksuele ik vond dat het in het belachelijke getrokken werd en ik denk dus dat er een heleboel mensen daardoor gekwetst zijn want werd in het seksuele vlak getrokken en dat vond ik dus niet goed" .


###  https://raw.githubusercontent.com/MaddaGh/DataProcessing_EmoAnnotation/main/meaw.ttl#43_1
<https://raw.githubusercontent.com/MaddaGh/DataProcessing_EmoAnnotation/main/meaw.ttl#43_1> rdf:type owl:NamedIndividual ,
                                                                                                     :Frame ;
                                                                                            :frames <https://raw.githubusercontent.com/MaddaGh/DataProcessing_EmoAnnotation/main/meaw.ttl#43_fear> ;
                                                                                            :hasAngle :horizontal_frontal ;
                                                                                            :hasAuralComposition :aligned ;
                                                                                            :hasFramingTechnique :horizontal_frontal ,
                                                                                                                 :medium_close_up ,
                                                                                                                 :stationary ;
                                                                                            :hasMovement :stationary ;
                                                                                            :hasShotType :medium_close_up ;
                                                                                            :precedes <https://raw.githubusercontent.com/MaddaGh/DataProcessing_EmoAnnotation/main/meaw.ttl#43_2> ;
                                                                                            :shows :eyes_up ,
                                                                                                   :head_shake_up_and_down ;
                                                                                            :showsEyes :eyes_up ;
                                                                                            :showsHeadGesture :head_shake_up_and_down .


###  https://raw.githubusercontent.com/MaddaGh/DataProcessing_EmoAnnotation/main/meaw.ttl#43_2
<https://raw.githubusercontent.com/MaddaGh/DataProcessing_EmoAnnotation/main/meaw.ttl#43_2> rdf:type owl:NamedIndividual ,
                                                                                                     :Frame ;
                                                                                            :follows <https://raw.githubusercontent.com/MaddaGh/DataProcessing_EmoAnnotation/main/meaw.ttl#43_1> ;
                                                                                            :frames <https://raw.githubusercontent.com/MaddaGh/DataProcessing_EmoAnnotation/main/meaw.ttl#43_fear> ;
                                                                                            :hasAngle :reverse_shot ;
                                                                                            :hasAuralComposition :voiceover ;
                                                                                            :hasFramingTechnique :medium_close_up ,
                                                                                                                 :reverse_shot ,
                                                                                                                 :stationary ;
                                                                                            :hasMovement :stationary ;
                                                                                            :hasShotType :medium_close_up ;
                                                                                            :shows :frowning ,
                                                                                                   :head_down ,
                                                                                                   :lower_brow ;
                                                                                            :showsExpression :frowning ,
                                                                                                             :lower_brow ;
                                                                                            :showsHeadGesture :head_down .


###  https://raw.githubusercontent.com/MaddaGh/DataProcessing_EmoAnnotation/main/meaw.ttl#43_anger
<https://raw.githubusercontent.com/MaddaGh/DataProcessing_EmoAnnotation/main/meaw.ttl#43_anger> rdf:type owl:NamedIndividual ,
                                                                                                         :EmotionAnnotation ,
                                                                                                         :ExperiencedEmotionAnnotation ,
                                                                                                         :PastEmotionAnnotation ;
                                                                                                :emotion :annoyance ;
                                                                                                :hasTrigger :ik_vond_het_heel_vervelend ;
                                                                                                :hasVerbalTrigger :ik_vond_het_heel_vervelend ;
                                                                                                :hasStart "431" ;
                                                                                                :hasText "Nou ja ze begonnen dus mee met die bossen te schreeuwen en dergelijke op een vervelende manier ja ik ben doodzenuwachtig dat dat mag misschien wel maar ik vond het heel vervelend want er lopen een heleboel van die mensen rond ik heb zelf persoonlijk eentje gekend" .


###  https://raw.githubusercontent.com/MaddaGh/DataProcessing_EmoAnnotation/main/meaw.ttl#43_fear
<https://raw.githubusercontent.com/MaddaGh/DataProcessing_EmoAnnotation/main/meaw.ttl#43_fear> rdf:type owl:NamedIndividual ,
                                                                                                        :EmotionAnnotation ,
                                                                                                        :ExperiencedEmotionAnnotation ,
                                                                                                        :PresentEmotionAnnotation ;
                                                                                               :emotion :fear ;
                                                                                               :experiencer :anonymous ;
                                                                                               :framedBy <https://raw.githubusercontent.com/MaddaGh/DataProcessing_EmoAnnotation/main/meaw.ttl#43_1> ,
                                                                                                         <https://raw.githubusercontent.com/MaddaGh/DataProcessing_EmoAnnotation/main/meaw.ttl#43_2> ;
                                                                                               :hasCameraFramingInterpretation :involvement ;
                                                                                               :hasFrameContext :argumenting_with_personal_experience ;
                                                                                               :hasTrigger :ik_ben_doodzenuwachtig ;
                                                                                               :hasVerbalTrigger :ik_ben_doodzenuwachtig ;
                                                                                               :isInScopeOf :welles_nietes ;
                                                                                               :hasStart "431" ;
                                                                                               :hasText "Nou ja ze begonnen dus mee met die bossen te schreeuwen en dergelijke op een vervelende manier ja ik ben doodzenuwachtig dat dat mag misschien wel maar ik vond het heel vervelend want er lopen een heleboel van die mensen rond ik heb zelf persoonlijk eentje gekend." .


###  https://raw.githubusercontent.com/MaddaGh/DataProcessing_EmoAnnotation/main/meaw.ttl#45_1
<https://raw.githubusercontent.com/MaddaGh/DataProcessing_EmoAnnotation/main/meaw.ttl#45_1> rdf:type owl:NamedIndividual ,
                                                                                                     :Frame ;
                                                                                            :frames <https://raw.githubusercontent.com/MaddaGh/DataProcessing_EmoAnnotation/main/meaw.ttl#45_neutrality> ;
                                                                                            :hasAngle :horizontal_frontal ;
                                                                                            :hasAuralComposition :aligned ;
                                                                                            :hasFramingTechnique :horizontal_frontal ,
                                                                                                                 :medium_long_shot ,
                                                                                                                 :tracking_shot ;
                                                                                            :hasMovement :tracking_shot ;
                                                                                            :hasShotType :medium_long_shot ;
                                                                                            :precedes <https://raw.githubusercontent.com/MaddaGh/DataProcessing_EmoAnnotation/main/meaw.ttl#45_2> ;
                                                                                            :shows :walking ;
                                                                                            :showsMovement :walking .


###  https://raw.githubusercontent.com/MaddaGh/DataProcessing_EmoAnnotation/main/meaw.ttl#45_2
<https://raw.githubusercontent.com/MaddaGh/DataProcessing_EmoAnnotation/main/meaw.ttl#45_2> rdf:type owl:NamedIndividual ,
                                                                                                     :Frame ;
                                                                                            :follows <https://raw.githubusercontent.com/MaddaGh/DataProcessing_EmoAnnotation/main/meaw.ttl#45_1> ;
                                                                                            :frames <https://raw.githubusercontent.com/MaddaGh/DataProcessing_EmoAnnotation/main/meaw.ttl#45_neutrality> ;
                                                                                            :hasAngle :horizontal_frontal ;
                                                                                            :hasAuralComposition :voiceover ;
                                                                                            :hasFramingTechnique :horizontal_frontal ,
                                                                                                                 :medium_close_up ,
                                                                                                                 :stationary ;
                                                                                            :hasMovement :stationary ;
                                                                                            :hasShotType :medium_close_up ;
                                                                                            :shows :head_shake_up_and_down ,
                                                                                                   :make_eye_contact ;
                                                                                            :showsEyes :make_eye_contact ;
                                                                                            :showsHeadGesture :head_shake_up_and_down .


###  https://raw.githubusercontent.com/MaddaGh/DataProcessing_EmoAnnotation/main/meaw.ttl#45_neutrality
<https://raw.githubusercontent.com/MaddaGh/DataProcessing_EmoAnnotation/main/meaw.ttl#45_neutrality> rdf:type owl:NamedIndividual ,
                                                                                                              :EmotionAnnotation ;
                                                                                                     :experiencer :legien_kromkamp ;
                                                                                                     :framedBy <https://raw.githubusercontent.com/MaddaGh/DataProcessing_EmoAnnotation/main/meaw.ttl#45_1> ,
                                                                                                               <https://raw.githubusercontent.com/MaddaGh/DataProcessing_EmoAnnotation/main/meaw.ttl#45_2> ;
                                                                                                     :hasCameraFramingInterpretation :engaging_with ;
                                                                                                     :hasFrameContext :giving_talking_space ;
                                                                                                     :isInScopeOf :welles_nietes ;
                                                                                                     :hasEnd "" ;
                                                                                                     :hasStart "454" ;
                                                                                                     :hasText "Nou ze adelheid u zegt het is kwetsend aan het zit bij ons in de studio we hebben van veel mensen gehoord dat een nacht zo kwetsend is die manier hÃ¨ die je bij jou in de uitzending was mevrouw mevrouw." .


###  https://raw.githubusercontent.com/MaddaGh/DataProcessing_EmoAnnotation/main/meaw.ttl#46_1
<https://raw.githubusercontent.com/MaddaGh/DataProcessing_EmoAnnotation/main/meaw.ttl#46_1> rdf:type owl:NamedIndividual ,
                                                                                                     :Frame ;
                                                                                            :frames <https://raw.githubusercontent.com/MaddaGh/DataProcessing_EmoAnnotation/main/meaw.ttl#46_fear> ;
                                                                                            :hasAngle :horizontal_frontal ;
                                                                                            :hasAuralComposition :voiceover ;
                                                                                            :hasFramingTechnique :horizontal_frontal ,
                                                                                                                 :medium_close_up ,
                                                                                                                 :stationary ;
                                                                                            :hasMovement :stationary ;
                                                                                            :hasShotType :medium_close_up ;
                                                                                            :precedes <https://raw.githubusercontent.com/MaddaGh/DataProcessing_EmoAnnotation/main/meaw.ttl#46_2> ;
                                                                                            :shows :smiling ;
                                                                                            :showsExpression :smiling .


###  https://raw.githubusercontent.com/MaddaGh/DataProcessing_EmoAnnotation/main/meaw.ttl#46_2
<https://raw.githubusercontent.com/MaddaGh/DataProcessing_EmoAnnotation/main/meaw.ttl#46_2> rdf:type owl:NamedIndividual ,
                                                                                                     :Frame ;
                                                                                            :follows <https://raw.githubusercontent.com/MaddaGh/DataProcessing_EmoAnnotation/main/meaw.ttl#46_1> ;
                                                                                            :frames <https://raw.githubusercontent.com/MaddaGh/DataProcessing_EmoAnnotation/main/meaw.ttl#46_fear> ;
                                                                                            :hasAngle :horizontal_oblique ;
                                                                                            :hasAuralComposition :aligned ;
                                                                                            :hasFramingTechnique :horizontal_oblique ,
                                                                                                                 :medium_shot ,
                                                                                                                 :stationary ;
                                                                                            :hasMovement :stationary ;
                                                                                            :hasShotType :medium_shot ;
                                                                                            :precedes <https://raw.githubusercontent.com/MaddaGh/DataProcessing_EmoAnnotation/main/meaw.ttl#46_3> ;
                                                                                            :shows :cover_mouth ,
                                                                                                   :head_shake_up_and_down ,
                                                                                                   :make_eye_contact ,
                                                                                                   :smiling ;
                                                                                            :showsExpression :smiling ;
                                                                                            :showsEyes :make_eye_contact ;
                                                                                            :showsHandGesture :cover_mouth ;
                                                                                            :showsHeadGesture :head_shake_up_and_down .


###  https://raw.githubusercontent.com/MaddaGh/DataProcessing_EmoAnnotation/main/meaw.ttl#46_3
<https://raw.githubusercontent.com/MaddaGh/DataProcessing_EmoAnnotation/main/meaw.ttl#46_3> rdf:type owl:NamedIndividual ,
                                                                                                     :Frame ;
                                                                                            :follows <https://raw.githubusercontent.com/MaddaGh/DataProcessing_EmoAnnotation/main/meaw.ttl#46_2> ;
                                                                                            :frames <https://raw.githubusercontent.com/MaddaGh/DataProcessing_EmoAnnotation/main/meaw.ttl#46_fear> ;
                                                                                            :hasAngle :horizontal_oblique ;
                                                                                            :hasAuralComposition :aligned ;
                                                                                            :hasFramingTechnique :horizontal_oblique ,
                                                                                                                 :medium_close_up ,
                                                                                                                 :stationary ;
                                                                                            :hasMovement :stationary ;
                                                                                            :hasShotType :medium_close_up ;
                                                                                            :shows :make_eye_contact ,
                                                                                                   :raise_finger ;
                                                                                            :showsEyes :make_eye_contact ;
                                                                                            :showsHandGesture :raise_finger .


###  https://raw.githubusercontent.com/MaddaGh/DataProcessing_EmoAnnotation/main/meaw.ttl#46_fear
<https://raw.githubusercontent.com/MaddaGh/DataProcessing_EmoAnnotation/main/meaw.ttl#46_fear> rdf:type owl:NamedIndividual ,
                                                                                                        :EmotionAnnotation ,
                                                                                                        :ExperiencedEmotionAnnotation ,
                                                                                                        :PresentEmotionAnnotation ;
                                                                                               :emotion :fear ,
                                                                                                        :nervousness ;
                                                                                               :experiencer :legien_kromkamp ;
                                                                                               :framedBy <https://raw.githubusercontent.com/MaddaGh/DataProcessing_EmoAnnotation/main/meaw.ttl#46_1> ,
                                                                                                         <https://raw.githubusercontent.com/MaddaGh/DataProcessing_EmoAnnotation/main/meaw.ttl#46_2> ,
                                                                                                         <https://raw.githubusercontent.com/MaddaGh/DataProcessing_EmoAnnotation/main/meaw.ttl#46_3> ;
                                                                                               :hasAuralTrigger :laughter ;
                                                                                               :hasCameraFramingInterpretation :contextualizing ;
                                                                                               :hasFrameContext :saying_something_wrong ;
                                                                                               :hasTrigger :cover_mouth ,
                                                                                                           :laughter ;
                                                                                               :hasVisualTrigger :cover_mouth ;
                                                                                               :isInScopeOf :welles_nietes ;
                                                                                               :hasStart "469" ;
                                                                                               :hasText "Vrouw en wat ik nu zeg maar zo snel zou dus want dit nou dit voorbeeld aanhalen." .


###  https://raw.githubusercontent.com/MaddaGh/DataProcessing_EmoAnnotation/main/meaw.ttl#50_1
<https://raw.githubusercontent.com/MaddaGh/DataProcessing_EmoAnnotation/main/meaw.ttl#50_1> rdf:type owl:NamedIndividual ,
                                                                                                     :Frame ;
                                                                                            :frames <https://raw.githubusercontent.com/MaddaGh/DataProcessing_EmoAnnotation/main/meaw.ttl#50_anger> ;
                                                                                            :hasAngle :horizontal_frontal ;
                                                                                            :hasAuralComposition :aligned ;
                                                                                            :hasFramingTechnique :horizontal_frontal ,
                                                                                                                 :medium_close_up ,
                                                                                                                 :stationary ;
                                                                                            :hasMovement :stationary ;
                                                                                            :hasShotType :medium_close_up ;
                                                                                            :shows :eyes_up ,
                                                                                                   :gesticulation ,
                                                                                                   :look_forward ;
                                                                                            :showsEyes :eyes_up ,
                                                                                                       :look_forward ;
                                                                                            :showsHandGesture :gesticulation .


###  https://raw.githubusercontent.com/MaddaGh/DataProcessing_EmoAnnotation/main/meaw.ttl#50_anger
<https://raw.githubusercontent.com/MaddaGh/DataProcessing_EmoAnnotation/main/meaw.ttl#50_anger> rdf:type owl:NamedIndividual ,
                                                                                                         :EmotionAnnotation ,
                                                                                                         :ExperiencedEmotionAnnotation ,
                                                                                                         :PresentEmotionAnnotation ;
                                                                                                :emotion :frustration ;
                                                                                                :experiencer :adelheid_roosen ;
                                                                                                :framedBy <https://raw.githubusercontent.com/MaddaGh/DataProcessing_EmoAnnotation/main/meaw.ttl#50_1> ;
                                                                                                :hasAuralTrigger :stressed_syllables ;
                                                                                                :hasCameraFramingInterpretation :involvement ;
                                                                                                :hasFrameContext :disagreeing_with_opinion ;
                                                                                                :hasTrigger :frowning ,
                                                                                                            :lower_brow ,
                                                                                                            :stressed_syllables ;
                                                                                                :hasVisualTrigger :frowning ,
                                                                                                                  :lower_brow ;
                                                                                                :isInScopeOf :welles_nietes ;
                                                                                                :hasStart "537" ;
                                                                                                :hasText "Tien minuten aan het woord moet laten proberen een uitgangspunt te vinden waardoor je niet zoals in de meeste talkshows is dat je dus niet." .


###  https://raw.githubusercontent.com/MaddaGh/DataProcessing_EmoAnnotation/main/meaw.ttl#51_1
<https://raw.githubusercontent.com/MaddaGh/DataProcessing_EmoAnnotation/main/meaw.ttl#51_1> rdf:type owl:NamedIndividual ,
                                                                                                     :Frame ;
                                                                                            :frames <https://raw.githubusercontent.com/MaddaGh/DataProcessing_EmoAnnotation/main/meaw.ttl#51_anger> ;
                                                                                            :hasAngle :horizontal_frontal ;
                                                                                            :hasAuralComposition :aligned ;
                                                                                            :hasFramingTechnique :horizontal_frontal ,
                                                                                                                 :medium_close_up ,
                                                                                                                 :stationary ;
                                                                                            :hasMovement :stationary ;
                                                                                            :hasShotType :medium_close_up ;
                                                                                            :precedes <https://raw.githubusercontent.com/MaddaGh/DataProcessing_EmoAnnotation/main/meaw.ttl#51_2> ;
                                                                                            :shows :eyes_up ,
                                                                                                   :frowning ,
                                                                                                   :gesticulation ,
                                                                                                   :lower_brow ;
                                                                                            :showsExpression :frowning ,
                                                                                                             :lower_brow ;
                                                                                            :showsEyes :eyes_up ;
                                                                                            :showsHandGesture :gesticulation .


###  https://raw.githubusercontent.com/MaddaGh/DataProcessing_EmoAnnotation/main/meaw.ttl#51_2
<https://raw.githubusercontent.com/MaddaGh/DataProcessing_EmoAnnotation/main/meaw.ttl#51_2> rdf:type owl:NamedIndividual ,
                                                                                                     :Frame ;
                                                                                            :follows <https://raw.githubusercontent.com/MaddaGh/DataProcessing_EmoAnnotation/main/meaw.ttl#51_1> ;
                                                                                            :frames <https://raw.githubusercontent.com/MaddaGh/DataProcessing_EmoAnnotation/main/meaw.ttl#51_anger> ;
                                                                                            :hasAngle :horizontal_oblique ;
                                                                                            :hasAuralComposition :aligned ;
                                                                                            :hasFramingTechnique :horizontal_oblique ,
                                                                                                                 :medium_shot ,
                                                                                                                 :stationary ;
                                                                                            :hasMovement :stationary ;
                                                                                            :hasShotType :medium_shot ;
                                                                                            :shows :head_shake_up_and_down ,
                                                                                                   :strong_gesticulation ;
                                                                                            :showsHandGesture :strong_gesticulation ;
                                                                                            :showsHeadGesture :head_shake_up_and_down .


###  https://raw.githubusercontent.com/MaddaGh/DataProcessing_EmoAnnotation/main/meaw.ttl#51_anger
<https://raw.githubusercontent.com/MaddaGh/DataProcessing_EmoAnnotation/main/meaw.ttl#51_anger> rdf:type owl:NamedIndividual ,
                                                                                                         :EmotionAnnotation ,
                                                                                                         :ExperiencedEmotionAnnotation ,
                                                                                                         :PresentEmotionAnnotation ;
                                                                                                :emotion :frustration ;
                                                                                                :experiencer :adelheid_roosen ;
                                                                                                :framedBy <https://raw.githubusercontent.com/MaddaGh/DataProcessing_EmoAnnotation/main/meaw.ttl#51_1> ,
                                                                                                          <https://raw.githubusercontent.com/MaddaGh/DataProcessing_EmoAnnotation/main/meaw.ttl#51_2> ;
                                                                                                :hasAuralTrigger :tense_articulation ;
                                                                                                :hasCameraFramingInterpretation :conflict ;
                                                                                                :hasFrameContext :disagreeing_with_opinion ;
                                                                                                :hasTrigger :frowning ,
                                                                                                            :gekwetst ,
                                                                                                            :lower_brow ,
                                                                                                            :tense_articulation ;
                                                                                                :hasVerbalTrigger :gekwetst ;
                                                                                                :hasVisualTrigger :frowning ,
                                                                                                                  :lower_brow ;
                                                                                                :isInScopeOf :welles_nietes ;
                                                                                                :hasStart "548" ;
                                                                                                :hasText "Het moet kiezen voor de persoon in kwestie of voor degenen die de talkshow leidt dat ik dus echt met alle respect wie acht minuten aan die persoon wilde geven als mensen dan kwetsend als kwetsend ervaren dan ben ik dus nou daar weer gekwetst en dan houdt het verhaal van mij op het uefa niets meer." .


###  https://raw.githubusercontent.com/MaddaGh/DataProcessing_EmoAnnotation/main/meaw.ttl#55_1
<https://raw.githubusercontent.com/MaddaGh/DataProcessing_EmoAnnotation/main/meaw.ttl#55_1> rdf:type owl:NamedIndividual ,
                                                                                                     :Frame ;
                                                                                            :frames <https://raw.githubusercontent.com/MaddaGh/DataProcessing_EmoAnnotation/main/meaw.ttl#55_anger> ;
                                                                                            :hasAngle :horizontal_frontal ;
                                                                                            :hasAuralComposition :aligned ;
                                                                                            :hasFramingTechnique :close_up ,
                                                                                                                 :horizontal_frontal ,
                                                                                                                 :stationary ;
                                                                                            :hasMovement :stationary ;
                                                                                            :hasShotType :close_up ;
                                                                                            :precedes <https://raw.githubusercontent.com/MaddaGh/DataProcessing_EmoAnnotation/main/meaw.ttl#55_2> ;
                                                                                            :shows :frowning ,
                                                                                                   :lower_brow ,
                                                                                                   :raise_shoulder ,
                                                                                                   :turning_towards_interlocutor ;
                                                                                            :showsExpression :frowning ,
                                                                                                             :lower_brow ;
                                                                                            :showsMovement :raise_shoulder ,
                                                                                                           :turning_towards_interlocutor .


###  https://raw.githubusercontent.com/MaddaGh/DataProcessing_EmoAnnotation/main/meaw.ttl#55_2
<https://raw.githubusercontent.com/MaddaGh/DataProcessing_EmoAnnotation/main/meaw.ttl#55_2> rdf:type owl:NamedIndividual ,
                                                                                                     :Frame ;
                                                                                            :follows <https://raw.githubusercontent.com/MaddaGh/DataProcessing_EmoAnnotation/main/meaw.ttl#55_1> ;
                                                                                            :frames <https://raw.githubusercontent.com/MaddaGh/DataProcessing_EmoAnnotation/main/meaw.ttl#55_anger> ;
                                                                                            :hasAngle :reverse_shot ;
                                                                                            :hasAuralComposition :aligned ;
                                                                                            :hasFramingTechnique :medium_close_up ,
                                                                                                                 :reverse_shot ,
                                                                                                                 :stationary ;
                                                                                            :hasMovement :stationary ;
                                                                                            :hasShotType :medium_close_up ;
                                                                                            :precedes <https://raw.githubusercontent.com/MaddaGh/DataProcessing_EmoAnnotation/main/meaw.ttl#55_3> ;
                                                                                            :shows :eyes_up ,
                                                                                                   :make_eye_contact ,
                                                                                                   :raise_eyebrow ,
                                                                                                   :raise_outer_brow ;
                                                                                            :showsExpression :raise_eyebrow ,
                                                                                                             :raise_outer_brow ;
                                                                                            :showsEyes :eyes_up ,
                                                                                                       :make_eye_contact .


###  https://raw.githubusercontent.com/MaddaGh/DataProcessing_EmoAnnotation/main/meaw.ttl#55_3
<https://raw.githubusercontent.com/MaddaGh/DataProcessing_EmoAnnotation/main/meaw.ttl#55_3> rdf:type owl:NamedIndividual ,
                                                                                                     :Frame ;
                                                                                            :follows <https://raw.githubusercontent.com/MaddaGh/DataProcessing_EmoAnnotation/main/meaw.ttl#55_2> ;
                                                                                            :frames <https://raw.githubusercontent.com/MaddaGh/DataProcessing_EmoAnnotation/main/meaw.ttl#55_anger> ;
                                                                                            :hasAngle :horizontal_frontal ;
                                                                                            :hasAuralComposition :dialogue ;
                                                                                            :hasFramingTechnique :close_up ,
                                                                                                                 :horizontal_frontal ,
                                                                                                                 :stationary ;
                                                                                            :hasMovement :stationary ;
                                                                                            :hasShotType :close_up ;
                                                                                            :precedes <https://raw.githubusercontent.com/MaddaGh/DataProcessing_EmoAnnotation/main/meaw.ttl#55_4> ;
                                                                                            :shows :head_shake_up_and_down ;
                                                                                            :showsHeadGesture :head_shake_up_and_down .


###  https://raw.githubusercontent.com/MaddaGh/DataProcessing_EmoAnnotation/main/meaw.ttl#55_4
<https://raw.githubusercontent.com/MaddaGh/DataProcessing_EmoAnnotation/main/meaw.ttl#55_4> rdf:type owl:NamedIndividual ,
                                                                                                     :Frame ;
                                                                                            :follows <https://raw.githubusercontent.com/MaddaGh/DataProcessing_EmoAnnotation/main/meaw.ttl#55_3> ;
                                                                                            :frames <https://raw.githubusercontent.com/MaddaGh/DataProcessing_EmoAnnotation/main/meaw.ttl#55_anger> ;
                                                                                            :hasAngle :reverse_shot ;
                                                                                            :hasAuralComposition :dialogue ,
                                                                                                                 :voiceover ;
                                                                                            :hasFramingTechnique :medium_close_up ,
                                                                                                                 :reverse_shot ,
                                                                                                                 :stationary ;
                                                                                            :hasMovement :stationary ;
                                                                                            :hasShotType :medium_close_up ;
                                                                                            :precedes <https://raw.githubusercontent.com/MaddaGh/DataProcessing_EmoAnnotation/main/meaw.ttl#55_5> ;
                                                                                            :shows :head_shake_up_and_down ,
                                                                                                   :raise_eyebrow ,
                                                                                                   :raise_outer_brow ;
                                                                                            :showsExpression :raise_eyebrow ,
                                                                                                             :raise_outer_brow ;
                                                                                            :showsHeadGesture :head_shake_up_and_down .


###  https://raw.githubusercontent.com/MaddaGh/DataProcessing_EmoAnnotation/main/meaw.ttl#55_5
<https://raw.githubusercontent.com/MaddaGh/DataProcessing_EmoAnnotation/main/meaw.ttl#55_5> rdf:type owl:NamedIndividual ,
                                                                                                     :Frame ;
                                                                                            :follows <https://raw.githubusercontent.com/MaddaGh/DataProcessing_EmoAnnotation/main/meaw.ttl#55_4> ;
                                                                                            :frames <https://raw.githubusercontent.com/MaddaGh/DataProcessing_EmoAnnotation/main/meaw.ttl#55_anger> ;
                                                                                            :hasAngle :horizontal_frontal ;
                                                                                            :hasAuralComposition :dialogue ;
                                                                                            :hasFramingTechnique :close_up ,
                                                                                                                 :horizontal_frontal ,
                                                                                                                 :stationary ;
                                                                                            :hasMovement :stationary ;
                                                                                            :hasShotType :close_up ;
                                                                                            :shows :head_shake_up_and_down ,
                                                                                                   :make_eye_contact ;
                                                                                            :showsEyes :make_eye_contact ;
                                                                                            :showsHeadGesture :head_shake_up_and_down .


###  https://raw.githubusercontent.com/MaddaGh/DataProcessing_EmoAnnotation/main/meaw.ttl#55_anger
<https://raw.githubusercontent.com/MaddaGh/DataProcessing_EmoAnnotation/main/meaw.ttl#55_anger> rdf:type owl:NamedIndividual ,
                                                                                                         :EmotionAnnotation ,
                                                                                                         :ExperiencedEmotionAnnotation ,
                                                                                                         :PresentEmotionAnnotation ;
                                                                                                :emotion :argumentativeness ;
                                                                                                :experiencer :couple ;
                                                                                                :framedBy <https://raw.githubusercontent.com/MaddaGh/DataProcessing_EmoAnnotation/main/meaw.ttl#55_1> ,
                                                                                                          <https://raw.githubusercontent.com/MaddaGh/DataProcessing_EmoAnnotation/main/meaw.ttl#55_2> ,
                                                                                                          <https://raw.githubusercontent.com/MaddaGh/DataProcessing_EmoAnnotation/main/meaw.ttl#55_3> ,
                                                                                                          <https://raw.githubusercontent.com/MaddaGh/DataProcessing_EmoAnnotation/main/meaw.ttl#55_4> ,
                                                                                                          <https://raw.githubusercontent.com/MaddaGh/DataProcessing_EmoAnnotation/main/meaw.ttl#55_5> ;
                                                                                                :hasAuralTrigger :quick_bicker ;
                                                                                                :hasCameraFramingInterpretation :conflict ;
                                                                                                :hasFrameContext :disagreeing_by_interrupting ;
                                                                                                :hasTrigger :quick_bicker ,
                                                                                                            :raise_eyebrow ,
                                                                                                            :raise_outer_brow ;
                                                                                                :hasVisualTrigger :raise_eyebrow ,
                                                                                                                  :raise_outer_brow ;
                                                                                                :isInScopeOf :welles_nietes ;
                                                                                                :hasStart "592" ;
                                                                                                :hasText "Wat bedoelt u met seksuele manier nou aan borst te raken en dergelijke ik denk dat een heleboel transseksuelen zich gekwetst zouden voelen ik weet het zeker van niet nou ik weet het dus niet maar wel voor mijn gevoel dus ja voor mijn gevoel dus helemaal niet ik mag dus mijn gevoel uit afstaan." .


###  https://raw.githubusercontent.com/MaddaGh/DataProcessing_EmoAnnotation/main/meaw.ttl#57_1
<https://raw.githubusercontent.com/MaddaGh/DataProcessing_EmoAnnotation/main/meaw.ttl#57_1> rdf:type owl:NamedIndividual ,
                                                                                                     :Frame ;
                                                                                            :frames <https://raw.githubusercontent.com/MaddaGh/DataProcessing_EmoAnnotation/main/meaw.ttl#57_disgust> ;
                                                                                            :hasAngle :horizontal_frontal ;
                                                                                            :hasAuralComposition :speaker_in_background ;
                                                                                            :hasFramingTechnique :horizontal_frontal ,
                                                                                                                 :medium_long_shot ,
                                                                                                                 :pan_right ,
                                                                                                                 :zoom_out ;
                                                                                            :hasMovement :pan_right ,
                                                                                                         :zoom_out ;
                                                                                            :hasShotType :medium_long_shot ;
                                                                                            :precedes <https://raw.githubusercontent.com/MaddaGh/DataProcessing_EmoAnnotation/main/meaw.ttl#57_2> ;
                                                                                            :shows :leaning_towards_interlocutor ,
                                                                                                   :walking ;
                                                                                            :showsMovement :leaning_towards_interlocutor ,
                                                                                                           :walking .


###  https://raw.githubusercontent.com/MaddaGh/DataProcessing_EmoAnnotation/main/meaw.ttl#57_2
<https://raw.githubusercontent.com/MaddaGh/DataProcessing_EmoAnnotation/main/meaw.ttl#57_2> rdf:type owl:NamedIndividual ,
                                                                                                     :Frame ;
                                                                                            :follows <https://raw.githubusercontent.com/MaddaGh/DataProcessing_EmoAnnotation/main/meaw.ttl#57_1> ;
                                                                                            :frames <https://raw.githubusercontent.com/MaddaGh/DataProcessing_EmoAnnotation/main/meaw.ttl#57_disgust> ;
                                                                                            :hasAngle :horizontal_frontal ;
                                                                                            :hasAuralComposition :aligned ;
                                                                                            :hasFramingTechnique :horizontal_frontal ,
                                                                                                                 :medium_close_up ,
                                                                                                                 :stationary ;
                                                                                            :hasMovement :stationary ;
                                                                                            :hasShotType :medium_close_up ;
                                                                                            :shows :gesticulation ;
                                                                                            :showsHandGesture :gesticulation .


###  https://raw.githubusercontent.com/MaddaGh/DataProcessing_EmoAnnotation/main/meaw.ttl#57_disgust
<https://raw.githubusercontent.com/MaddaGh/DataProcessing_EmoAnnotation/main/meaw.ttl#57_disgust> rdf:type owl:NamedIndividual ,
                                                                                                           :EmotionAnnotation ,
                                                                                                           :ExperiencedEmotionAnnotation ,
                                                                                                           :PresentEmotionAnnotation ;
                                                                                                  :emotion :aversion ,
                                                                                                           :disgust ;
                                                                                                  :experiencer :anonymous1 ;
                                                                                                  :framedBy <https://raw.githubusercontent.com/MaddaGh/DataProcessing_EmoAnnotation/main/meaw.ttl#57_1> ,
                                                                                                            <https://raw.githubusercontent.com/MaddaGh/DataProcessing_EmoAnnotation/main/meaw.ttl#57_2> ;
                                                                                                  :hasCameraFramingInterpretation :engaging_with ;
                                                                                                  :hasFrameContext :presenting_opinion ;
                                                                                                  :hasTrigger :head_shake_side_to_side ,
                                                                                                              :headshake ;
                                                                                                  :hasVisualTrigger :head_shake_side_to_side ,
                                                                                                                    :headshake ;
                                                                                                  :isInScopeOf :welles_nietes ;
                                                                                                  :hasEnd "" ;
                                                                                                  :hasStart "612" ;
                                                                                                  :hasText "Ja ik woon vragen je hoorde zoveel kan je geen programma onderhand meer beginnen of moet homoseksuelen als transseksueel aan te pas komt zo over gewone mensen praten." .


###  https://raw.githubusercontent.com/MaddaGh/DataProcessing_EmoAnnotation/main/meaw.ttl#58_1
<https://raw.githubusercontent.com/MaddaGh/DataProcessing_EmoAnnotation/main/meaw.ttl#58_1> rdf:type owl:NamedIndividual ,
                                                                                                     :Frame ;
                                                                                            :frames <https://raw.githubusercontent.com/MaddaGh/DataProcessing_EmoAnnotation/main/meaw.ttl#58_anger> ;
                                                                                            :hasAngle :horizontal_frontal ;
                                                                                            :hasAuralComposition :muddle ;
                                                                                            :hasFramingTechnique :horizontal_frontal ,
                                                                                                                 :medium_long_shot ,
                                                                                                                 :stationary ;
                                                                                            :hasMovement :stationary ;
                                                                                            :hasShotType :medium_long_shot ;
                                                                                            :shows :look_forward ,
                                                                                                   :raise_chin ;
                                                                                            :showsExpression :raise_chin ;
                                                                                            :showsEyes :look_forward .


###  https://raw.githubusercontent.com/MaddaGh/DataProcessing_EmoAnnotation/main/meaw.ttl#58_anger
<https://raw.githubusercontent.com/MaddaGh/DataProcessing_EmoAnnotation/main/meaw.ttl#58_anger> rdf:type owl:NamedIndividual ,
                                                                                                         :EmotionAnnotation ,
                                                                                                         :ExperiencedEmotionAnnotation ,
                                                                                                         :PresentEmotionAnnotation ;
                                                                                                :emotion :anger ,
                                                                                                         :argumentativeness ;
                                                                                                :experiencer :adelheid_roosen ;
                                                                                                :framedBy <https://raw.githubusercontent.com/MaddaGh/DataProcessing_EmoAnnotation/main/meaw.ttl#58_1> ;
                                                                                                :hasAuralTrigger :tense_articulation ;
                                                                                                :hasCameraFramingInterpretation :contextualizing ;
                                                                                                :hasFrameContext :disagreeing_by_interrupting ;
                                                                                                :hasTrigger :tense_articulation ;
                                                                                                :isInScopeOf :welles_nietes ;
                                                                                                :hasStart "624" ;
                                                                                                :hasText "Dat zijn." .


#################################################################
#    General axioms
#################################################################

[ rdf:type owl:AllDisjointClasses ;
  owl:members ( :AuralTrigger
                :VerbalTrigger
                :VisualTrigger
              )
] .


[ rdf:type owl:AllDisjointClasses ;
  owl:members ( :FutureEmotionAnnotation
                :PastEmotionAnnotation
                :PresentEmotionAnnotation
              )
] .


#################################################################
#    Rules
#################################################################

:emoann rdf:type <http://www.w3.org/2003/11/swrl#Variable> .

:f1 rdf:type <http://www.w3.org/2003/11/swrl#Variable> .

:f2 rdf:type <http://www.w3.org/2003/11/swrl#Variable> .

[ <http://swrl.stanford.edu/ontologies/3.3/swrla.owl#isRuleEnabled> "true"^^xsd:boolean ;
   rdfs:comment "condition to declare that if a Frame1 follows a Frame2 that frames an EmotionAnnotation, then Frame1 also Frames the same EmotionAnntoation." ;
   rdfs:label "S1" ;
   rdf:type <http://www.w3.org/2003/11/swrl#Imp> ;
   <http://www.w3.org/2003/11/swrl#body> [ rdf:type <http://www.w3.org/2003/11/swrl#AtomList> ;
                                           rdf:first [ rdf:type <http://www.w3.org/2003/11/swrl#ClassAtom> ;
                                                       <http://www.w3.org/2003/11/swrl#classPredicate> :EmotionAnnotation ;
                                                       <http://www.w3.org/2003/11/swrl#argument1> :emoann
                                                     ] ;
                                           rdf:rest [ rdf:type <http://www.w3.org/2003/11/swrl#AtomList> ;
                                                      rdf:first [ rdf:type <http://www.w3.org/2003/11/swrl#IndividualPropertyAtom> ;
                                                                  <http://www.w3.org/2003/11/swrl#propertyPredicate> :frames ;
                                                                  <http://www.w3.org/2003/11/swrl#argument1> :f1 ;
                                                                  <http://www.w3.org/2003/11/swrl#argument2> :emoann
                                                                ] ;
                                                      rdf:rest [ rdf:type <http://www.w3.org/2003/11/swrl#AtomList> ;
                                                                 rdf:first [ rdf:type <http://www.w3.org/2003/11/swrl#ClassAtom> ;
                                                                             <http://www.w3.org/2003/11/swrl#classPredicate> :Frame ;
                                                                             <http://www.w3.org/2003/11/swrl#argument1> :f1
                                                                           ] ;
                                                                 rdf:rest [ rdf:type <http://www.w3.org/2003/11/swrl#AtomList> ;
                                                                            rdf:first [ rdf:type <http://www.w3.org/2003/11/swrl#IndividualPropertyAtom> ;
                                                                                        <http://www.w3.org/2003/11/swrl#propertyPredicate> :follows ;
                                                                                        <http://www.w3.org/2003/11/swrl#argument1> :f2 ;
                                                                                        <http://www.w3.org/2003/11/swrl#argument2> :f1
                                                                                      ] ;
                                                                            rdf:rest [ rdf:type <http://www.w3.org/2003/11/swrl#AtomList> ;
                                                                                       rdf:first [ rdf:type <http://www.w3.org/2003/11/swrl#ClassAtom> ;
                                                                                                   <http://www.w3.org/2003/11/swrl#classPredicate> :Frame ;
                                                                                                   <http://www.w3.org/2003/11/swrl#argument1> :f2
                                                                                                 ] ;
                                                                                       rdf:rest rdf:nil
                                                                                     ]
                                                                          ]
                                                               ]
                                                    ]
                                         ] ;
   <http://www.w3.org/2003/11/swrl#head> [ rdf:type <http://www.w3.org/2003/11/swrl#AtomList> ;
                                           rdf:first [ rdf:type <http://www.w3.org/2003/11/swrl#IndividualPropertyAtom> ;
                                                       <http://www.w3.org/2003/11/swrl#propertyPredicate> :frames ;
                                                       <http://www.w3.org/2003/11/swrl#argument1> :f2 ;
                                                       <http://www.w3.org/2003/11/swrl#argument2> :emoann
                                                     ] ;
                                           rdf:rest rdf:nil
                                         ]
 ] .

[ <http://swrl.stanford.edu/ontologies/3.3/swrla.owl#isRuleEnabled> "true"^^xsd:boolean ;
   rdfs:comment "Condition to declare the inverese rule of S1" ;
   rdfs:label "S2" ;
   rdf:type <http://www.w3.org/2003/11/swrl#Imp> ;
   <http://www.w3.org/2003/11/swrl#body> [ rdf:type <http://www.w3.org/2003/11/swrl#AtomList> ;
                                           rdf:first [ rdf:type <http://www.w3.org/2003/11/swrl#ClassAtom> ;
                                                       <http://www.w3.org/2003/11/swrl#classPredicate> :EmotionAnnotation ;
                                                       <http://www.w3.org/2003/11/swrl#argument1> :emoann
                                                     ] ;
                                           rdf:rest [ rdf:type <http://www.w3.org/2003/11/swrl#AtomList> ;
                                                      rdf:first [ rdf:type <http://www.w3.org/2003/11/swrl#IndividualPropertyAtom> ;
                                                                  <http://www.w3.org/2003/11/swrl#propertyPredicate> :framedBy ;
                                                                  <http://www.w3.org/2003/11/swrl#argument1> :emoann ;
                                                                  <http://www.w3.org/2003/11/swrl#argument2> :f1
                                                                ] ;
                                                      rdf:rest [ rdf:type <http://www.w3.org/2003/11/swrl#AtomList> ;
                                                                 rdf:first [ rdf:type <http://www.w3.org/2003/11/swrl#ClassAtom> ;
                                                                             <http://www.w3.org/2003/11/swrl#classPredicate> :Frame ;
                                                                             <http://www.w3.org/2003/11/swrl#argument1> :f1
                                                                           ] ;
                                                                 rdf:rest [ rdf:type <http://www.w3.org/2003/11/swrl#AtomList> ;
                                                                            rdf:first [ rdf:type <http://www.w3.org/2003/11/swrl#IndividualPropertyAtom> ;
                                                                                        <http://www.w3.org/2003/11/swrl#propertyPredicate> :precedes ;
                                                                                        <http://www.w3.org/2003/11/swrl#argument1> :f1 ;
                                                                                        <http://www.w3.org/2003/11/swrl#argument2> :f2
                                                                                      ] ;
                                                                            rdf:rest [ rdf:type <http://www.w3.org/2003/11/swrl#AtomList> ;
                                                                                       rdf:first [ rdf:type <http://www.w3.org/2003/11/swrl#ClassAtom> ;
                                                                                                   <http://www.w3.org/2003/11/swrl#classPredicate> :Frame ;
                                                                                                   <http://www.w3.org/2003/11/swrl#argument1> :f2
                                                                                                 ] ;
                                                                                       rdf:rest rdf:nil
                                                                                     ]
                                                                          ]
                                                               ]
                                                    ]
                                         ] ;
   <http://www.w3.org/2003/11/swrl#head> [ rdf:type <http://www.w3.org/2003/11/swrl#AtomList> ;
                                           rdf:first [ rdf:type <http://www.w3.org/2003/11/swrl#IndividualPropertyAtom> ;
                                                       <http://www.w3.org/2003/11/swrl#propertyPredicate> :framedBy ;
                                                       <http://www.w3.org/2003/11/swrl#argument1> :emoann ;
                                                       <http://www.w3.org/2003/11/swrl#argument2> :f2
                                                     ] ;
                                           rdf:rest rdf:nil
                                         ]
 ] .

###  Generated by the OWL API (version 4.5.26.2023-07-17T20:34:13Z) https://github.com/owlcs/owlapi
